<?xml version="1.0"?>
<rdf:RDF xmlns="http://purl.org/ica/ric#"
     xml:base="http://purl.org/ica/ric"
     xmlns:rdf="http://www.w3.org/1999/02/22-rdf-syntax-ns#"
     xmlns:owl="http://www.w3.org/2002/07/owl#"
     xmlns:xml="http://www.w3.org/XML/1998/namespace"
     xmlns:xsd="http://www.w3.org/2001/XMLSchema#"
     xmlns:dcterms="http://purl.org/dc/terms/"
     xmlns:skos="http://www.w3.org/2004/02/skos/core#"
     xmlns:rdfs="http://www.w3.org/2000/01/rdf-schema#"
     xmlns:ric="http://purl.org/ica/ric#"
     xmlns:dc="http://purl.org/dc/elements/1.1/"
     xmlns:example="http://example.org/">
    <owl:Ontology rdf:about="http://purl.org/ica/ric">
        <owl:imports rdf:resource="http://protege.stanford.edu/plugins/owl/dc/dublincore.owl"/>
        <owl:imports rdf:resource="http://www.w3.org/2004/02/skos/core"/>
        <dcterms:creator xml:lang="es">Juan-Antonio Pastor-Sánchez (pastor@um.es)</dcterms:creator>
        <skos:changeNote xml:lang="en">Changes from versión 0.1: a) Duplicate object/datatype properties for resources/values had been defined as simultaneously as owl:ObjectProperty and owl:DatatypeProperty because there is not any OWL axiom that define these classes as pairwise disjoint.</skos:changeNote>
        <dcterms:title xml:lang="en">Records in Contexts Ontology</dcterms:title>
        <owl:versionInfo xml:lang="en">0.2</owl:versionInfo>
        <skos:changeNote xml:lang="en">Adopted the namespace http://purl.org/ica/ric instead http://www.example.org/ric</skos:changeNote>
        <dcterms:description xml:lang="en">Non Oficial Ontology based on the interpretation of the International Council on Archives&apos; document &quot;Records in Contexts: A conceptual Model for Archival Description&quot; (Consultation Draft v0.1 - September 2016)</dcterms:description>
        <dcterms:created xml:lang="en">2017-04-28</dcterms:created>
        <dcterms:license>http://creativecommons.org/licenses/by-nc-sa/4.0</dcterms:license>
    </owl:Ontology>
    


    <!-- 
    ///////////////////////////////////////////////////////////////////////////////////////
    //
    // Object Properties
    //
    ///////////////////////////////////////////////////////////////////////////////////////
     -->

    


    <!-- http://purl.org/ica/ric#RiC-P-accrualStatus -->

    <owl:ObjectProperty rdf:about="http://purl.org/ica/ric#RiC-P-accrualStatus">
        <rdfs:domain rdf:resource="http://purl.org/ica/ric#RiC-E3-RecordSet"/>
    </owl:ObjectProperty>
    


    <!-- http://purl.org/ica/ric#RiC-P-classification -->

    <owl:ObjectProperty rdf:about="http://purl.org/ica/ric#RiC-P-classification">
        <rdfs:domain>
            <owl:Class>
                <owl:unionOf rdf:parseType="Collection">
                    <rdf:Description rdf:about="http://purl.org/ica/ric#RiC-E1-Record"/>
                    <rdf:Description rdf:about="http://purl.org/ica/ric#RiC-E3-RecordSet"/>
                </owl:unionOf>
            </owl:Class>
        </rdfs:domain>
    </owl:ObjectProperty>
    


    <!-- http://purl.org/ica/ric#RiC-P-contentType -->

    <owl:ObjectProperty rdf:about="http://purl.org/ica/ric#RiC-P-contentType">
        <rdfs:domain>
            <owl:Class>
                <owl:unionOf rdf:parseType="Collection">
                    <rdf:Description rdf:about="http://purl.org/ica/ric#RiC-E1-Record"/>
                    <rdf:Description rdf:about="http://purl.org/ica/ric#RiC-E3-RecordSet"/>
                </owl:unionOf>
            </owl:Class>
        </rdfs:domain>
    </owl:ObjectProperty>
    


    <!-- http://purl.org/ica/ric#RiC-P-encodingFormat -->

    <owl:ObjectProperty rdf:about="http://purl.org/ica/ric#RiC-P-encodingFormat">
        <rdfs:domain>
            <owl:Class>
                <owl:unionOf rdf:parseType="Collection">
                    <rdf:Description rdf:about="http://purl.org/ica/ric#RiC-E1-Record"/>
                    <rdf:Description rdf:about="http://purl.org/ica/ric#RiC-E3-RecordSet"/>
                </owl:unionOf>
            </owl:Class>
        </rdfs:domain>
    </owl:ObjectProperty>
    


    <!-- http://purl.org/ica/ric#RiC-P-gender -->

    <owl:ObjectProperty rdf:about="http://purl.org/ica/ric#RiC-P-gender">
        <rdfs:domain rdf:resource="http://purl.org/ica/ric#RiC-E4-Agent-Person"/>
    </owl:ObjectProperty>
    


    <!-- http://purl.org/ica/ric#RiC-P-geographicCoordinates -->

    <owl:ObjectProperty rdf:about="http://purl.org/ica/ric#RiC-P-geographicCoordinates">
        <rdfs:domain rdf:resource="http://purl.org/ica/ric#RiC-E13-Place"/>
    </owl:ObjectProperty>
    


    <!-- http://purl.org/ica/ric#RiC-P-identityType -->

    <owl:ObjectProperty rdf:about="http://purl.org/ica/ric#RiC-P-identityType">
        <rdfs:domain rdf:resource="http://purl.org/ica/ric#RiC-E4-Agent"/>
    </owl:ObjectProperty>
    


    <!-- http://purl.org/ica/ric#RiC-P-languageInformation -->

    <owl:ObjectProperty rdf:about="http://purl.org/ica/ric#RiC-P-languageInformation">
        <rdfs:domain>
            <owl:Class>
                <owl:unionOf rdf:parseType="Collection">
                    <rdf:Description rdf:about="http://purl.org/ica/ric#RiC-E1-Record"/>
                    <rdf:Description rdf:about="http://purl.org/ica/ric#RiC-E3-RecordSet"/>
                    <rdf:Description rdf:about="http://purl.org/ica/ric#RiC-E4-Agent"/>
                </owl:unionOf>
            </owl:Class>
        </rdfs:domain>
    </owl:ObjectProperty>
    


    <!-- http://purl.org/ica/ric#RiC-P-mediaType -->

    <owl:ObjectProperty rdf:about="http://purl.org/ica/ric#RiC-P-mediaType">
        <rdfs:domain>
            <owl:Class>
                <owl:unionOf rdf:parseType="Collection">
                    <rdf:Description rdf:about="http://purl.org/ica/ric#RiC-E1-Record"/>
                    <rdf:Description rdf:about="http://purl.org/ica/ric#RiC-E3-RecordSet"/>
                </owl:unionOf>
            </owl:Class>
        </rdfs:domain>
    </owl:ObjectProperty>
    


    <!-- http://purl.org/ica/ric#RiC-P-medium -->

    <owl:ObjectProperty rdf:about="http://purl.org/ica/ric#RiC-P-medium">
        <rdfs:domain>
            <owl:Class>
                <owl:unionOf rdf:parseType="Collection">
                    <rdf:Description rdf:about="http://purl.org/ica/ric#RiC-E1-Record"/>
                    <rdf:Description rdf:about="http://purl.org/ica/ric#RiC-E3-RecordSet"/>
                </owl:unionOf>
            </owl:Class>
        </rdfs:domain>
    </owl:ObjectProperty>
    


    <!-- http://purl.org/ica/ric#RiC-P-name -->

    <owl:ObjectProperty rdf:about="http://purl.org/ica/ric#RiC-P-name">
        <rdfs:domain>
            <owl:Class>
                <owl:unionOf rdf:parseType="Collection">
                    <rdf:Description rdf:about="http://purl.org/ica/ric#RiC-E1-Record"/>
                    <rdf:Description rdf:about="http://purl.org/ica/ric#RiC-E10-Mandate"/>
                    <rdf:Description rdf:about="http://purl.org/ica/ric#RiC-E11-DocumentaryForm"/>
                    <rdf:Description rdf:about="http://purl.org/ica/ric#RiC-E12-Date"/>
                    <rdf:Description rdf:about="http://purl.org/ica/ric#RiC-E13-Place"/>
                    <rdf:Description rdf:about="http://purl.org/ica/ric#RiC-E14-ConceptThing"/>
                    <rdf:Description rdf:about="http://purl.org/ica/ric#RiC-E2-RecordComponent"/>
                    <rdf:Description rdf:about="http://purl.org/ica/ric#RiC-E3-RecordSet"/>
                    <rdf:Description rdf:about="http://purl.org/ica/ric#RiC-E4-Agent"/>
                    <rdf:Description rdf:about="http://purl.org/ica/ric#RiC-E5-Occupation"/>
                    <rdf:Description rdf:about="http://purl.org/ica/ric#RiC-E6-Position"/>
                    <rdf:Description rdf:about="http://purl.org/ica/ric#RiC-E7-Function"/>
                    <rdf:Description rdf:about="http://purl.org/ica/ric#RiC-E8-FunctionAbstract"/>
                    <rdf:Description rdf:about="http://purl.org/ica/ric#RiC-E9-Activity"/>
                </owl:unionOf>
            </owl:Class>
        </rdfs:domain>
    </owl:ObjectProperty>
    


    <!-- http://purl.org/ica/ric#RiC-P-place -->

    <owl:ObjectProperty rdf:about="http://purl.org/ica/ric#RiC-P-place"/>
    


    <!-- http://purl.org/ica/ric#RiC-P-productionTechnique -->

    <owl:ObjectProperty rdf:about="http://purl.org/ica/ric#RiC-P-productionTechnique">
        <rdfs:domain>
            <owl:Class>
                <owl:unionOf rdf:parseType="Collection">
                    <rdf:Description rdf:about="http://purl.org/ica/ric#RiC-E1-Record"/>
                    <rdf:Description rdf:about="http://purl.org/ica/ric#RiC-E3-RecordSet"/>
                </owl:unionOf>
            </owl:Class>
        </rdfs:domain>
    </owl:ObjectProperty>
    


    <!-- http://purl.org/ica/ric#RiC-P-recordState -->

    <owl:ObjectProperty rdf:about="http://purl.org/ica/ric#RiC-P-recordState">
        <rdfs:domain>
            <owl:Class>
                <owl:unionOf rdf:parseType="Collection">
                    <rdf:Description rdf:about="http://purl.org/ica/ric#RiC-E1-Record"/>
                    <rdf:Description rdf:about="http://purl.org/ica/ric#RiC-E3-RecordSet"/>
                </owl:unionOf>
            </owl:Class>
        </rdfs:domain>
    </owl:ObjectProperty>
    


    <!-- http://purl.org/ica/ric#RiC-P-type -->

    <owl:ObjectProperty rdf:about="http://purl.org/ica/ric#RiC-P-type">
        <rdfs:domain>
            <owl:Class>
                <owl:unionOf rdf:parseType="Collection">
                    <rdf:Description rdf:about="http://purl.org/ica/ric#RiC-E10-Mandate"/>
                    <rdf:Description rdf:about="http://purl.org/ica/ric#RiC-E11-DocumentaryForm"/>
                    <rdf:Description rdf:about="http://purl.org/ica/ric#RiC-E12-Date"/>
                    <rdf:Description rdf:about="http://purl.org/ica/ric#RiC-E13-Place"/>
                    <rdf:Description rdf:about="http://purl.org/ica/ric#RiC-E14-ConceptThing"/>
                    <rdf:Description rdf:about="http://purl.org/ica/ric#RiC-E3-RecordSet"/>
                    <rdf:Description rdf:about="http://purl.org/ica/ric#RiC-E4-Agent"/>
                    <rdf:Description rdf:about="http://purl.org/ica/ric#RiC-E5-Occupation"/>
                    <rdf:Description rdf:about="http://purl.org/ica/ric#RiC-E6-Position"/>
                    <rdf:Description rdf:about="http://purl.org/ica/ric#RiC-E7-Function"/>
                    <rdf:Description rdf:about="http://purl.org/ica/ric#RiC-E9-Activity"/>
                </owl:unionOf>
            </owl:Class>
        </rdfs:domain>
    </owl:ObjectProperty>
    


    <!-- http://purl.org/ica/ric#RiC-R-accumulated -->

    <owl:ObjectProperty rdf:about="http://purl.org/ica/ric#RiC-R-accumulated">
        <owl:inverseOf rdf:resource="http://purl.org/ica/ric#RiC-R-wasAccumulatedBy"/>
        <rdfs:domain rdf:resource="http://purl.org/ica/ric#RiC-E4-Agent"/>
        <rdfs:range rdf:resource="http://purl.org/ica/ric#RiC-E3-RecordSet"/>
        <rdfs:comment xml:lang="en">Relations RiC-R232</rdfs:comment>
        <rdfs:label xml:lang="en">accumulated</rdfs:label>
    </owl:ObjectProperty>
    


    <!-- http://purl.org/ica/ric#RiC-R-arranged -->

    <owl:ObjectProperty rdf:about="http://purl.org/ica/ric#RiC-R-arranged">
        <owl:inverseOf rdf:resource="http://purl.org/ica/ric#RiC-R-wasArrangedBy"/>
        <rdfs:domain rdf:resource="http://purl.org/ica/ric#RiC-E4-Agent"/>
        <rdfs:range rdf:resource="http://purl.org/ica/ric#RiC-E3-RecordSet"/>
        <rdfs:comment xml:lang="en">Relations RiC-R233</rdfs:comment>
        <rdfs:label xml:lang="en">arranged</rdfs:label>
    </owl:ObjectProperty>
    


    <!-- http://purl.org/ica/ric#RiC-R-assembled -->

    <owl:ObjectProperty rdf:about="http://purl.org/ica/ric#RiC-R-assembled">
        <owl:inverseOf rdf:resource="http://purl.org/ica/ric#RiC-R-wasAssembledBy"/>
        <rdfs:domain rdf:resource="http://purl.org/ica/ric#RiC-E4-Agent"/>
        <rdfs:range rdf:resource="http://purl.org/ica/ric#RiC-E3-RecordSet"/>
        <rdfs:comment xml:lang="en">Relations RiC-R234</rdfs:comment>
        <rdfs:label xml:lang="en">assembled</rdfs:label>
    </owl:ObjectProperty>
    


    <!-- http://purl.org/ica/ric#RiC-R-authored -->

    <owl:ObjectProperty rdf:about="http://purl.org/ica/ric#RiC-R-authored">
        <owl:inverseOf rdf:resource="http://purl.org/ica/ric#RiC-R-wasAuthoredBy"/>
        <rdfs:domain rdf:resource="http://purl.org/ica/ric#RiC-E4-Agent"/>
        <rdfs:range>
            <owl:Class>
                <owl:unionOf rdf:parseType="Collection">
                    <rdf:Description rdf:about="http://purl.org/ica/ric#RiC-E1-Record"/>
                    <rdf:Description rdf:about="http://purl.org/ica/ric#RiC-E2-RecordComponent"/>
                </owl:unionOf>
            </owl:Class>
        </rdfs:range>
        <rdfs:comment xml:lang="en">Relations RiC-R204, RiC-R219</rdfs:comment>
        <rdfs:label xml:lang="en">authored</rdfs:label>
    </owl:ObjectProperty>
    


    <!-- http://purl.org/ica/ric#RiC-R-authorized -->

    <owl:ObjectProperty rdf:about="http://purl.org/ica/ric#RiC-R-authorized">
        <owl:inverseOf rdf:resource="http://purl.org/ica/ric#RiC-R-wasAuthorizedBy"/>
        <rdfs:domain rdf:resource="http://purl.org/ica/ric#RiC-E10-Mandate"/>
        <rdfs:range rdf:resource="http://purl.org/ica/ric#RiC-E4-Agent"/>
        <rdfs:comment xml:lang="en">Relations RiC-R572</rdfs:comment>
        <rdfs:label xml:lang="en">authorized</rdfs:label>
    </owl:ObjectProperty>
    


    <!-- http://purl.org/ica/ric#RiC-R-collected -->

    <owl:ObjectProperty rdf:about="http://purl.org/ica/ric#RiC-R-collected">
        <owl:inverseOf rdf:resource="http://purl.org/ica/ric#RiC-R-wasCollectedBy"/>
        <rdfs:domain rdf:resource="http://purl.org/ica/ric#RiC-E4-Agent"/>
        <rdfs:range>
            <owl:Class>
                <owl:unionOf rdf:parseType="Collection">
                    <rdf:Description rdf:about="http://purl.org/ica/ric#RiC-E1-Record"/>
                    <rdf:Description rdf:about="http://purl.org/ica/ric#RiC-E2-RecordComponent"/>
                    <rdf:Description rdf:about="http://purl.org/ica/ric#RiC-E3-RecordSet"/>
                </owl:unionOf>
            </owl:Class>
        </rdfs:range>
        <rdfs:comment xml:lang="en">Relations RiC-R205, RiC-R220, RiC-R235</rdfs:comment>
        <rdfs:label xml:lang="en">collected</rdfs:label>
    </owl:ObjectProperty>
    


    <!-- http://purl.org/ica/ric#RiC-R-controlled -->

    <owl:ObjectProperty rdf:about="http://purl.org/ica/ric#RiC-R-controlled">
        <owl:inverseOf rdf:resource="http://purl.org/ica/ric#RiC-R-wasControlledBy"/>
        <rdfs:domain rdf:resource="http://purl.org/ica/ric#RiC-E4-Agent"/>
        <rdfs:range rdf:resource="http://purl.org/ica/ric#RiC-E4-Agent"/>
        <rdfs:comment xml:lang="en">Relations RiC-R250</rdfs:comment>
        <rdfs:label xml:lang="en">controlled</rdfs:label>
        <rdfs:seeAlso rdf:resource="http://purl.org/ica/ric#RiC-R-controls"/>
    </owl:ObjectProperty>
    


    <!-- http://purl.org/ica/ric#RiC-R-controls -->

    <owl:ObjectProperty rdf:about="http://purl.org/ica/ric#RiC-R-controls">
        <owl:inverseOf rdf:resource="http://purl.org/ica/ric#RiC-R-isControlledBy"/>
        <rdfs:domain rdf:resource="http://purl.org/ica/ric#RiC-E4-Agent"/>
        <rdfs:range rdf:resource="http://purl.org/ica/ric#RiC-E4-Agent"/>
        <rdfs:comment xml:lang="en">Relations RiC-R251</rdfs:comment>
        <rdfs:label xml:lang="en">controls</rdfs:label>
        <rdfs:seeAlso rdf:resource="http://purl.org/ica/ric#RiC-R-controlled"/>
    </owl:ObjectProperty>
    


    <!-- http://purl.org/ica/ric#RiC-R-created -->

    <owl:ObjectProperty rdf:about="http://purl.org/ica/ric#RiC-R-created">
        <owl:inverseOf rdf:resource="http://purl.org/ica/ric#RiC-R-wasCreatedBy"/>
        <rdfs:domain rdf:resource="http://purl.org/ica/ric#RiC-E4-Agent"/>
        <rdfs:range>
            <owl:Class>
                <owl:unionOf rdf:parseType="Collection">
                    <rdf:Description rdf:about="http://purl.org/ica/ric#RiC-E1-Record"/>
                    <rdf:Description rdf:about="http://purl.org/ica/ric#RiC-E2-RecordComponent"/>
                    <rdf:Description rdf:about="http://purl.org/ica/ric#RiC-E3-RecordSet"/>
                    <rdf:Description rdf:about="http://purl.org/ica/ric#RiC-E4-Agent-DelegateAgent"/>
                </owl:unionOf>
            </owl:Class>
        </rdfs:range>
        <rdfs:comment xml:lang="en">Relations RiC-R206, RiC-R221, RiC-R236, RiC-R252</rdfs:comment>
        <rdfs:label xml:lang="en">created</rdfs:label>
    </owl:ObjectProperty>
    


    <!-- http://purl.org/ica/ric#RiC-R-defined -->

    <owl:ObjectProperty rdf:about="http://purl.org/ica/ric#RiC-R-defined">
        <owl:inverseOf rdf:resource="http://purl.org/ica/ric#RiC-R-wasDefinedBy"/>
        <rdfs:domain rdf:resource="http://purl.org/ica/ric#RiC-E10-Mandate"/>
        <rdfs:range>
            <owl:Class>
                <owl:unionOf rdf:parseType="Collection">
                    <rdf:Description rdf:about="http://purl.org/ica/ric#RiC-E6-Position"/>
                    <rdf:Description rdf:about="http://purl.org/ica/ric#RiC-E7-Function"/>
                    <rdf:Description rdf:about="http://purl.org/ica/ric#RiC-E9-Activity"/>
                </owl:unionOf>
            </owl:Class>
        </rdfs:range>
        <rdfs:comment xml:lang="en">Relations RiC-R577, RiC-R582, RiC-R589</rdfs:comment>
        <rdfs:label xml:lang="en">defined</rdfs:label>
        <rdfs:seeAlso rdf:resource="http://purl.org/ica/ric#RiC-R-defines"/>
    </owl:ObjectProperty>
    


    <!-- http://purl.org/ica/ric#RiC-R-defines -->

    <owl:ObjectProperty rdf:about="http://purl.org/ica/ric#RiC-R-defines">
        <owl:inverseOf rdf:resource="http://purl.org/ica/ric#RiC-R-isDefinedBy"/>
        <rdfs:domain rdf:resource="http://purl.org/ica/ric#RiC-E10-Mandate"/>
        <rdfs:range>
            <owl:Class>
                <owl:unionOf rdf:parseType="Collection">
                    <rdf:Description rdf:about="http://purl.org/ica/ric#RiC-E6-Position"/>
                    <rdf:Description rdf:about="http://purl.org/ica/ric#RiC-E7-Function"/>
                    <rdf:Description rdf:about="http://purl.org/ica/ric#RiC-E9-Activity"/>
                </owl:unionOf>
            </owl:Class>
        </rdfs:range>
        <rdfs:comment xml:lang="en">Relations RiC-R578, RiC-R583, RiC-R590</rdfs:comment>
        <rdfs:label xml:lang="en">defines</rdfs:label>
        <rdfs:seeAlso rdf:resource="http://purl.org/ica/ric#RiC-R-defined"/>
    </owl:ObjectProperty>
    


    <!-- http://purl.org/ica/ric#RiC-R-established -->

    <owl:ObjectProperty rdf:about="http://purl.org/ica/ric#RiC-R-established">
        <owl:inverseOf rdf:resource="http://purl.org/ica/ric#RiC-R-wasEstablishedBy"/>
        <rdfs:domain rdf:resource="http://purl.org/ica/ric#RiC-E4-Agent-Group"/>
        <rdfs:range rdf:resource="http://purl.org/ica/ric#RiC-E6-Position"/>
        <rdfs:comment xml:lang="en">Relations RiC-R296</rdfs:comment>
        <rdfs:label xml:lang="en">established</rdfs:label>
    </owl:ObjectProperty>
    


    <!-- http://purl.org/ica/ric#RiC-R-fulfilled -->

    <owl:ObjectProperty rdf:about="http://purl.org/ica/ric#RiC-R-fulfilled">
        <owl:inverseOf rdf:resource="http://purl.org/ica/ric#RiC-R-wasFulfilledBy"/>
        <rdfs:domain rdf:resource="http://purl.org/ica/ric#RiC-E4-Agent"/>
        <rdfs:range rdf:resource="http://purl.org/ica/ric#RiC-E7-Function"/>
        <rdfs:comment xml:lang="en">Relations RiC-R301</rdfs:comment>
        <rdfs:label xml:lang="en">fulfilled</rdfs:label>
        <rdfs:seeAlso rdf:resource="http://purl.org/ica/ric#RiC-R-fulfils"/>
    </owl:ObjectProperty>
    


    <!-- http://purl.org/ica/ric#RiC-R-fulfils -->

    <owl:ObjectProperty rdf:about="http://purl.org/ica/ric#RiC-R-fulfils">
        <owl:inverseOf rdf:resource="http://purl.org/ica/ric#RiC-R-isFulfilledBy"/>
        <rdfs:domain rdf:resource="http://purl.org/ica/ric#RiC-E4-Agent"/>
        <rdfs:range rdf:resource="http://purl.org/ica/ric#RiC-E7-Function"/>
        <rdfs:comment xml:lang="en">Relations RiC-R302</rdfs:comment>
        <rdfs:label xml:lang="en">fulfils</rdfs:label>
        <rdfs:seeAlso rdf:resource="http://purl.org/ica/ric#RiC-R-fulfilled"/>
    </owl:ObjectProperty>
    


    <!-- http://purl.org/ica/ric#RiC-R-hadActiveDate -->

    <owl:ObjectProperty rdf:about="http://purl.org/ica/ric#RiC-R-hadActiveDate">
        <owl:inverseOf rdf:resource="http://purl.org/ica/ric#RiC-R-wasActiveDateOf"/>
        <rdfs:domain>
            <owl:Class>
                <owl:unionOf rdf:parseType="Collection">
                    <rdf:Description rdf:about="http://purl.org/ica/ric#RiC-E10-Mandate"/>
                    <rdf:Description rdf:about="http://purl.org/ica/ric#RiC-E13-Place"/>
                    <rdf:Description rdf:about="http://purl.org/ica/ric#RiC-E4-Agent"/>
                    <rdf:Description rdf:about="http://purl.org/ica/ric#RiC-E7-Function"/>
                    <rdf:Description rdf:about="http://purl.org/ica/ric#RiC-E9-Activity"/>
                </owl:unionOf>
            </owl:Class>
        </rdfs:domain>
        <rdfs:range rdf:resource="http://purl.org/ica/ric#RiC-E12-Date"/>
        <rdfs:comment xml:lang="en">Relations RiC-R316, RiC-R466, RiC-R550, RiC-R600, RiC-R751</rdfs:comment>
        <rdfs:label xml:lang="en">had active date</rdfs:label>
        <rdfs:seeAlso rdf:resource="http://purl.org/ica/ric#RiC-R-hasActiveDate"/>
    </owl:ObjectProperty>
    


    <!-- http://purl.org/ica/ric#RiC-R-hadBirthDate -->

    <owl:ObjectProperty rdf:about="http://purl.org/ica/ric#RiC-R-hadBirthDate">
        <owl:inverseOf rdf:resource="http://purl.org/ica/ric#RiC-R-wasBirthDateOf"/>
        <rdfs:domain rdf:resource="http://purl.org/ica/ric#RiC-E4-Agent-Person"/>
        <rdfs:range rdf:resource="http://purl.org/ica/ric#RiC-E12-Date"/>
        <rdfs:comment xml:lang="en">Relations RiC-R317</rdfs:comment>
        <rdfs:label xml:lang="en">had birth date</rdfs:label>
    </owl:ObjectProperty>
    


    <!-- http://purl.org/ica/ric#RiC-R-hadBirthPlace -->

    <owl:ObjectProperty rdf:about="http://purl.org/ica/ric#RiC-R-hadBirthPlace">
        <owl:inverseOf rdf:resource="http://purl.org/ica/ric#RiC-R-wasBirthPlaceOf"/>
        <rdfs:domain rdf:resource="http://purl.org/ica/ric#RiC-E4-Agent-Person"/>
        <rdfs:range rdf:resource="http://purl.org/ica/ric#RiC-E13-Place"/>
        <rdfs:comment xml:lang="en">Relations RiC-R325</rdfs:comment>
        <rdfs:label xml:lang="en">had birth place</rdfs:label>
    </owl:ObjectProperty>
    


    <!-- http://purl.org/ica/ric#RiC-R-hadCitizen -->

    <owl:ObjectProperty rdf:about="http://purl.org/ica/ric#RiC-R-hadCitizen">
        <owl:inverseOf rdf:resource="http://purl.org/ica/ric#RiC-R-wasCitizenOf"/>
        <rdfs:domain rdf:resource="http://purl.org/ica/ric#RiC-E13-Place"/>
        <rdfs:range rdf:resource="http://purl.org/ica/ric#RiC-E4-Agent-Person"/>
        <rdfs:comment xml:lang="en">Relations RiC-R725</rdfs:comment>
        <rdfs:label xml:lang="en">had citizen</rdfs:label>
        <rdfs:seeAlso rdf:resource="http://purl.org/ica/ric#RiC-R-hasCitizen"/>
    </owl:ObjectProperty>
    


    <!-- http://purl.org/ica/ric#RiC-R-hadCreationDate -->

    <owl:ObjectProperty rdf:about="http://purl.org/ica/ric#RiC-R-hadCreationDate">
        <owl:inverseOf rdf:resource="http://purl.org/ica/ric#RiC-R-wasCreationDateOf"/>
        <rdfs:domain>
            <owl:Class>
                <owl:unionOf rdf:parseType="Collection">
                    <rdf:Description rdf:about="http://purl.org/ica/ric#RiC-E1-Record"/>
                    <rdf:Description rdf:about="http://purl.org/ica/ric#RiC-E2-RecordComponent"/>
                    <rdf:Description rdf:about="http://purl.org/ica/ric#RiC-E3-RecordSet"/>
                </owl:unionOf>
            </owl:Class>
        </rdfs:domain>
        <rdfs:range rdf:resource="http://purl.org/ica/ric#RiC-E12-Date"/>
        <rdfs:comment xml:lang="en">Relations RiC-R62, RiC-R122, RiC-R191</rdfs:comment>
        <rdfs:label xml:lang="en">had creation date</rdfs:label>
    </owl:ObjectProperty>
    


    <!-- http://purl.org/ica/ric#RiC-R-hadDeathDate -->

    <owl:ObjectProperty rdf:about="http://purl.org/ica/ric#RiC-R-hadDeathDate">
        <owl:inverseOf rdf:resource="http://purl.org/ica/ric#RiC-R-wasDeathDateOf"/>
        <rdfs:domain rdf:resource="http://purl.org/ica/ric#RiC-E4-Agent-Person"/>
        <rdfs:range rdf:resource="http://purl.org/ica/ric#RiC-E12-Date"/>
        <rdfs:comment xml:lang="en">Relations RiC-R318</rdfs:comment>
        <rdfs:label xml:lang="en">had death date</rdfs:label>
    </owl:ObjectProperty>
    


    <!-- http://purl.org/ica/ric#RiC-R-hadDeathPlace -->

    <owl:ObjectProperty rdf:about="http://purl.org/ica/ric#RiC-R-hadDeathPlace">
        <owl:inverseOf rdf:resource="http://purl.org/ica/ric#RiC-R-wasDeathPlaceOf"/>
        <rdfs:domain rdf:resource="http://purl.org/ica/ric#RiC-E4-Agent-Person"/>
        <rdfs:range rdf:resource="http://purl.org/ica/ric#RiC-E13-Place"/>
        <rdfs:comment xml:lang="en">Relations RiC-R326</rdfs:comment>
        <rdfs:label xml:lang="en">had death place</rdfs:label>
    </owl:ObjectProperty>
    


    <!-- http://purl.org/ica/ric#RiC-R-hadEndDate -->

    <owl:ObjectProperty rdf:about="http://purl.org/ica/ric#RiC-R-hadEndDate">
        <owl:inverseOf rdf:resource="http://purl.org/ica/ric#RiC-R-wasEndDateOf"/>
        <rdfs:domain>
            <owl:Class>
                <owl:unionOf rdf:parseType="Collection">
                    <rdf:Description rdf:about="http://purl.org/ica/ric#RiC-E10-Mandate"/>
                    <rdf:Description rdf:about="http://purl.org/ica/ric#RiC-E13-Place"/>
                    <rdf:Description rdf:about="http://purl.org/ica/ric#RiC-E4-Agent-Group"/>
                    <rdf:Description rdf:about="http://purl.org/ica/ric#RiC-E6-Position"/>
                    <rdf:Description rdf:about="http://purl.org/ica/ric#RiC-E7-Function"/>
                    <rdf:Description rdf:about="http://purl.org/ica/ric#RiC-E9-Activity"/>
                </owl:unionOf>
            </owl:Class>
        </rdfs:domain>
        <rdfs:range rdf:resource="http://purl.org/ica/ric#RiC-E12-Date"/>
        <rdfs:comment xml:lang="en">Relations RiC-R319, RiC-R413, RiC-R467, RiC-R551, RiC-R601, RiC-R752</rdfs:comment>
        <rdfs:label xml:lang="en">had end date</rdfs:label>
        <rdfs:seeAlso rdf:resource="http://purl.org/ica/ric#RiC-R-hasEndDate"/>
    </owl:ObjectProperty>
    


    <!-- http://purl.org/ica/ric#RiC-R-hadFunctionalRelationWith -->

    <owl:ObjectProperty rdf:about="http://purl.org/ica/ric#RiC-R-hadFunctionalRelationWith">
        <rdf:type rdf:resource="http://www.w3.org/2002/07/owl#SymmetricProperty"/>
        <rdfs:domain rdf:resource="http://purl.org/ica/ric#RiC-E4-Agent"/>
        <rdfs:range rdf:resource="http://purl.org/ica/ric#RiC-E4-Agent"/>
        <rdfs:comment xml:lang="en">Relations RiC-R253</rdfs:comment>
        <rdfs:label xml:lang="en">had functional relation with</rdfs:label>
        <rdfs:seeAlso rdf:resource="http://purl.org/ica/ric#RiC-R-hasFunctionalRelationWith"/>
    </owl:ObjectProperty>
    


    <!-- http://purl.org/ica/ric#RiC-R-hadHoldingLocation -->

    <owl:ObjectProperty rdf:about="http://purl.org/ica/ric#RiC-R-hadHoldingLocation">
        <owl:inverseOf rdf:resource="http://purl.org/ica/ric#RiC-R-wasHoldingLocationPlaceOf"/>
        <rdfs:domain>
            <owl:Class>
                <owl:unionOf rdf:parseType="Collection">
                    <rdf:Description rdf:about="http://purl.org/ica/ric#RiC-E1-Record"/>
                    <rdf:Description rdf:about="http://purl.org/ica/ric#RiC-E2-RecordComponent"/>
                    <rdf:Description rdf:about="http://purl.org/ica/ric#RiC-E3-RecordSet"/>
                </owl:unionOf>
            </owl:Class>
        </rdfs:domain>
        <rdfs:range rdf:resource="http://purl.org/ica/ric#RiC-E13-Place"/>
        <rdfs:comment xml:lang="en">Relations RiC-R65, RiC-R125, RiC-R195</rdfs:comment>
        <rdfs:label xml:lang="en">had holding location</rdfs:label>
        <rdfs:seeAlso rdf:resource="http://purl.org/ica/ric#RiC-R-hasHoldingLocation"/>
    </owl:ObjectProperty>
    


    <!-- http://purl.org/ica/ric#RiC-R-hadJurisdiction -->

    <owl:ObjectProperty rdf:about="http://purl.org/ica/ric#RiC-R-hadJurisdiction">
        <owl:inverseOf rdf:resource="http://purl.org/ica/ric#RiC-R-wasJurisdictionOf"/>
        <rdfs:domain rdf:resource="http://purl.org/ica/ric#RiC-E10-Mandate"/>
        <rdfs:range rdf:resource="http://purl.org/ica/ric#RiC-E13-Place"/>
        <rdfs:comment xml:lang="en">Relations RiC-R608</rdfs:comment>
        <rdfs:label xml:lang="en">had jurisdiction</rdfs:label>
        <rdfs:seeAlso rdf:resource="http://purl.org/ica/ric#RiC-R-hasJurisdiction"/>
    </owl:ObjectProperty>
    


    <!-- http://purl.org/ica/ric#RiC-R-hadMember -->

    <owl:ObjectProperty rdf:about="http://purl.org/ica/ric#RiC-R-hadMember">
        <owl:inverseOf rdf:resource="http://purl.org/ica/ric#RiC-R-wasMemberOf"/>
        <rdfs:domain>
            <owl:Class>
                <owl:unionOf rdf:parseType="Collection">
                    <rdf:Description rdf:about="http://purl.org/ica/ric#RiC-E3-RecordSet"/>
                    <rdf:Description rdf:about="http://purl.org/ica/ric#RiC-E4-Agent-Group"/>
                </owl:unionOf>
            </owl:Class>
        </rdfs:domain>
        <rdfs:range>
            <owl:Class>
                <owl:unionOf rdf:parseType="Collection">
                    <rdf:Description rdf:about="http://purl.org/ica/ric#RiC-E1-Record"/>
                    <rdf:Description rdf:about="http://purl.org/ica/ric#RiC-E3-RecordSet"/>
                    <rdf:Description rdf:about="http://purl.org/ica/ric#RiC-E4-Agent"/>
                </owl:unionOf>
            </owl:Class>
        </rdfs:range>
        <rdfs:comment xml:lang="en">Relations RiC-R134, RiC-R140, RiC-R254</rdfs:comment>
        <rdfs:label xml:lang="en">had member</rdfs:label>
        <rdfs:seeAlso rdf:resource="http://purl.org/ica/ric#RiC-R-hasMember"/>
    </owl:ObjectProperty>
    


    <!-- http://purl.org/ica/ric#RiC-R-hadPart -->

    <owl:ObjectProperty rdf:about="http://purl.org/ica/ric#RiC-R-hadPart">
        <owl:inverseOf rdf:resource="http://purl.org/ica/ric#RiC-R-wasPartOf"/>
        <rdfs:domain>
            <owl:Class>
                <owl:unionOf rdf:parseType="Collection">
                    <rdf:Description rdf:about="http://purl.org/ica/ric#RiC-E1-Record"/>
                    <rdf:Description rdf:about="http://purl.org/ica/ric#RiC-E4-Agent-Group"/>
                    <rdf:Description rdf:about="http://purl.org/ica/ric#RiC-E7-Function"/>
                    <rdf:Description rdf:about="http://purl.org/ica/ric#RiC-E9-Activity"/>
                </owl:unionOf>
            </owl:Class>
        </rdfs:domain>
        <rdfs:range>
            <owl:Class>
                <owl:unionOf rdf:parseType="Collection">
                    <rdf:Description rdf:about="http://purl.org/ica/ric#RiC-E2-RecordComponent"/>
                    <rdf:Description rdf:about="http://purl.org/ica/ric#RiC-E4-Agent-Group"/>
                    <rdf:Description rdf:about="http://purl.org/ica/ric#RiC-E7-Function"/>
                    <rdf:Description rdf:about="http://purl.org/ica/ric#RiC-E9-Activity"/>
                </owl:unionOf>
            </owl:Class>
        </rdfs:range>
        <rdfs:comment xml:lang="en">Relations RiC-R13, RiC-R255, RiC-R444, RiC-R535</rdfs:comment>
        <rdfs:label xml:lang="en">had part</rdfs:label>
        <rdfs:seeAlso rdf:resource="http://purl.org/ica/ric#RiC-R-hasPart"/>
    </owl:ObjectProperty>
    


    <!-- http://purl.org/ica/ric#RiC-R-hadRevisionDate -->

    <owl:ObjectProperty rdf:about="http://purl.org/ica/ric#RiC-R-hadRevisionDate">
        <owl:inverseOf rdf:resource="http://purl.org/ica/ric#RiC-R-wasRevisionDateOf"/>
        <rdfs:domain rdf:resource="http://purl.org/ica/ric#RiC-E10-Mandate"/>
        <rdfs:range rdf:resource="http://purl.org/ica/ric#RiC-E12-Date"/>
        <rdfs:comment xml:lang="en">Relations RiC-R602</rdfs:comment>
        <rdfs:label xml:lang="en">had revision date</rdfs:label>
    </owl:ObjectProperty>
    


    <!-- http://purl.org/ica/ric#RiC-R-hadRightsHeldBy -->

    <owl:ObjectProperty rdf:about="http://purl.org/ica/ric#RiC-R-hadRightsHeldBy">
        <owl:inverseOf rdf:resource="http://purl.org/ica/ric#RiC-R-wasRightsHolderOf"/>
        <rdfs:domain>
            <owl:Class>
                <owl:unionOf rdf:parseType="Collection">
                    <rdf:Description rdf:about="http://purl.org/ica/ric#RiC-E1-Record"/>
                    <rdf:Description rdf:about="http://purl.org/ica/ric#RiC-E2-RecordComponent"/>
                    <rdf:Description rdf:about="http://purl.org/ica/ric#RiC-E3-RecordSet"/>
                </owl:unionOf>
            </owl:Class>
        </rdfs:domain>
        <rdfs:range rdf:resource="http://purl.org/ica/ric#RiC-E4-Agent"/>
        <rdfs:comment xml:lang="en">Relations RiC-R21, RiC-R84, RiC-R148</rdfs:comment>
        <rdfs:label xml:lang="en">had rights held by</rdfs:label>
        <rdfs:seeAlso rdf:resource="http://purl.org/ica/ric#RiC-R-hasRightsHeldBy"/>
    </owl:ObjectProperty>
    


    <!-- http://purl.org/ica/ric#RiC-R-hadStartDate -->

    <owl:ObjectProperty rdf:about="http://purl.org/ica/ric#RiC-R-hadStartDate">
        <owl:inverseOf rdf:resource="http://purl.org/ica/ric#RiC-R-wasStartDateOf"/>
        <rdfs:domain>
            <owl:Class>
                <owl:unionOf rdf:parseType="Collection">
                    <rdf:Description rdf:about="http://purl.org/ica/ric#RiC-E10-Mandate"/>
                    <rdf:Description rdf:about="http://purl.org/ica/ric#RiC-E13-Place"/>
                    <rdf:Description rdf:about="http://purl.org/ica/ric#RiC-E4-Agent-Group"/>
                    <rdf:Description rdf:about="http://purl.org/ica/ric#RiC-E6-Position"/>
                    <rdf:Description rdf:about="http://purl.org/ica/ric#RiC-E7-Function"/>
                    <rdf:Description rdf:about="http://purl.org/ica/ric#RiC-E9-Activity"/>
                </owl:unionOf>
            </owl:Class>
        </rdfs:domain>
        <rdfs:range rdf:resource="http://purl.org/ica/ric#RiC-E12-Date"/>
        <rdfs:comment xml:lang="en">Relations RiC-R320, RiC-R414, RiC-R468, RiC-R552, RiC-R603, RiC-R753</rdfs:comment>
        <rdfs:label xml:lang="en">had start date</rdfs:label>
    </owl:ObjectProperty>
    


    <!-- http://purl.org/ica/ric#RiC-R-hasActiveDate -->

    <owl:ObjectProperty rdf:about="http://purl.org/ica/ric#RiC-R-hasActiveDate">
        <owl:inverseOf rdf:resource="http://purl.org/ica/ric#RiC-R-isActiveDateOf"/>
        <rdfs:domain>
            <owl:Class>
                <owl:unionOf rdf:parseType="Collection">
                    <rdf:Description rdf:about="http://purl.org/ica/ric#RiC-E10-Mandate"/>
                    <rdf:Description rdf:about="http://purl.org/ica/ric#RiC-E13-Place"/>
                    <rdf:Description rdf:about="http://purl.org/ica/ric#RiC-E4-Agent"/>
                    <rdf:Description rdf:about="http://purl.org/ica/ric#RiC-E7-Function"/>
                    <rdf:Description rdf:about="http://purl.org/ica/ric#RiC-E9-Activity"/>
                </owl:unionOf>
            </owl:Class>
        </rdfs:domain>
        <rdfs:range rdf:resource="http://purl.org/ica/ric#RiC-E12-Date"/>
        <rdfs:comment xml:lang="en">Relations RiC-R321, RiC-R469, RiC-R553, RiC-R604, RiC-R754</rdfs:comment>
        <rdfs:label xml:lang="en">has active date</rdfs:label>
        <rdfs:seeAlso rdf:resource="http://purl.org/ica/ric#RiC-R-hadActiveDate"/>
    </owl:ObjectProperty>
    


    <!-- http://purl.org/ica/ric#RiC-R-hasAssumedIdentity -->

    <owl:ObjectProperty rdf:about="http://purl.org/ica/ric#RiC-R-hasAssumedIdentity">
        <owl:inverseOf rdf:resource="http://purl.org/ica/ric#RiC-R-isAssumedIdentityOf"/>
        <rdfs:domain rdf:resource="http://purl.org/ica/ric#RiC-E4-Agent"/>
        <rdfs:range rdf:resource="http://purl.org/ica/ric#RiC-E4-Agent"/>
        <rdfs:comment xml:lang="en">Relations RiC-R256</rdfs:comment>
        <rdfs:label xml:lang="en">has assumed identity</rdfs:label>
    </owl:ObjectProperty>
    


    <!-- http://purl.org/ica/ric#RiC-R-hasCitizen -->

    <owl:ObjectProperty rdf:about="http://purl.org/ica/ric#RiC-R-hasCitizen">
        <owl:inverseOf rdf:resource="http://purl.org/ica/ric#RiC-R-isCitizenOf"/>
        <rdfs:domain rdf:resource="http://purl.org/ica/ric#RiC-E13-Place"/>
        <rdfs:range rdf:resource="http://purl.org/ica/ric#RiC-E4-Agent-Person"/>
        <rdfs:comment xml:lang="en">Relations RiC-R726</rdfs:comment>
        <rdfs:label xml:lang="en">has citizen</rdfs:label>
        <rdfs:seeAlso rdf:resource="http://purl.org/ica/ric#RiC-R-hadCitizen"/>
    </owl:ObjectProperty>
    


    <!-- http://purl.org/ica/ric#RiC-R-hasCopy -->

    <owl:ObjectProperty rdf:about="http://purl.org/ica/ric#RiC-R-hasCopy">
        <owl:inverseOf rdf:resource="http://purl.org/ica/ric#RiC-R-isCopyOf"/>
        <rdfs:domain rdf:resource="http://purl.org/ica/ric#RiC-E1-Record"/>
        <rdfs:range rdf:resource="http://purl.org/ica/ric#RiC-E1-Record"/>
        <rdfs:comment xml:lang="en">Relations RiC-R1</rdfs:comment>
        <rdfs:label xml:lang="en">has copy</rdfs:label>
    </owl:ObjectProperty>
    


    <!-- http://purl.org/ica/ric#RiC-R-hasCoverageDate -->

    <owl:ObjectProperty rdf:about="http://purl.org/ica/ric#RiC-R-hasCoverageDate">
        <owl:inverseOf rdf:resource="http://purl.org/ica/ric#RiC-R-isCoverageDateOf"/>
        <rdfs:domain rdf:resource="http://purl.org/ica/ric#RiC-E3-RecordSet"/>
        <rdfs:range rdf:resource="http://purl.org/ica/ric#RiC-E12-Date"/>
        <rdfs:comment xml:lang="en">Relations RiC-R192</rdfs:comment>
        <rdfs:label xml:lang="en">has coverage date</rdfs:label>
    </owl:ObjectProperty>
    


    <!-- http://purl.org/ica/ric#RiC-R-hasDocumentaryForm -->

    <owl:ObjectProperty rdf:about="http://purl.org/ica/ric#RiC-R-hasDocumentaryForm">
        <owl:inverseOf rdf:resource="http://purl.org/ica/ric#RiC-R-isDocumentaryFormOf"/>
        <rdfs:domain>
            <owl:Class>
                <owl:unionOf rdf:parseType="Collection">
                    <rdf:Description rdf:about="http://purl.org/ica/ric#RiC-E1-Record"/>
                    <rdf:Description rdf:about="http://purl.org/ica/ric#RiC-E2-RecordComponent"/>
                </owl:unionOf>
            </owl:Class>
        </rdfs:domain>
        <rdfs:range rdf:resource="http://purl.org/ica/ric#RiC-E11-DocumentaryForm"/>
        <rdfs:comment xml:lang="en">Relations RiC-R59, RiC-R119</rdfs:comment>
        <rdfs:label xml:lang="en">has documentary form</rdfs:label>
    </owl:ObjectProperty>
    


    <!-- http://purl.org/ica/ric#RiC-R-hasDraft -->

    <owl:ObjectProperty rdf:about="http://purl.org/ica/ric#RiC-R-hasDraft">
        <owl:inverseOf rdf:resource="http://purl.org/ica/ric#RiC-R-isDraftOf"/>
        <rdfs:domain rdf:resource="http://purl.org/ica/ric#RiC-E1-Record"/>
        <rdfs:range rdf:resource="http://purl.org/ica/ric#RiC-E1-Record"/>
        <rdfs:comment xml:lang="en">Relations RiC-R2</rdfs:comment>
        <rdfs:label xml:lang="en">has draft</rdfs:label>
    </owl:ObjectProperty>
    


    <!-- http://purl.org/ica/ric#RiC-R-hasEndDate -->

    <owl:ObjectProperty rdf:about="http://purl.org/ica/ric#RiC-R-hasEndDate">
        <owl:inverseOf rdf:resource="http://purl.org/ica/ric#RiC-R-isEndDateOf"/>
        <rdfs:domain>
            <owl:Class>
                <owl:unionOf rdf:parseType="Collection">
                    <rdf:Description rdf:about="http://purl.org/ica/ric#RiC-E10-Mandate"/>
                    <rdf:Description rdf:about="http://purl.org/ica/ric#RiC-E13-Place"/>
                    <rdf:Description rdf:about="http://purl.org/ica/ric#RiC-E4-Agent-Group"/>
                    <rdf:Description rdf:about="http://purl.org/ica/ric#RiC-E6-Position"/>
                    <rdf:Description rdf:about="http://purl.org/ica/ric#RiC-E7-Function"/>
                    <rdf:Description rdf:about="http://purl.org/ica/ric#RiC-E9-Activity"/>
                </owl:unionOf>
            </owl:Class>
        </rdfs:domain>
        <rdfs:range rdf:resource="http://purl.org/ica/ric#RiC-E12-Date"/>
        <rdfs:comment xml:lang="en">Relations RiC-R322, RiC-R415, RiC-R470, RiC-R554, RiC-R605, RiC-R755</rdfs:comment>
        <rdfs:label xml:lang="en">has end date</rdfs:label>
        <rdfs:seeAlso rdf:resource="http://purl.org/ica/ric#RiC-R-hadEndDate"/>
    </owl:ObjectProperty>
    


    <!-- http://purl.org/ica/ric#RiC-R-hasExample -->

    <owl:ObjectProperty rdf:about="http://purl.org/ica/ric#RiC-R-hasExample">
        <owl:inverseOf rdf:resource="http://purl.org/ica/ric#RiC-R-isExampleOf"/>
        <rdfs:domain rdf:resource="http://purl.org/ica/ric#RiC-E8-FunctionAbstract"/>
        <rdfs:range rdf:resource="http://purl.org/ica/ric#RiC-E7-Function"/>
        <rdfs:comment xml:lang="en">Relations RiC-R492</rdfs:comment>
        <rdfs:label xml:lang="en">has example</rdfs:label>
    </owl:ObjectProperty>
    


    <!-- http://purl.org/ica/ric#RiC-R-hasFunctionalRelationWith -->

    <owl:ObjectProperty rdf:about="http://purl.org/ica/ric#RiC-R-hasFunctionalRelationWith">
        <rdf:type rdf:resource="http://www.w3.org/2002/07/owl#SymmetricProperty"/>
        <rdfs:domain rdf:resource="http://purl.org/ica/ric#RiC-E4-Agent"/>
        <rdfs:range rdf:resource="http://purl.org/ica/ric#RiC-E4-Agent"/>
        <rdfs:comment xml:lang="en">Relations RiC-R257</rdfs:comment>
        <rdfs:label xml:lang="en">has functional relation with</rdfs:label>
        <rdfs:seeAlso rdf:resource="http://purl.org/ica/ric#RiC-R-hadFunctionalRelationWith"/>
    </owl:ObjectProperty>
    


    <!-- http://purl.org/ica/ric#RiC-R-hasHoldingLocation -->

    <owl:ObjectProperty rdf:about="http://purl.org/ica/ric#RiC-R-hasHoldingLocation">
        <owl:inverseOf rdf:resource="http://purl.org/ica/ric#RiC-R-isHoldingLocationPlaceOf"/>
        <rdfs:domain>
            <owl:Class>
                <owl:unionOf rdf:parseType="Collection">
                    <rdf:Description rdf:about="http://purl.org/ica/ric#RiC-E1-Record"/>
                    <rdf:Description rdf:about="http://purl.org/ica/ric#RiC-E2-RecordComponent"/>
                    <rdf:Description rdf:about="http://purl.org/ica/ric#RiC-E3-RecordSet"/>
                </owl:unionOf>
            </owl:Class>
        </rdfs:domain>
        <rdfs:range rdf:resource="http://purl.org/ica/ric#RiC-E13-Place"/>
        <rdfs:comment xml:lang="en">Relations RiC-R66, RiC-R126, RiC-R196</rdfs:comment>
        <rdfs:label xml:lang="en">has holding location</rdfs:label>
        <rdfs:seeAlso rdf:resource="http://purl.org/ica/ric#RiC-R-hadHoldingLocation"/>
    </owl:ObjectProperty>
    


    <!-- http://purl.org/ica/ric#RiC-R-hasJurisdiction -->

    <owl:ObjectProperty rdf:about="http://purl.org/ica/ric#RiC-R-hasJurisdiction">
        <owl:inverseOf rdf:resource="http://purl.org/ica/ric#RiC-R-isJurisdictionOf"/>
        <rdfs:domain rdf:resource="http://purl.org/ica/ric#RiC-E10-Mandate"/>
        <rdfs:range rdf:resource="http://purl.org/ica/ric#RiC-E13-Place"/>
        <rdfs:comment xml:lang="en">Relations RiC-R609</rdfs:comment>
        <rdfs:label xml:lang="en">has jurisdiction</rdfs:label>
        <rdfs:seeAlso rdf:resource="http://purl.org/ica/ric#RiC-R-hadJurisdiction"/>
    </owl:ObjectProperty>
    


    <!-- http://purl.org/ica/ric#RiC-R-hasMember -->

    <owl:ObjectProperty rdf:about="http://purl.org/ica/ric#RiC-R-hasMember">
        <owl:inverseOf rdf:resource="http://purl.org/ica/ric#RiC-R-isMemberOf"/>
        <rdfs:domain>
            <owl:Class>
                <owl:unionOf rdf:parseType="Collection">
                    <rdf:Description rdf:about="http://purl.org/ica/ric#RiC-E3-RecordSet"/>
                    <rdf:Description rdf:about="http://purl.org/ica/ric#RiC-E4-Agent-Group"/>
                </owl:unionOf>
            </owl:Class>
        </rdfs:domain>
        <rdfs:range>
            <owl:Class>
                <owl:unionOf rdf:parseType="Collection">
                    <rdf:Description rdf:about="http://purl.org/ica/ric#RiC-E1-Record"/>
                    <rdf:Description rdf:about="http://purl.org/ica/ric#RiC-E3-RecordSet"/>
                    <rdf:Description rdf:about="http://purl.org/ica/ric#RiC-E4-Agent"/>
                </owl:unionOf>
            </owl:Class>
        </rdfs:range>
        <rdfs:comment xml:lang="en">Relations RiC-R135, RiC-R141, RiC-R258</rdfs:comment>
        <rdfs:label xml:lang="en">has member</rdfs:label>
        <rdfs:seeAlso rdf:resource="http://purl.org/ica/ric#RiC-R-hadMember"/>
    </owl:ObjectProperty>
    


    <!-- http://purl.org/ica/ric#RiC-R-hasOriginal -->

    <owl:ObjectProperty rdf:about="http://purl.org/ica/ric#RiC-R-hasOriginal">
        <owl:inverseOf rdf:resource="http://purl.org/ica/ric#RiC-R-isOriginalOf"/>
        <rdfs:domain rdf:resource="http://purl.org/ica/ric#RiC-E1-Record"/>
        <rdfs:range rdf:resource="http://purl.org/ica/ric#RiC-E1-Record"/>
        <rdfs:comment xml:lang="en">Relations RiC-R3</rdfs:comment>
        <rdfs:label xml:lang="en">has original</rdfs:label>
    </owl:ObjectProperty>
    


    <!-- http://purl.org/ica/ric#RiC-R-hasPart -->

    <owl:ObjectProperty rdf:about="http://purl.org/ica/ric#RiC-R-hasPart">
        <owl:inverseOf rdf:resource="http://purl.org/ica/ric#RiC-R-isPartOf"/>
        <rdfs:domain>
            <owl:Class>
                <owl:unionOf rdf:parseType="Collection">
                    <rdf:Description rdf:about="http://purl.org/ica/ric#RiC-E1-Record"/>
                    <rdf:Description rdf:about="http://purl.org/ica/ric#RiC-E4-Agent-Group"/>
                    <rdf:Description rdf:about="http://purl.org/ica/ric#RiC-E7-Function"/>
                    <rdf:Description rdf:about="http://purl.org/ica/ric#RiC-E9-Activity"/>
                </owl:unionOf>
            </owl:Class>
        </rdfs:domain>
        <rdfs:range>
            <owl:Class>
                <owl:unionOf rdf:parseType="Collection">
                    <rdf:Description rdf:about="http://purl.org/ica/ric#RiC-E2-RecordComponent"/>
                    <rdf:Description rdf:about="http://purl.org/ica/ric#RiC-E4-Agent-Group"/>
                    <rdf:Description rdf:about="http://purl.org/ica/ric#RiC-E7-Function"/>
                    <rdf:Description rdf:about="http://purl.org/ica/ric#RiC-E9-Activity"/>
                </owl:unionOf>
            </owl:Class>
        </rdfs:range>
        <rdfs:comment xml:lang="en">Relations RiC-R14, RiC-R259, RiC-R445, RiC-R536</rdfs:comment>
        <rdfs:label xml:lang="en">has part</rdfs:label>
        <rdfs:seeAlso rdf:resource="http://purl.org/ica/ric#RiC-R-hadPart"/>
    </owl:ObjectProperty>
    


    <!-- http://purl.org/ica/ric#RiC-R-hasRightsHeldBy -->

    <owl:ObjectProperty rdf:about="http://purl.org/ica/ric#RiC-R-hasRightsHeldBy">
        <owl:inverseOf rdf:resource="http://purl.org/ica/ric#RiC-R-isRightsHolderOf"/>
        <rdfs:domain>
            <owl:Class>
                <owl:unionOf rdf:parseType="Collection">
                    <rdf:Description rdf:about="http://purl.org/ica/ric#RiC-E1-Record"/>
                    <rdf:Description rdf:about="http://purl.org/ica/ric#RiC-E2-RecordComponent"/>
                    <rdf:Description rdf:about="http://purl.org/ica/ric#RiC-E3-RecordSet"/>
                </owl:unionOf>
            </owl:Class>
        </rdfs:domain>
        <rdfs:range rdf:resource="http://purl.org/ica/ric#RiC-E4-Agent"/>
        <rdfs:comment xml:lang="en">Relations RiC-R22, RiC-R85, RiC-R149</rdfs:comment>
        <rdfs:label xml:lang="en">has rights held by</rdfs:label>
        <rdfs:seeAlso rdf:resource="http://purl.org/ica/ric#RiC-R-hadRightsHeldBy"/>
    </owl:ObjectProperty>
    


    <!-- http://purl.org/ica/ric#RiC-R-hasSubject -->

    <owl:ObjectProperty rdf:about="http://purl.org/ica/ric#RiC-R-hasSubject">
        <owl:inverseOf rdf:resource="http://purl.org/ica/ric#RiC-R-isSubjectOf"/>
        <rdfs:domain>
            <owl:Class>
                <owl:unionOf rdf:parseType="Collection">
                    <rdf:Description rdf:about="http://purl.org/ica/ric#RiC-E1-Record"/>
                    <rdf:Description rdf:about="http://purl.org/ica/ric#RiC-E2-RecordComponent"/>
                    <rdf:Description rdf:about="http://purl.org/ica/ric#RiC-E3-RecordSet"/>
                </owl:unionOf>
            </owl:Class>
        </rdfs:domain>
        <rdfs:range>
            <owl:Class>
                <owl:unionOf rdf:parseType="Collection">
                    <rdf:Description rdf:about="http://purl.org/ica/ric#RiC-E1-Record"/>
                    <rdf:Description rdf:about="http://purl.org/ica/ric#RiC-E10-Mandate"/>
                    <rdf:Description rdf:about="http://purl.org/ica/ric#RiC-E13-Place"/>
                    <rdf:Description rdf:about="http://purl.org/ica/ric#RiC-E14-ConceptThing"/>
                    <rdf:Description rdf:about="http://purl.org/ica/ric#RiC-E4-Agent"/>
                    <rdf:Description rdf:about="http://purl.org/ica/ric#RiC-E5-Occupation"/>
                    <rdf:Description rdf:about="http://purl.org/ica/ric#RiC-E6-Position"/>
                    <rdf:Description rdf:about="http://purl.org/ica/ric#RiC-E7-Function"/>
                    <rdf:Description rdf:about="http://purl.org/ica/ric#RiC-E8-FunctionAbstract"/>
                    <rdf:Description rdf:about="http://purl.org/ica/ric#RiC-E9-Activity"/>
                </owl:unionOf>
            </owl:Class>
        </rdfs:range>
        <rdfs:comment xml:lang="en">Relations RiC-R4, RiC-R23, RiC-R36, RiC-R40, RiC-R44, RiC-R48, RiC-R51, RiC-R55, RiC-R67, RiC-R71, RiC-R86, RiC-R97, RiC-R101, RiC-R105, RiC-R109, RiC-R112, RiC-R116, RiC-R127, RiC-R131, RiC-R150, RiC-R166, RiC-R170, RiC-R174, RiC-R178, RiC-R181, RiC-R185, RiC-R197, RiC-R201</rdfs:comment>
        <rdfs:label xml:lang="en">has subject</rdfs:label>
    </owl:ObjectProperty>
    


    <!-- http://purl.org/ica/ric#RiC-R-isActiveDateOf -->

    <owl:ObjectProperty rdf:about="http://purl.org/ica/ric#RiC-R-isActiveDateOf">
        <rdfs:domain rdf:resource="http://purl.org/ica/ric#RiC-E12-Date"/>
        <rdfs:range>
            <owl:Class>
                <owl:unionOf rdf:parseType="Collection">
                    <rdf:Description rdf:about="http://purl.org/ica/ric#RiC-E10-Mandate"/>
                    <rdf:Description rdf:about="http://purl.org/ica/ric#RiC-E13-Place"/>
                    <rdf:Description rdf:about="http://purl.org/ica/ric#RiC-E4-Agent"/>
                    <rdf:Description rdf:about="http://purl.org/ica/ric#RiC-E7-Function"/>
                    <rdf:Description rdf:about="http://purl.org/ica/ric#RiC-E9-Activity"/>
                </owl:unionOf>
            </owl:Class>
        </rdfs:range>
        <rdfs:comment xml:lang="en">Relations RiC-R654, RiC-R670, RiC-R679, RiC-R686, RiC-R698</rdfs:comment>
        <rdfs:label xml:lang="en">is active date of</rdfs:label>
        <rdfs:seeAlso rdf:resource="http://purl.org/ica/ric#RiC-R-wasActiveDateOf"/>
    </owl:ObjectProperty>
    


    <!-- http://purl.org/ica/ric#RiC-R-isAssociatedWith -->

    <owl:ObjectProperty rdf:about="http://purl.org/ica/ric#RiC-R-isAssociatedWith">
        <rdf:type rdf:resource="http://www.w3.org/2002/07/owl#SymmetricProperty"/>
        <rdfs:domain>
            <owl:Class>
                <owl:unionOf rdf:parseType="Collection">
                    <rdf:Description rdf:about="http://purl.org/ica/ric#RiC-E1-Record"/>
                    <rdf:Description rdf:about="http://purl.org/ica/ric#RiC-E10-Mandate"/>
                    <rdf:Description rdf:about="http://purl.org/ica/ric#RiC-E11-DocumentaryForm"/>
                    <rdf:Description rdf:about="http://purl.org/ica/ric#RiC-E12-Date"/>
                    <rdf:Description rdf:about="http://purl.org/ica/ric#RiC-E13-Place"/>
                    <rdf:Description rdf:about="http://purl.org/ica/ric#RiC-E14-ConceptThing"/>
                    <rdf:Description rdf:about="http://purl.org/ica/ric#RiC-E2-RecordComponent"/>
                    <rdf:Description rdf:about="http://purl.org/ica/ric#RiC-E3-RecordSet"/>
                    <rdf:Description rdf:about="http://purl.org/ica/ric#RiC-E4-Agent"/>
                    <rdf:Description rdf:about="http://purl.org/ica/ric#RiC-E5-Occupation"/>
                    <rdf:Description rdf:about="http://purl.org/ica/ric#RiC-E6-Position"/>
                    <rdf:Description rdf:about="http://purl.org/ica/ric#RiC-E7-Function"/>
                    <rdf:Description rdf:about="http://purl.org/ica/ric#RiC-E8-FunctionAbstract"/>
                    <rdf:Description rdf:about="http://purl.org/ica/ric#RiC-E9-Activity"/>
                </owl:unionOf>
            </owl:Class>
        </rdfs:domain>
        <rdfs:range>
            <owl:Class>
                <owl:unionOf rdf:parseType="Collection">
                    <rdf:Description rdf:about="http://purl.org/ica/ric#RiC-E1-Record"/>
                    <rdf:Description rdf:about="http://purl.org/ica/ric#RiC-E10-Mandate"/>
                    <rdf:Description rdf:about="http://purl.org/ica/ric#RiC-E11-DocumentaryForm"/>
                    <rdf:Description rdf:about="http://purl.org/ica/ric#RiC-E12-Date"/>
                    <rdf:Description rdf:about="http://purl.org/ica/ric#RiC-E13-Place"/>
                    <rdf:Description rdf:about="http://purl.org/ica/ric#RiC-E14-ConceptThing"/>
                    <rdf:Description rdf:about="http://purl.org/ica/ric#RiC-E2-RecordComponent"/>
                    <rdf:Description rdf:about="http://purl.org/ica/ric#RiC-E3-RecordSet"/>
                    <rdf:Description rdf:about="http://purl.org/ica/ric#RiC-E4-Agent"/>
                    <rdf:Description rdf:about="http://purl.org/ica/ric#RiC-E5-Occupation"/>
                    <rdf:Description rdf:about="http://purl.org/ica/ric#RiC-E6-Position"/>
                    <rdf:Description rdf:about="http://purl.org/ica/ric#RiC-E7-Function"/>
                    <rdf:Description rdf:about="http://purl.org/ica/ric#RiC-E8-FunctionAbstract"/>
                    <rdf:Description rdf:about="http://purl.org/ica/ric#RiC-E9-Activity"/>
                </owl:unionOf>
            </owl:Class>
        </rdfs:range>
        <rdfs:comment xml:lang="en">Relations RiC-R5, RiC-R15, RiC-R17, RiC-R24, RiC-R37, RiC-R41, RiC-R45, RiC-R49, RiC-R52, RiC-R56, RiC-R60, RiC-R63, RiC-R68, RiC-R72, RiC-R74, RiC-R78, RiC-R82, RiC-R87, RiC-R98, RiC-R102, RiC-R106, RiC-R110, RiC-R113, RiC-R117, RiC-R120, RiC-R123, RiC-R128, RiC-R132, RiC-R136, RiC-R138, RiC-R142, RiC-R151, RiC-R167, RiC-R171, RiC-R175, RiC-R179, RiC-R182, RiC-R186, RiC-R189, RiC-R193, RiC-R198, RiC-R202, RiC-R207, RiC-R222, RiC-R237, RiC-R260, RiC-R292, RiC-R297, RiC-R303, RiC-R305, RiC-R307, RiC-R311, RiC-R314, RiC-R323, RiC-R327, RiC-R333, RiC-R335, RiC-R339, RiC-R343, RiC-R347, RiC-R351, RiC-R355, RiC-R359, RiC-R361, RiC-R363, RiC-R365, RiC-R367, RiC-R369, RiC-R371, RiC-R373, RiC-R375, RiC-R379, RiC-R383, RiC-R387, RiC-R392, RiC-R396, RiC-R400, RiC-R402, RiC-R404, RiC-R406, RiC-R411, RiC-R416, RiC-R418, RiC-R422, RiC-R424, RiC-R428, RiC-R432, RiC-R436, RiC-R440, RiC-R442, RiC-R446, RiC-R452, RiC-R455, RiC-R459, RiC-R464, RiC-R471, RiC-R473, RiC-R475, RiC-R477, RiC-R480, RiC-R483, RiC-R486, RiC-R488, RiC-R490, RiC-R493, RiC-R495, RiC-R497, RiC-R499, RiC-R501, RiC-R503, RiC-R505, RiC-R507, RiC-R509, RiC-R513, RiC-R517, RiC-R521, RiC-R525, RiC-R527, RiC-R529, RiC-R533, RiC-R537, RiC-R543, RiC-R548, RiC-R555, RiC-R557, RiC-R559, RiC-R561, RiC-R565, RiC-R568, RiC-R573, RiC-R575, RiC-R579, RiC-R584, RiC-R587, RiC-R591, RiC-R594, RiC-R598, RiC-R606, RiC-R610, RiC-R612, RiC-R614, RiC-R617, RiC-R620, RiC-R622, RiC-R624, RiC-R626, RiC-R628, RiC-R630, RiC-R632, RiC-R634, RiC-R636, RiC-R638, RiC-R640, RiC-R642, RiC-R644, RiC-R647, RiC-R650, RiC-R655, RiC-R663, RiC-R665, RiC-R671, RiC-R677, RiC-R680, RiC-R687, RiC-R694, RiC-R696, RiC-R699, RiC-R705, RiC-R707, RiC-R713, RiC-R719, RiC-R727, RiC-R733, RiC-R735, RiC-R739, RiC-R741, RiC-R743, RiC-R745, RiC-R749, RiC-R756, RiC-R758, RiC-R760, RiC-R762, RiC-R765, RiC-R768, RiC-R771, RiC-R773, RiC-R775, RiC-R777, RiC-R779, RiC-R781, RiC-R783, RiC-R785, RiC-R787, RiC-R789, RiC-R791</rdfs:comment>
        <rdfs:label xml:lang="en">is associated with</rdfs:label>
        <rdfs:seeAlso rdf:resource="http://purl.org/ica/ric#RiC-R-wasAssociatedWith"/>
    </owl:ObjectProperty>
    


    <!-- http://purl.org/ica/ric#RiC-R-isAssumedIdentityOf -->

    <owl:ObjectProperty rdf:about="http://purl.org/ica/ric#RiC-R-isAssumedIdentityOf">
        <rdfs:domain rdf:resource="http://purl.org/ica/ric#RiC-E4-Agent"/>
        <rdfs:range rdf:resource="http://purl.org/ica/ric#RiC-E4-Agent"/>
        <rdfs:comment xml:lang="en">Relations RiC-R261</rdfs:comment>
        <rdfs:label xml:lang="en">is assumed identity of</rdfs:label>
    </owl:ObjectProperty>
    


    <!-- http://purl.org/ica/ric#RiC-R-isChildOf -->

    <owl:ObjectProperty rdf:about="http://purl.org/ica/ric#RiC-R-isChildOf">
        <owl:inverseOf rdf:resource="http://purl.org/ica/ric#RiC-R-isParentOf"/>
        <rdfs:domain rdf:resource="http://purl.org/ica/ric#RiC-E4-Agent-Person"/>
        <rdfs:range rdf:resource="http://purl.org/ica/ric#RiC-E4-Agent-Person"/>
        <rdfs:comment xml:lang="en">Relations RiC-R262</rdfs:comment>
        <rdfs:label xml:lang="en">is child of</rdfs:label>
        <rdfs:seeAlso rdf:resource="http://purl.org/ica/ric#RiC-R-wasChildOf"/>
    </owl:ObjectProperty>
    


    <!-- http://purl.org/ica/ric#RiC-R-isCitizenOf -->

    <owl:ObjectProperty rdf:about="http://purl.org/ica/ric#RiC-R-isCitizenOf">
        <rdfs:domain rdf:resource="http://purl.org/ica/ric#RiC-E4-Agent-Person"/>
        <rdfs:range rdf:resource="http://purl.org/ica/ric#RiC-E13-Place"/>
        <rdfs:comment xml:lang="en">Relations RiC-R328</rdfs:comment>
        <rdfs:label xml:lang="en">is citizen of</rdfs:label>
        <rdfs:seeAlso rdf:resource="http://purl.org/ica/ric#RiC-R-wasCitizenOf"/>
    </owl:ObjectProperty>
    


    <!-- http://purl.org/ica/ric#RiC-R-isControlledBy -->

    <owl:ObjectProperty rdf:about="http://purl.org/ica/ric#RiC-R-isControlledBy">
        <rdfs:domain rdf:resource="http://purl.org/ica/ric#RiC-E4-Agent"/>
        <rdfs:range rdf:resource="http://purl.org/ica/ric#RiC-E4-Agent"/>
        <rdfs:comment xml:lang="en">Relations RiC-R263</rdfs:comment>
        <rdfs:label xml:lang="en">is controlled by</rdfs:label>
        <rdfs:seeAlso rdf:resource="http://purl.org/ica/ric#RiC-R-wasControlledBy"/>
    </owl:ObjectProperty>
    


    <!-- http://purl.org/ica/ric#RiC-R-isCopyOf -->

    <owl:ObjectProperty rdf:about="http://purl.org/ica/ric#RiC-R-isCopyOf">
        <rdfs:domain rdf:resource="http://purl.org/ica/ric#RiC-E1-Record"/>
        <rdfs:range rdf:resource="http://purl.org/ica/ric#RiC-E1-Record"/>
        <rdfs:comment xml:lang="en">Relations RiC-R6</rdfs:comment>
        <rdfs:label xml:lang="en">is copy of</rdfs:label>
    </owl:ObjectProperty>
    


    <!-- http://purl.org/ica/ric#RiC-R-isCoverageDateOf -->

    <owl:ObjectProperty rdf:about="http://purl.org/ica/ric#RiC-R-isCoverageDateOf">
        <rdfs:domain rdf:resource="http://purl.org/ica/ric#RiC-E12-Date"/>
        <rdfs:range rdf:resource="http://purl.org/ica/ric#RiC-E3-RecordSet"/>
        <rdfs:comment xml:lang="en">Relations RiC-R651</rdfs:comment>
        <rdfs:label xml:lang="en">is coverage date of</rdfs:label>
    </owl:ObjectProperty>
    


    <!-- http://purl.org/ica/ric#RiC-R-isDefinedBy -->

    <owl:ObjectProperty rdf:about="http://purl.org/ica/ric#RiC-R-isDefinedBy">
        <rdfs:domain>
            <owl:Class>
                <owl:unionOf rdf:parseType="Collection">
                    <rdf:Description rdf:about="http://purl.org/ica/ric#RiC-E6-Position"/>
                    <rdf:Description rdf:about="http://purl.org/ica/ric#RiC-E7-Function"/>
                    <rdf:Description rdf:about="http://purl.org/ica/ric#RiC-E9-Activity"/>
                </owl:unionOf>
            </owl:Class>
        </rdfs:domain>
        <rdfs:range rdf:resource="http://purl.org/ica/ric#RiC-E10-Mandate"/>
        <rdfs:comment xml:lang="en">Relations RiC-R407, RiC-R460, RiC-R544</rdfs:comment>
        <rdfs:label xml:lang="en">is defined by</rdfs:label>
        <rdfs:seeAlso rdf:resource="http://purl.org/ica/ric#RiC-R-wasDefinedBy"/>
    </owl:ObjectProperty>
    


    <!-- http://purl.org/ica/ric#RiC-R-isDirectedBy -->

    <owl:ObjectProperty rdf:about="http://purl.org/ica/ric#RiC-R-isDirectedBy">
        <owl:inverseOf rdf:resource="http://purl.org/ica/ric#RiC-R-isDirectorOf"/>
        <rdfs:range rdf:resource="http://purl.org/ica/ric#RiC-E4-Agent-Person"/>
        <rdfs:comment xml:lang="en">Relations RiC-R264</rdfs:comment>
        <rdfs:label xml:lang="en">is directed by</rdfs:label>
        <rdfs:seeAlso rdf:resource="http://purl.org/ica/ric#RiC-R-wasDirectedBy"/>
    </owl:ObjectProperty>
    


    <!-- http://purl.org/ica/ric#RiC-R-isDirectorOf -->

    <owl:ObjectProperty rdf:about="http://purl.org/ica/ric#RiC-R-isDirectorOf">
        <rdfs:domain rdf:resource="http://purl.org/ica/ric#RiC-E4-Agent-Person"/>
        <rdfs:comment xml:lang="en">Relations RiC-R265</rdfs:comment>
        <rdfs:label xml:lang="en">is director of</rdfs:label>
        <rdfs:seeAlso rdf:resource="http://purl.org/ica/ric#RiC-R-wasDirectorOf"/>
    </owl:ObjectProperty>
    


    <!-- http://purl.org/ica/ric#RiC-R-isDocumentaryFormOf -->

    <owl:ObjectProperty rdf:about="http://purl.org/ica/ric#RiC-R-isDocumentaryFormOf">
        <rdfs:domain rdf:resource="http://purl.org/ica/ric#RiC-E11-DocumentaryForm"/>
        <rdfs:range>
            <owl:Class>
                <owl:unionOf rdf:parseType="Collection">
                    <rdf:Description rdf:about="http://purl.org/ica/ric#RiC-E1-Record"/>
                    <rdf:Description rdf:about="http://purl.org/ica/ric#RiC-E2-RecordComponent"/>
                </owl:unionOf>
            </owl:Class>
        </rdfs:range>
        <rdfs:comment xml:lang="en">Relations RiC-R615, RiC-R618</rdfs:comment>
        <rdfs:label xml:lang="en">is documentary form of</rdfs:label>
    </owl:ObjectProperty>
    


    <!-- http://purl.org/ica/ric#RiC-R-isDraftOf -->

    <owl:ObjectProperty rdf:about="http://purl.org/ica/ric#RiC-R-isDraftOf">
        <rdfs:domain rdf:resource="http://purl.org/ica/ric#RiC-E1-Record"/>
        <rdfs:range rdf:resource="http://purl.org/ica/ric#RiC-E1-Record"/>
        <rdfs:comment xml:lang="en">Relations RiC-R7</rdfs:comment>
        <rdfs:label xml:lang="en">is draft of</rdfs:label>
    </owl:ObjectProperty>
    


    <!-- http://purl.org/ica/ric#RiC-R-isEndDateOf -->

    <owl:ObjectProperty rdf:about="http://purl.org/ica/ric#RiC-R-isEndDateOf">
        <rdfs:domain rdf:resource="http://purl.org/ica/ric#RiC-E12-Date"/>
        <rdfs:range>
            <owl:Class>
                <owl:unionOf rdf:parseType="Collection">
                    <rdf:Description rdf:about="http://purl.org/ica/ric#RiC-E10-Mandate"/>
                    <rdf:Description rdf:about="http://purl.org/ica/ric#RiC-E13-Place"/>
                    <rdf:Description rdf:about="http://purl.org/ica/ric#RiC-E4-Agent-Group"/>
                    <rdf:Description rdf:about="http://purl.org/ica/ric#RiC-E6-Position"/>
                    <rdf:Description rdf:about="http://purl.org/ica/ric#RiC-E7-Function"/>
                    <rdf:Description rdf:about="http://purl.org/ica/ric#RiC-E9-Activity"/>
                </owl:unionOf>
            </owl:Class>
        </rdfs:range>
        <rdfs:comment xml:lang="en">Relations RiC-R656, RiC-R666, RiC-R672, RiC-R681, RiC-R688, RiC-R700</rdfs:comment>
        <rdfs:label xml:lang="en">is end date of</rdfs:label>
        <rdfs:seeAlso rdf:resource="http://purl.org/ica/ric#RiC-R-wasEndDateOf"/>
    </owl:ObjectProperty>
    


    <!-- http://purl.org/ica/ric#RiC-R-isEvidenceOf -->

    <owl:ObjectProperty rdf:about="http://purl.org/ica/ric#RiC-R-isEvidenceOf">
        <owl:inverseOf rdf:resource="http://purl.org/ica/ric#RiC-R-isEvidencedBy"/>
        <rdfs:domain>
            <owl:Class>
                <owl:unionOf rdf:parseType="Collection">
                    <rdf:Description rdf:about="http://purl.org/ica/ric#RiC-E1-Record"/>
                    <rdf:Description rdf:about="http://purl.org/ica/ric#RiC-E2-RecordComponent"/>
                    <rdf:Description rdf:about="http://purl.org/ica/ric#RiC-E3-RecordSet"/>
                </owl:unionOf>
            </owl:Class>
        </rdfs:domain>
        <rdfs:range>
            <owl:Class>
                <owl:unionOf rdf:parseType="Collection">
                    <rdf:Description rdf:about="http://purl.org/ica/ric#RiC-E10-Mandate"/>
                    <rdf:Description rdf:about="http://purl.org/ica/ric#RiC-E7-Function"/>
                </owl:unionOf>
            </owl:Class>
        </rdfs:range>
        <rdfs:comment xml:lang="en">Relations RiC-R46, RiC-R57, RiC-R107, RiC-R176, RiC-R187</rdfs:comment>
        <rdfs:label xml:lang="en">is evidence of</rdfs:label>
    </owl:ObjectProperty>
    


    <!-- http://purl.org/ica/ric#RiC-R-isEvidencedBy -->

    <owl:ObjectProperty rdf:about="http://purl.org/ica/ric#RiC-R-isEvidencedBy">
        <rdfs:domain>
            <owl:Class>
                <owl:unionOf rdf:parseType="Collection">
                    <rdf:Description rdf:about="http://purl.org/ica/ric#RiC-E10-Mandate"/>
                    <rdf:Description rdf:about="http://purl.org/ica/ric#RiC-E7-Function"/>
                </owl:unionOf>
            </owl:Class>
        </rdfs:domain>
        <rdfs:range>
            <owl:Class>
                <owl:unionOf rdf:parseType="Collection">
                    <rdf:Description rdf:about="http://purl.org/ica/ric#RiC-E1-Record"/>
                    <rdf:Description rdf:about="http://purl.org/ica/ric#RiC-E2-RecordComponent"/>
                    <rdf:Description rdf:about="http://purl.org/ica/ric#RiC-E3-RecordSet"/>
                </owl:unionOf>
            </owl:Class>
        </rdfs:range>
        <rdfs:comment xml:lang="en">Relations RiC-R425, RiC-R429, RiC-R433, RiC-R562, RiC-R569</rdfs:comment>
        <rdfs:label xml:lang="en">is evidenced by</rdfs:label>
    </owl:ObjectProperty>
    


    <!-- http://purl.org/ica/ric#RiC-R-isExampleOf -->

    <owl:ObjectProperty rdf:about="http://purl.org/ica/ric#RiC-R-isExampleOf">
        <rdfs:domain rdf:resource="http://purl.org/ica/ric#RiC-E7-Function"/>
        <rdfs:range rdf:resource="http://purl.org/ica/ric#RiC-E8-FunctionAbstract"/>
        <rdfs:comment xml:lang="en">Relations RiC-R453</rdfs:comment>
        <rdfs:label xml:lang="en">is example of</rdfs:label>
    </owl:ObjectProperty>
    


    <!-- http://purl.org/ica/ric#RiC-R-isFulfilledBy -->

    <owl:ObjectProperty rdf:about="http://purl.org/ica/ric#RiC-R-isFulfilledBy">
        <rdfs:domain rdf:resource="http://purl.org/ica/ric#RiC-E7-Function"/>
        <rdfs:range rdf:resource="http://purl.org/ica/ric#RiC-E4-Agent"/>
        <rdfs:comment xml:lang="en">Relations RiC-R437</rdfs:comment>
        <rdfs:label xml:lang="en">is fulfilled by</rdfs:label>
        <rdfs:seeAlso rdf:resource="http://purl.org/ica/ric#RiC-R-wasFulfilledBy"/>
    </owl:ObjectProperty>
    


    <!-- http://purl.org/ica/ric#RiC-R-isFulfilledByPerformanceOf -->

    <owl:ObjectProperty rdf:about="http://purl.org/ica/ric#RiC-R-isFulfilledByPerformanceOf">
        <owl:inverseOf rdf:resource="http://purl.org/ica/ric#RiC-R-isPerformedToFulfil"/>
        <rdfs:domain rdf:resource="http://purl.org/ica/ric#RiC-E7-Function"/>
        <rdfs:range rdf:resource="http://purl.org/ica/ric#RiC-E9-Activity"/>
        <rdfs:comment xml:lang="en">Relations RiC-R456</rdfs:comment>
        <rdfs:label xml:lang="en">is fulfilled by performance of</rdfs:label>
        <rdfs:seeAlso rdf:resource="http://purl.org/ica/ric#RiC-R-wasFulfilledByPerformanceOf"/>
    </owl:ObjectProperty>
    


    <!-- http://purl.org/ica/ric#RiC-R-isHeldBy -->

    <owl:ObjectProperty rdf:about="http://purl.org/ica/ric#RiC-R-isHeldBy">
        <owl:inverseOf rdf:resource="http://purl.org/ica/ric#RiC-R-isHolderOf"/>
        <rdfs:domain>
            <owl:Class>
                <owl:unionOf rdf:parseType="Collection">
                    <rdf:Description rdf:about="http://purl.org/ica/ric#RiC-E1-Record"/>
                    <rdf:Description rdf:about="http://purl.org/ica/ric#RiC-E2-RecordComponent"/>
                    <rdf:Description rdf:about="http://purl.org/ica/ric#RiC-E3-RecordSet"/>
                </owl:unionOf>
            </owl:Class>
        </rdfs:domain>
        <rdfs:range rdf:resource="http://purl.org/ica/ric#RiC-E4-Agent"/>
        <rdfs:comment xml:lang="en">Relations RiC-R25, RiC-R88, RiC-R152</rdfs:comment>
        <rdfs:label xml:lang="en">is held by</rdfs:label>
        <rdfs:seeAlso rdf:resource="http://purl.org/ica/ric#RiC-R-wasHeldBy"/>
    </owl:ObjectProperty>
    


    <!-- http://purl.org/ica/ric#RiC-R-isHolderOf -->

    <owl:ObjectProperty rdf:about="http://purl.org/ica/ric#RiC-R-isHolderOf">
        <rdfs:domain rdf:resource="http://purl.org/ica/ric#RiC-E4-Agent"/>
        <rdfs:range>
            <owl:Class>
                <owl:unionOf rdf:parseType="Collection">
                    <rdf:Description rdf:about="http://purl.org/ica/ric#RiC-E1-Record"/>
                    <rdf:Description rdf:about="http://purl.org/ica/ric#RiC-E2-RecordComponent"/>
                    <rdf:Description rdf:about="http://purl.org/ica/ric#RiC-E3-RecordSet"/>
                </owl:unionOf>
            </owl:Class>
        </rdfs:range>
        <rdfs:comment xml:lang="en">Relations RiC-R208, RiC-R223, RiC-R238</rdfs:comment>
        <rdfs:label xml:lang="en">is holder of</rdfs:label>
        <rdfs:seeAlso rdf:resource="http://purl.org/ica/ric#RiC-R-wasHolderOf"/>
    </owl:ObjectProperty>
    


    <!-- http://purl.org/ica/ric#RiC-R-isHoldingLocationPlaceOf -->

    <owl:ObjectProperty rdf:about="http://purl.org/ica/ric#RiC-R-isHoldingLocationPlaceOf">
        <rdfs:domain rdf:resource="http://purl.org/ica/ric#RiC-E13-Place"/>
        <rdfs:range>
            <owl:Class>
                <owl:unionOf rdf:parseType="Collection">
                    <rdf:Description rdf:about="http://purl.org/ica/ric#RiC-E1-Record"/>
                    <rdf:Description rdf:about="http://purl.org/ica/ric#RiC-E2-RecordComponent"/>
                    <rdf:Description rdf:about="http://purl.org/ica/ric#RiC-E3-RecordSet"/>
                </owl:unionOf>
            </owl:Class>
        </rdfs:range>
        <rdfs:comment xml:lang="en">Relations RiC-R708, RiC-R714, RiC-R720</rdfs:comment>
        <rdfs:label xml:lang="en">is holding location of / is holding place of</rdfs:label>
        <rdfs:seeAlso rdf:resource="http://purl.org/ica/ric#RiC-R-wasHoldingLocationOf"/>
    </owl:ObjectProperty>
    


    <!-- http://purl.org/ica/ric#RiC-R-isJurisdictionOf -->

    <owl:ObjectProperty rdf:about="http://purl.org/ica/ric#RiC-R-isJurisdictionOf">
        <rdfs:domain rdf:resource="http://purl.org/ica/ric#RiC-E13-Place"/>
        <rdfs:range rdf:resource="http://purl.org/ica/ric#RiC-E10-Mandate"/>
        <rdfs:comment xml:lang="en">Relations RiC-R746</rdfs:comment>
        <rdfs:label xml:lang="en">is jurisdiction of</rdfs:label>
        <rdfs:seeAlso rdf:resource="http://purl.org/ica/ric#RiC-R-wasJurisdictionOf"/>
    </owl:ObjectProperty>
    


    <!-- http://purl.org/ica/ric#RiC-R-isLocatedAtIn -->

    <owl:ObjectProperty rdf:about="http://purl.org/ica/ric#RiC-R-isLocatedAtIn">
        <owl:inverseOf rdf:resource="http://purl.org/ica/ric#RiC-R-isLocationOf"/>
        <rdfs:domain>
            <owl:Class>
                <owl:unionOf rdf:parseType="Collection">
                    <rdf:Description rdf:about="http://purl.org/ica/ric#RiC-E4-Agent"/>
                    <rdf:Description rdf:about="http://purl.org/ica/ric#RiC-E6-Position"/>
                </owl:unionOf>
            </owl:Class>
        </rdfs:domain>
        <rdfs:range rdf:resource="http://purl.org/ica/ric#RiC-E13-Place"/>
        <rdfs:comment xml:lang="en">Relations RiC-R329, RiC-R419</rdfs:comment>
        <rdfs:label xml:lang="en">is located at / is located in</rdfs:label>
        <rdfs:seeAlso rdf:resource="http://purl.org/ica/ric#RiC-R-wasLocatedAt-wasLocatedIn"/>
    </owl:ObjectProperty>
    


    <!-- http://purl.org/ica/ric#RiC-R-isLocationOf -->

    <owl:ObjectProperty rdf:about="http://purl.org/ica/ric#RiC-R-isLocationOf">
        <rdfs:domain rdf:resource="http://purl.org/ica/ric#RiC-E13-Place"/>
        <rdfs:range>
            <owl:Class>
                <owl:unionOf rdf:parseType="Collection">
                    <rdf:Description rdf:about="http://purl.org/ica/ric#RiC-E4-Agent"/>
                    <rdf:Description rdf:about="http://purl.org/ica/ric#RiC-E6-Position"/>
                </owl:unionOf>
            </owl:Class>
        </rdfs:range>
        <rdfs:comment xml:lang="en">Relations RiC-R728, RiC-R736</rdfs:comment>
        <rdfs:label xml:lang="en">is location of</rdfs:label>
        <rdfs:seeAlso rdf:resource="http://purl.org/ica/ric#RiC-R-wasLocationOf"/>
    </owl:ObjectProperty>
    


    <!-- http://purl.org/ica/ric#RiC-R-isManagedBy -->

    <owl:ObjectProperty rdf:about="http://purl.org/ica/ric#RiC-R-isManagedBy">
        <owl:inverseOf rdf:resource="http://purl.org/ica/ric#RiC-R-manages"/>
        <rdfs:domain rdf:resource="http://purl.org/ica/ric#RiC-E3-RecordSet"/>
        <rdfs:range rdf:resource="http://purl.org/ica/ric#RiC-E4-Agent"/>
        <rdfs:comment xml:lang="en">Relations RiC-R153</rdfs:comment>
        <rdfs:label xml:lang="en">is managed by</rdfs:label>
        <rdfs:seeAlso rdf:resource="http://purl.org/ica/ric#RiC-R-wasManagedBy"/>
    </owl:ObjectProperty>
    


    <!-- http://purl.org/ica/ric#RiC-R-isMemberOf -->

    <owl:ObjectProperty rdf:about="http://purl.org/ica/ric#RiC-R-isMemberOf">
        <rdfs:domain>
            <owl:Class>
                <owl:unionOf rdf:parseType="Collection">
                    <rdf:Description rdf:about="http://purl.org/ica/ric#RiC-E1-Record"/>
                    <rdf:Description rdf:about="http://purl.org/ica/ric#RiC-E3-RecordSet"/>
                    <rdf:Description rdf:about="http://purl.org/ica/ric#RiC-E4-Agent"/>
                </owl:unionOf>
            </owl:Class>
        </rdfs:domain>
        <rdfs:range>
            <owl:Class>
                <owl:unionOf rdf:parseType="Collection">
                    <rdf:Description rdf:about="http://purl.org/ica/ric#RiC-E3-RecordSet"/>
                    <rdf:Description rdf:about="http://purl.org/ica/ric#RiC-E4-Agent-Group"/>
                </owl:unionOf>
            </owl:Class>
        </rdfs:range>
        <rdfs:comment xml:lang="en">Relations RiC-R18, RiC-R143, RiC-R266</rdfs:comment>
        <rdfs:label xml:lang="en">is member of</rdfs:label>
        <rdfs:seeAlso rdf:resource="http://purl.org/ica/ric#RiC-R-wasMemberOf"/>
    </owl:ObjectProperty>
    


    <!-- http://purl.org/ica/ric#RiC-R-isOccupiedBy -->

    <owl:ObjectProperty rdf:about="http://purl.org/ica/ric#RiC-R-isOccupiedBy">
        <owl:inverseOf rdf:resource="http://purl.org/ica/ric#RiC-R-occupies"/>
        <rdfs:domain rdf:resource="http://purl.org/ica/ric#RiC-E6-Position"/>
        <rdfs:range rdf:resource="http://purl.org/ica/ric#RiC-E4-Agent-Person"/>
        <rdfs:comment xml:lang="en">Relations RiC-R388</rdfs:comment>
        <rdfs:label xml:lang="en">is occupied by</rdfs:label>
        <rdfs:seeAlso rdf:resource="http://purl.org/ica/ric#RiC-R-wasOccupiedBy"/>
    </owl:ObjectProperty>
    


    <!-- http://purl.org/ica/ric#RiC-R-isOriginalOf -->

    <owl:ObjectProperty rdf:about="http://purl.org/ica/ric#RiC-R-isOriginalOf">
        <rdfs:domain rdf:resource="http://purl.org/ica/ric#RiC-E1-Record"/>
        <rdfs:range rdf:resource="http://purl.org/ica/ric#RiC-E1-Record"/>
        <rdfs:comment xml:lang="en">Relations RiC-R8</rdfs:comment>
        <rdfs:label xml:lang="en">is original of</rdfs:label>
    </owl:ObjectProperty>
    


    <!-- http://purl.org/ica/ric#RiC-R-isOwnedByOwnerOf -->

    <owl:ObjectProperty rdf:about="http://purl.org/ica/ric#RiC-R-isOwnedByOwnerOf">
        <owl:inverseOf rdf:resource="http://purl.org/ica/ric#RiC-R-owns"/>
        <rdfs:domain>
            <owl:Class>
                <owl:unionOf rdf:parseType="Collection">
                    <rdf:Description rdf:about="http://purl.org/ica/ric#RiC-E1-Record"/>
                    <rdf:Description rdf:about="http://purl.org/ica/ric#RiC-E2-RecordComponent"/>
                    <rdf:Description rdf:about="http://purl.org/ica/ric#RiC-E3-RecordSet"/>
                </owl:unionOf>
            </owl:Class>
        </rdfs:domain>
        <rdfs:range rdf:resource="http://purl.org/ica/ric#RiC-E4-Agent"/>
        <rdfs:comment xml:lang="en">Relations RiC-R26, RiC-R89, RiC-R154</rdfs:comment>
        <rdfs:label xml:lang="en">is owned by / is owner of</rdfs:label>
        <rdfs:seeAlso rdf:resource="http://purl.org/ica/ric#RiC-R-wasOwnedBy"/>
    </owl:ObjectProperty>
    


    <!-- http://purl.org/ica/ric#RiC-R-isParentOf -->

    <owl:ObjectProperty rdf:about="http://purl.org/ica/ric#RiC-R-isParentOf">
        <rdfs:domain rdf:resource="http://purl.org/ica/ric#RiC-E4-Agent-Person"/>
        <rdfs:range rdf:resource="http://purl.org/ica/ric#RiC-E4-Agent-Person"/>
        <rdfs:comment xml:lang="en">Relations RiC-R267</rdfs:comment>
        <rdfs:label xml:lang="en">is parent of</rdfs:label>
        <rdfs:seeAlso rdf:resource="http://purl.org/ica/ric#RiC-R-wasParentOf"/>
    </owl:ObjectProperty>
    


    <!-- http://purl.org/ica/ric#RiC-R-isPartOf -->

    <owl:ObjectProperty rdf:about="http://purl.org/ica/ric#RiC-R-isPartOf">
        <rdfs:domain>
            <owl:Class>
                <owl:unionOf rdf:parseType="Collection">
                    <rdf:Description rdf:about="http://purl.org/ica/ric#RiC-E2-RecordComponent"/>
                    <rdf:Description rdf:about="http://purl.org/ica/ric#RiC-E4-Agent-Group"/>
                    <rdf:Description rdf:about="http://purl.org/ica/ric#RiC-E7-Function"/>
                    <rdf:Description rdf:about="http://purl.org/ica/ric#RiC-E9-Activity"/>
                </owl:unionOf>
            </owl:Class>
        </rdfs:domain>
        <rdfs:range>
            <owl:Class>
                <owl:unionOf rdf:parseType="Collection">
                    <rdf:Description rdf:about="http://purl.org/ica/ric#RiC-E1-Record"/>
                    <rdf:Description rdf:about="http://purl.org/ica/ric#RiC-E4-Agent-Group"/>
                    <rdf:Description rdf:about="http://purl.org/ica/ric#RiC-E7-Function"/>
                    <rdf:Description rdf:about="http://purl.org/ica/ric#RiC-E9-Activity"/>
                </owl:unionOf>
            </owl:Class>
        </rdfs:range>
        <rdfs:comment xml:lang="en">Relations RiC-R75, RiC-R268, RiC-R447, RiC-R538</rdfs:comment>
        <rdfs:label xml:lang="en">is part of</rdfs:label>
        <rdfs:seeAlso rdf:resource="http://purl.org/ica/ric#RiC-R-wasPartOf"/>
    </owl:ObjectProperty>
    


    <!-- http://purl.org/ica/ric#RiC-R-isPerformedBy -->

    <owl:ObjectProperty rdf:about="http://purl.org/ica/ric#RiC-R-isPerformedBy">
        <owl:inverseOf rdf:resource="http://purl.org/ica/ric#RiC-R-performs"/>
        <rdfs:domain rdf:resource="http://purl.org/ica/ric#RiC-E9-Activity"/>
        <rdfs:range rdf:resource="http://purl.org/ica/ric#RiC-E4-Agent"/>
        <rdfs:comment xml:lang="en">Relations RiC-R522</rdfs:comment>
        <rdfs:label xml:lang="en">is performed by</rdfs:label>
        <rdfs:seeAlso rdf:resource="http://purl.org/ica/ric#RiC-R-wasPerformedBy"/>
    </owl:ObjectProperty>
    


    <!-- http://purl.org/ica/ric#RiC-R-isPerformedToFulfil -->

    <owl:ObjectProperty rdf:about="http://purl.org/ica/ric#RiC-R-isPerformedToFulfil">
        <rdfs:domain rdf:resource="http://purl.org/ica/ric#RiC-E9-Activity"/>
        <rdfs:range rdf:resource="http://purl.org/ica/ric#RiC-E7-Function"/>
        <rdfs:comment xml:lang="en">Relations RiC-R530</rdfs:comment>
        <rdfs:label xml:lang="en">is performed to fulfil</rdfs:label>
        <rdfs:seeAlso rdf:resource="http://purl.org/ica/ric#RiC-R-wasPerformedToFulfill"/>
    </owl:ObjectProperty>
    


    <!-- http://purl.org/ica/ric#RiC-R-isPredecessorOf -->

    <owl:ObjectProperty rdf:about="http://purl.org/ica/ric#RiC-R-isPredecessorOf">
        <owl:inverseOf rdf:resource="http://purl.org/ica/ric#RiC-R-isSuccessorOf"/>
        <rdf:type rdf:resource="http://www.w3.org/2002/07/owl#TransitiveProperty"/>
        <rdf:type rdf:resource="http://www.w3.org/2002/07/owl#ReflexiveProperty"/>
        <rdfs:domain>
            <owl:Class>
                <owl:unionOf rdf:parseType="Collection">
                    <rdf:Description rdf:about="http://purl.org/ica/ric#RiC-E1-Record"/>
                    <rdf:Description rdf:about="http://purl.org/ica/ric#RiC-E10-Mandate"/>
                    <rdf:Description rdf:about="http://purl.org/ica/ric#RiC-E2-RecordComponent"/>
                    <rdf:Description rdf:about="http://purl.org/ica/ric#RiC-E3-RecordSet"/>
                    <rdf:Description rdf:about="http://purl.org/ica/ric#RiC-E4-Agent"/>
                    <rdf:Description rdf:about="http://purl.org/ica/ric#RiC-E5-Occupation"/>
                    <rdf:Description rdf:about="http://purl.org/ica/ric#RiC-E6-Position"/>
                    <rdf:Description rdf:about="http://purl.org/ica/ric#RiC-E7-Function"/>
                    <rdf:Description rdf:about="http://purl.org/ica/ric#RiC-E9-Activity"/>
                </owl:unionOf>
            </owl:Class>
        </rdfs:domain>
        <rdfs:range>
            <owl:Class>
                <owl:unionOf rdf:parseType="Collection">
                    <rdf:Description rdf:about="http://purl.org/ica/ric#RiC-E1-Record"/>
                    <rdf:Description rdf:about="http://purl.org/ica/ric#RiC-E10-Mandate"/>
                    <rdf:Description rdf:about="http://purl.org/ica/ric#RiC-E2-RecordComponent"/>
                    <rdf:Description rdf:about="http://purl.org/ica/ric#RiC-E3-RecordSet"/>
                    <rdf:Description rdf:about="http://purl.org/ica/ric#RiC-E4-Agent"/>
                    <rdf:Description rdf:about="http://purl.org/ica/ric#RiC-E5-Occupation"/>
                    <rdf:Description rdf:about="http://purl.org/ica/ric#RiC-E6-Position"/>
                    <rdf:Description rdf:about="http://purl.org/ica/ric#RiC-E7-Function"/>
                    <rdf:Description rdf:about="http://purl.org/ica/ric#RiC-E9-Activity"/>
                </owl:unionOf>
            </owl:Class>
        </rdfs:range>
        <rdfs:comment xml:lang="en">Relations RiC-R9, RiC-R79, RiC-R144, RiC-R269, RiC-R352, RiC-R397, RiC-R448, RiC-R539, RiC-R595</rdfs:comment>
        <rdfs:label xml:lang="en">is predecessor of</rdfs:label>
    </owl:ObjectProperty>
    


    <!-- http://purl.org/ica/ric#RiC-R-isPursuedBy -->

    <owl:ObjectProperty rdf:about="http://purl.org/ica/ric#RiC-R-isPursuedBy">
        <owl:inverseOf rdf:resource="http://purl.org/ica/ric#RiC-R-pursues"/>
        <rdfs:domain rdf:resource="http://purl.org/ica/ric#RiC-E5-Occupation"/>
        <rdfs:range rdf:resource="http://purl.org/ica/ric#RiC-E4-Agent"/>
        <rdfs:comment xml:lang="en">Relations RiC-R348</rdfs:comment>
        <rdfs:label xml:lang="en">is pursued by</rdfs:label>
        <rdfs:seeAlso rdf:resource="http://purl.org/ica/ric#RiC-R-wasPursuedBy"/>
    </owl:ObjectProperty>
    


    <!-- http://purl.org/ica/ric#RiC-R-isRequiredCompetencyOf -->

    <owl:ObjectProperty rdf:about="http://purl.org/ica/ric#RiC-R-isRequiredCompetencyOf">
        <owl:inverseOf rdf:resource="http://purl.org/ica/ric#RiC-R-requiresCompetency"/>
        <rdfs:domain rdf:resource="http://purl.org/ica/ric#RiC-E5-Occupation"/>
        <rdfs:range rdf:resource="http://purl.org/ica/ric#RiC-E6-Position"/>
        <rdfs:comment xml:lang="en">Relations RiC-R356</rdfs:comment>
        <rdfs:label xml:lang="en">is required competency of</rdfs:label>
        <rdfs:seeAlso rdf:resource="http://purl.org/ica/ric#RiC-R-wasRequiredCompetencyOf"/>
    </owl:ObjectProperty>
    


    <!-- http://purl.org/ica/ric#RiC-R-isRightsHolderOf -->

    <owl:ObjectProperty rdf:about="http://purl.org/ica/ric#RiC-R-isRightsHolderOf">
        <rdfs:domain rdf:resource="http://purl.org/ica/ric#RiC-E4-Agent"/>
        <rdfs:range>
            <owl:Class>
                <owl:unionOf rdf:parseType="Collection">
                    <rdf:Description rdf:about="http://purl.org/ica/ric#RiC-E1-Record"/>
                    <rdf:Description rdf:about="http://purl.org/ica/ric#RiC-E2-RecordComponent"/>
                    <rdf:Description rdf:about="http://purl.org/ica/ric#RiC-E3-RecordSet"/>
                </owl:unionOf>
            </owl:Class>
        </rdfs:range>
        <rdfs:comment xml:lang="en">Relations RiC-R209, RiC-R224, RiC-R239</rdfs:comment>
        <rdfs:label xml:lang="en">is rights holder of</rdfs:label>
        <rdfs:seeAlso rdf:resource="http://purl.org/ica/ric#RiC-R-wasRightsHolderOf"/>
    </owl:ObjectProperty>
    


    <!-- http://purl.org/ica/ric#RiC-R-isSiblingOf -->

    <owl:ObjectProperty rdf:about="http://purl.org/ica/ric#RiC-R-isSiblingOf">
        <rdf:type rdf:resource="http://www.w3.org/2002/07/owl#SymmetricProperty"/>
        <rdfs:domain rdf:resource="http://purl.org/ica/ric#RiC-E4-Agent-Person"/>
        <rdfs:range rdf:resource="http://purl.org/ica/ric#RiC-E4-Agent-Person"/>
        <rdfs:comment xml:lang="en">Relations RiC-R270</rdfs:comment>
        <rdfs:label xml:lang="en">is sibling of</rdfs:label>
        <rdfs:seeAlso rdf:resource="http://purl.org/ica/ric#RiC-R-wasSiblingOf"/>
    </owl:ObjectProperty>
    


    <!-- http://purl.org/ica/ric#RiC-R-isSpouseOf -->

    <owl:ObjectProperty rdf:about="http://purl.org/ica/ric#RiC-R-isSpouseOf">
        <rdf:type rdf:resource="http://www.w3.org/2002/07/owl#SymmetricProperty"/>
        <rdfs:domain rdf:resource="http://purl.org/ica/ric#RiC-E4-Agent-Person"/>
        <rdfs:range rdf:resource="http://purl.org/ica/ric#RiC-E4-Agent-Person"/>
        <rdfs:comment xml:lang="en">Relations RiC-R271</rdfs:comment>
        <rdfs:label xml:lang="en">is spouse of</rdfs:label>
        <rdfs:seeAlso rdf:resource="http://purl.org/ica/ric#RiC-R-wasSpouseOf"/>
    </owl:ObjectProperty>
    


    <!-- http://purl.org/ica/ric#RiC-R-isSubjectOf -->

    <owl:ObjectProperty rdf:about="http://purl.org/ica/ric#RiC-R-isSubjectOf">
        <rdfs:domain>
            <owl:Class>
                <owl:unionOf rdf:parseType="Collection">
                    <rdf:Description rdf:about="http://purl.org/ica/ric#RiC-E1-Record"/>
                    <rdf:Description rdf:about="http://purl.org/ica/ric#RiC-E10-Mandate"/>
                    <rdf:Description rdf:about="http://purl.org/ica/ric#RiC-E13-Place"/>
                    <rdf:Description rdf:about="http://purl.org/ica/ric#RiC-E14-ConceptThing"/>
                    <rdf:Description rdf:about="http://purl.org/ica/ric#RiC-E4-Agent"/>
                    <rdf:Description rdf:about="http://purl.org/ica/ric#RiC-E5-Occupation"/>
                    <rdf:Description rdf:about="http://purl.org/ica/ric#RiC-E6-Position"/>
                    <rdf:Description rdf:about="http://purl.org/ica/ric#RiC-E7-Function"/>
                    <rdf:Description rdf:about="http://purl.org/ica/ric#RiC-E8-FunctionAbstract"/>
                    <rdf:Description rdf:about="http://purl.org/ica/ric#RiC-E9-Activity"/>
                </owl:unionOf>
            </owl:Class>
        </rdfs:domain>
        <rdfs:range>
            <owl:Class>
                <owl:unionOf rdf:parseType="Collection">
                    <rdf:Description rdf:about="http://purl.org/ica/ric#RiC-E1-Record"/>
                    <rdf:Description rdf:about="http://purl.org/ica/ric#RiC-E2-RecordComponent"/>
                    <rdf:Description rdf:about="http://purl.org/ica/ric#RiC-E3-RecordSet"/>
                </owl:unionOf>
            </owl:Class>
        </rdfs:range>
        <rdfs:comment xml:lang="en">Relations RiC-R10, RiC-R210, RiC-R225, RiC-R240, RiC-R336, RiC-R340, RiC-R344, RiC-R376, RiC-R380, RiC-R384, RiC-R426, RiC-R430, RiC-R434, RiC-R478, RiC-R481, RiC-R484, RiC-R510, RiC-R514, RiC-R518, RiC-R563, RiC-R566, RiC-R570, RiC-R709, RiC-R715, RiC-R721, RiC-R763, RiC-R766, RiC-R769</rdfs:comment>
        <rdfs:label xml:lang="en">is subject of</rdfs:label>
    </owl:ObjectProperty>
    


    <!-- http://purl.org/ica/ric#RiC-R-isSubordinateOf -->

    <owl:ObjectProperty rdf:about="http://purl.org/ica/ric#RiC-R-isSubordinateOf">
        <owl:inverseOf rdf:resource="http://purl.org/ica/ric#RiC-R-isSuperiorOf"/>
        <rdfs:domain rdf:resource="http://purl.org/ica/ric#RiC-E4-Agent"/>
        <rdfs:range rdf:resource="http://purl.org/ica/ric#RiC-E4-Agent"/>
        <rdfs:comment xml:lang="en">Relations RiC-R272</rdfs:comment>
        <rdfs:label xml:lang="en">is subordinate of</rdfs:label>
        <rdfs:seeAlso rdf:resource="http://purl.org/ica/ric#RiC-R-wasSubordinateOf"/>
    </owl:ObjectProperty>
    


    <!-- http://purl.org/ica/ric#RiC-R-isSuccessorOf -->

    <owl:ObjectProperty rdf:about="http://purl.org/ica/ric#RiC-R-isSuccessorOf">
        <rdf:type rdf:resource="http://www.w3.org/2002/07/owl#TransitiveProperty"/>
        <rdf:type rdf:resource="http://www.w3.org/2002/07/owl#ReflexiveProperty"/>
        <rdfs:domain>
            <owl:Class>
                <owl:unionOf rdf:parseType="Collection">
                    <rdf:Description rdf:about="http://purl.org/ica/ric#RiC-E1-Record"/>
                    <rdf:Description rdf:about="http://purl.org/ica/ric#RiC-E10-Mandate"/>
                    <rdf:Description rdf:about="http://purl.org/ica/ric#RiC-E2-RecordComponent"/>
                    <rdf:Description rdf:about="http://purl.org/ica/ric#RiC-E3-RecordSet"/>
                    <rdf:Description rdf:about="http://purl.org/ica/ric#RiC-E4-Agent"/>
                    <rdf:Description rdf:about="http://purl.org/ica/ric#RiC-E5-Occupation"/>
                    <rdf:Description rdf:about="http://purl.org/ica/ric#RiC-E6-Position"/>
                    <rdf:Description rdf:about="http://purl.org/ica/ric#RiC-E7-Function"/>
                    <rdf:Description rdf:about="http://purl.org/ica/ric#RiC-E9-Activity"/>
                </owl:unionOf>
            </owl:Class>
        </rdfs:domain>
        <rdfs:range>
            <owl:Class>
                <owl:unionOf rdf:parseType="Collection">
                    <rdf:Description rdf:about="http://purl.org/ica/ric#RiC-E1-Record"/>
                    <rdf:Description rdf:about="http://purl.org/ica/ric#RiC-E10-Mandate"/>
                    <rdf:Description rdf:about="http://purl.org/ica/ric#RiC-E2-RecordComponent"/>
                    <rdf:Description rdf:about="http://purl.org/ica/ric#RiC-E3-RecordSet"/>
                    <rdf:Description rdf:about="http://purl.org/ica/ric#RiC-E4-Agent"/>
                    <rdf:Description rdf:about="http://purl.org/ica/ric#RiC-E5-Occupation"/>
                    <rdf:Description rdf:about="http://purl.org/ica/ric#RiC-E6-Position"/>
                    <rdf:Description rdf:about="http://purl.org/ica/ric#RiC-E7-Function"/>
                    <rdf:Description rdf:about="http://purl.org/ica/ric#RiC-E9-Activity"/>
                </owl:unionOf>
            </owl:Class>
        </rdfs:range>
        <rdfs:comment xml:lang="en">Relations RiC-R11, RiC-R80, RiC-R145, RiC-R273, RiC-R353, RiC-R398, RiC-R449, RiC-R540, RiC-R596</rdfs:comment>
        <rdfs:label xml:lang="en">is successor of</rdfs:label>
    </owl:ObjectProperty>
    


    <!-- http://purl.org/ica/ric#RiC-R-isSuperiorOf -->

    <owl:ObjectProperty rdf:about="http://purl.org/ica/ric#RiC-R-isSuperiorOf">
        <rdfs:domain rdf:resource="http://purl.org/ica/ric#RiC-E4-Agent"/>
        <rdfs:range rdf:resource="http://purl.org/ica/ric#RiC-E4-Agent"/>
        <rdfs:comment xml:lang="en">Relations RiC-R274</rdfs:comment>
        <rdfs:label xml:lang="en">is superior of</rdfs:label>
        <rdfs:seeAlso rdf:resource="http://purl.org/ica/ric#RiC-R-wasSuperiorOf"/>
    </owl:ObjectProperty>
    


    <!-- http://purl.org/ica/ric#RiC-R-isUsedBy -->

    <owl:ObjectProperty rdf:about="http://purl.org/ica/ric#RiC-R-isUsedBy">
        <owl:inverseOf rdf:resource="http://purl.org/ica/ric#RiC-R-uses"/>
        <rdfs:domain rdf:resource="http://purl.org/ica/ric#RiC-E4-Agent-DelegateAgent"/>
        <rdfs:range rdf:resource="http://purl.org/ica/ric#RiC-E4-Agent"/>
        <rdfs:comment xml:lang="en">Relations RiC-R275</rdfs:comment>
        <rdfs:label xml:lang="en">is used by</rdfs:label>
        <rdfs:seeAlso rdf:resource="http://purl.org/ica/ric#RiC-R-wasUsedBy"/>
    </owl:ObjectProperty>
    


    <!-- http://purl.org/ica/ric#RiC-R-managed -->

    <owl:ObjectProperty rdf:about="http://purl.org/ica/ric#RiC-R-managed">
        <owl:inverseOf rdf:resource="http://purl.org/ica/ric#RiC-R-wasManagedBy"/>
        <rdfs:domain rdf:resource="http://purl.org/ica/ric#RiC-E4-Agent"/>
        <rdfs:range rdf:resource="http://purl.org/ica/ric#RiC-E3-RecordSet"/>
        <rdfs:comment xml:lang="en">Relations RiC-R241</rdfs:comment>
        <rdfs:label xml:lang="en">managed</rdfs:label>
        <rdfs:seeAlso rdf:resource="http://purl.org/ica/ric#RiC-R-manages"/>
    </owl:ObjectProperty>
    


    <!-- http://purl.org/ica/ric#RiC-R-manages -->

    <owl:ObjectProperty rdf:about="http://purl.org/ica/ric#RiC-R-manages">
        <rdfs:domain rdf:resource="http://purl.org/ica/ric#RiC-E4-Agent"/>
        <rdfs:range rdf:resource="http://purl.org/ica/ric#RiC-E3-RecordSet"/>
        <rdfs:comment xml:lang="en">Relations RiC-R242</rdfs:comment>
        <rdfs:label xml:lang="en">manages</rdfs:label>
        <rdfs:seeAlso rdf:resource="http://purl.org/ica/ric#RiC-R-managed"/>
    </owl:ObjectProperty>
    


    <!-- http://purl.org/ica/ric#RiC-R-occupied -->

    <owl:ObjectProperty rdf:about="http://purl.org/ica/ric#RiC-R-occupied">
        <owl:inverseOf rdf:resource="http://purl.org/ica/ric#RiC-R-wasOccupiedBy"/>
        <rdfs:domain rdf:resource="http://purl.org/ica/ric#RiC-E4-Agent-Person"/>
        <rdfs:range rdf:resource="http://purl.org/ica/ric#RiC-E6-Position"/>
        <rdfs:comment xml:lang="en">Relations RiC-R298</rdfs:comment>
        <rdfs:label xml:lang="en">occupied</rdfs:label>
        <rdfs:seeAlso rdf:resource="http://purl.org/ica/ric#RiC-R-occupies"/>
    </owl:ObjectProperty>
    


    <!-- http://purl.org/ica/ric#RiC-R-occupies -->

    <owl:ObjectProperty rdf:about="http://purl.org/ica/ric#RiC-R-occupies">
        <rdfs:domain rdf:resource="http://purl.org/ica/ric#RiC-E4-Agent-Person"/>
        <rdfs:range rdf:resource="http://purl.org/ica/ric#RiC-E6-Position"/>
        <rdfs:comment xml:lang="en">Relations RiC-R299</rdfs:comment>
        <rdfs:label xml:lang="en">occupies</rdfs:label>
        <rdfs:seeAlso rdf:resource="http://purl.org/ica/ric#RiC-R-occupied"/>
    </owl:ObjectProperty>
    


    <!-- http://purl.org/ica/ric#RiC-R-owned -->

    <owl:ObjectProperty rdf:about="http://purl.org/ica/ric#RiC-R-owned">
        <owl:inverseOf rdf:resource="http://purl.org/ica/ric#RiC-R-wasOwnedByOwnerOf"/>
        <rdfs:domain rdf:resource="http://purl.org/ica/ric#RiC-E4-Agent"/>
        <rdfs:range>
            <owl:Class>
                <owl:unionOf rdf:parseType="Collection">
                    <rdf:Description rdf:about="http://purl.org/ica/ric#RiC-E1-Record"/>
                    <rdf:Description rdf:about="http://purl.org/ica/ric#RiC-E2-RecordComponent"/>
                    <rdf:Description rdf:about="http://purl.org/ica/ric#RiC-E3-RecordSet"/>
                </owl:unionOf>
            </owl:Class>
        </rdfs:range>
        <rdfs:comment xml:lang="en">Relations RiC-R211, RiC-R226, RiC-R243</rdfs:comment>
        <rdfs:label xml:lang="en">owned</rdfs:label>
        <rdfs:seeAlso rdf:resource="http://purl.org/ica/ric#RiC-R-owns"/>
    </owl:ObjectProperty>
    


    <!-- http://purl.org/ica/ric#RiC-R-owns -->

    <owl:ObjectProperty rdf:about="http://purl.org/ica/ric#RiC-R-owns">
        <rdfs:domain rdf:resource="http://purl.org/ica/ric#RiC-E4-Agent"/>
        <rdfs:range>
            <owl:Class>
                <owl:unionOf rdf:parseType="Collection">
                    <rdf:Description rdf:about="http://purl.org/ica/ric#RiC-E1-Record"/>
                    <rdf:Description rdf:about="http://purl.org/ica/ric#RiC-E2-RecordComponent"/>
                    <rdf:Description rdf:about="http://purl.org/ica/ric#RiC-E3-RecordSet"/>
                </owl:unionOf>
            </owl:Class>
        </rdfs:range>
        <rdfs:comment xml:lang="en">Relations RiC-R212, RiC-R227, RiC-R244</rdfs:comment>
        <rdfs:label xml:lang="en">owns</rdfs:label>
        <rdfs:seeAlso rdf:resource="http://purl.org/ica/ric#RiC-R-owned"/>
    </owl:ObjectProperty>
    


    <!-- http://purl.org/ica/ric#RiC-R-performed -->

    <owl:ObjectProperty rdf:about="http://purl.org/ica/ric#RiC-R-performed">
        <owl:inverseOf rdf:resource="http://purl.org/ica/ric#RiC-R-wasPerformedBy"/>
        <rdfs:domain rdf:resource="http://purl.org/ica/ric#RiC-E4-Agent"/>
        <rdfs:range rdf:resource="http://purl.org/ica/ric#RiC-E9-Activity"/>
        <rdfs:comment xml:lang="en">Relations RiC-R308</rdfs:comment>
        <rdfs:label xml:lang="en">performed</rdfs:label>
        <rdfs:seeAlso rdf:resource="http://purl.org/ica/ric#RiC-R-performs"/>
    </owl:ObjectProperty>
    


    <!-- http://purl.org/ica/ric#RiC-R-performs -->

    <owl:ObjectProperty rdf:about="http://purl.org/ica/ric#RiC-R-performs">
        <rdfs:domain rdf:resource="http://purl.org/ica/ric#RiC-E4-Agent"/>
        <rdfs:range rdf:resource="http://purl.org/ica/ric#RiC-E9-Activity"/>
        <rdfs:comment xml:lang="en">Relations RiC-R309</rdfs:comment>
        <rdfs:label xml:lang="en">performs</rdfs:label>
        <rdfs:seeAlso rdf:resource="http://purl.org/ica/ric#RiC-R-performed"/>
    </owl:ObjectProperty>
    


    <!-- http://purl.org/ica/ric#RiC-R-pursued -->

    <owl:ObjectProperty rdf:about="http://purl.org/ica/ric#RiC-R-pursued">
        <owl:inverseOf rdf:resource="http://purl.org/ica/ric#RiC-R-wasPursuedBy"/>
        <rdfs:domain rdf:resource="http://purl.org/ica/ric#RiC-E4-Agent"/>
        <rdfs:range rdf:resource="http://purl.org/ica/ric#RiC-E5-Occupation"/>
        <rdfs:comment xml:lang="en">Relations RiC-R293</rdfs:comment>
        <rdfs:label xml:lang="en">pursued</rdfs:label>
        <rdfs:seeAlso rdf:resource="http://purl.org/ica/ric#RiC-R-pursues"/>
    </owl:ObjectProperty>
    


    <!-- http://purl.org/ica/ric#RiC-R-pursues -->

    <owl:ObjectProperty rdf:about="http://purl.org/ica/ric#RiC-R-pursues">
        <rdfs:domain rdf:resource="http://purl.org/ica/ric#RiC-E4-Agent"/>
        <rdfs:range rdf:resource="http://purl.org/ica/ric#RiC-E5-Occupation"/>
        <rdfs:comment xml:lang="en">Relations RiC-R294</rdfs:comment>
        <rdfs:label xml:lang="en">pursues</rdfs:label>
        <rdfs:seeAlso rdf:resource="http://purl.org/ica/ric#RiC-R-pursued"/>
    </owl:ObjectProperty>
    


    <!-- http://purl.org/ica/ric#RiC-R-requiredCompetency -->

    <owl:ObjectProperty rdf:about="http://purl.org/ica/ric#RiC-R-requiredCompetency">
        <owl:inverseOf rdf:resource="http://purl.org/ica/ric#RiC-R-wasRequiredCompetencyOf"/>
        <rdfs:domain rdf:resource="http://purl.org/ica/ric#RiC-E6-Position"/>
        <rdfs:range rdf:resource="http://purl.org/ica/ric#RiC-E5-Occupation"/>
        <rdfs:comment xml:lang="en">Relations RiC-R393</rdfs:comment>
        <rdfs:label xml:lang="en">required competency</rdfs:label>
        <rdfs:seeAlso rdf:resource="http://purl.org/ica/ric#RiC-R-requiresCompetency"/>
    </owl:ObjectProperty>
    


    <!-- http://purl.org/ica/ric#RiC-R-requiresCompetency -->

    <owl:ObjectProperty rdf:about="http://purl.org/ica/ric#RiC-R-requiresCompetency">
        <rdfs:domain rdf:resource="http://purl.org/ica/ric#RiC-E6-Position"/>
        <rdfs:range rdf:resource="http://purl.org/ica/ric#RiC-E5-Occupation"/>
        <rdfs:comment xml:lang="en">Relations RiC-R394</rdfs:comment>
        <rdfs:label xml:lang="en">requires competency</rdfs:label>
        <rdfs:seeAlso rdf:resource="http://purl.org/ica/ric#RiC-R-requiredCompetency"/>
    </owl:ObjectProperty>
    


    <!-- http://purl.org/ica/ric#RiC-R-resultedFrom -->

    <owl:ObjectProperty rdf:about="http://purl.org/ica/ric#RiC-R-resultedFrom">
        <owl:inverseOf rdf:resource="http://purl.org/ica/ric#RiC-R-resultedIn"/>
        <rdfs:domain>
            <owl:Class>
                <owl:unionOf rdf:parseType="Collection">
                    <rdf:Description rdf:about="http://purl.org/ica/ric#RiC-E1-Record"/>
                    <rdf:Description rdf:about="http://purl.org/ica/ric#RiC-E2-RecordComponent"/>
                    <rdf:Description rdf:about="http://purl.org/ica/ric#RiC-E3-RecordSet"/>
                </owl:unionOf>
            </owl:Class>
        </rdfs:domain>
        <rdfs:range>
            <owl:Class>
                <owl:unionOf rdf:parseType="Collection">
                    <rdf:Description rdf:about="http://purl.org/ica/ric#RiC-E5-Occupation"/>
                    <rdf:Description rdf:about="http://purl.org/ica/ric#RiC-E6-Position"/>
                    <rdf:Description rdf:about="http://purl.org/ica/ric#RiC-E9-Activity"/>
                </owl:unionOf>
            </owl:Class>
        </rdfs:range>
        <rdfs:comment xml:lang="en">Relations RiC-R38, RiC-R42, RiC-R53, RiC-R99, RiC-R103, RiC-R114, RiC-R168, RiC-R172, RiC-R183</rdfs:comment>
        <rdfs:label xml:lang="en">resulted from</rdfs:label>
    </owl:ObjectProperty>
    


    <!-- http://purl.org/ica/ric#RiC-R-resultedIn -->

    <owl:ObjectProperty rdf:about="http://purl.org/ica/ric#RiC-R-resultedIn">
        <rdfs:domain>
            <owl:Class>
                <owl:unionOf rdf:parseType="Collection">
                    <rdf:Description rdf:about="http://purl.org/ica/ric#RiC-E5-Occupation"/>
                    <rdf:Description rdf:about="http://purl.org/ica/ric#RiC-E6-Position"/>
                    <rdf:Description rdf:about="http://purl.org/ica/ric#RiC-E9-Activity"/>
                </owl:unionOf>
            </owl:Class>
        </rdfs:domain>
        <rdfs:range>
            <owl:Class>
                <owl:unionOf rdf:parseType="Collection">
                    <rdf:Description rdf:about="http://purl.org/ica/ric#RiC-E1-Record"/>
                    <rdf:Description rdf:about="http://purl.org/ica/ric#RiC-E2-RecordComponent"/>
                    <rdf:Description rdf:about="http://purl.org/ica/ric#RiC-E3-RecordSet"/>
                </owl:unionOf>
            </owl:Class>
        </rdfs:range>
        <rdfs:comment xml:lang="en">Relations RiC-R337, RiC-R341, RiC-R345, RiC-R377, RiC-R381, RiC-R385, RiC-R511, RiC-R515, RiC-R519</rdfs:comment>
        <rdfs:label xml:lang="en">resulted in</rdfs:label>
    </owl:ObjectProperty>
    


    <!-- http://purl.org/ica/ric#RiC-R-revised -->

    <owl:ObjectProperty rdf:about="http://purl.org/ica/ric#RiC-R-revised">
        <owl:inverseOf rdf:resource="http://purl.org/ica/ric#RiC-R-wasRevisedBy"/>
        <rdfs:domain rdf:resource="http://purl.org/ica/ric#RiC-E10-Mandate"/>
        <rdfs:range>
            <owl:Class>
                <owl:unionOf rdf:parseType="Collection">
                    <rdf:Description rdf:about="http://purl.org/ica/ric#RiC-E6-Position"/>
                    <rdf:Description rdf:about="http://purl.org/ica/ric#RiC-E7-Function"/>
                    <rdf:Description rdf:about="http://purl.org/ica/ric#RiC-E9-Activity"/>
                </owl:unionOf>
            </owl:Class>
        </rdfs:range>
        <rdfs:comment xml:lang="en">Relations RiC-R580, RiC-R585, RiC-R592</rdfs:comment>
        <rdfs:label xml:lang="en">revised</rdfs:label>
    </owl:ObjectProperty>
    


    <!-- http://purl.org/ica/ric#RiC-R-sent -->

    <owl:ObjectProperty rdf:about="http://purl.org/ica/ric#RiC-R-sent">
        <owl:inverseOf rdf:resource="http://purl.org/ica/ric#RiC-R-wasSentBy"/>
        <rdfs:domain rdf:resource="http://purl.org/ica/ric#RiC-E4-Agent"/>
        <rdfs:range>
            <owl:Class>
                <owl:unionOf rdf:parseType="Collection">
                    <rdf:Description rdf:about="http://purl.org/ica/ric#RiC-E1-Record"/>
                    <rdf:Description rdf:about="http://purl.org/ica/ric#RiC-E3-RecordSet"/>
                </owl:unionOf>
            </owl:Class>
        </rdfs:range>
        <rdfs:comment xml:lang="en">Relations RiC-R213, RiC-R245</rdfs:comment>
        <rdfs:label xml:lang="en">sent</rdfs:label>
    </owl:ObjectProperty>
    


    <!-- http://purl.org/ica/ric#RiC-R-used -->

    <owl:ObjectProperty rdf:about="http://purl.org/ica/ric#RiC-R-used">
        <owl:inverseOf rdf:resource="http://purl.org/ica/ric#RiC-R-wasUsedBy"/>
        <rdfs:domain rdf:resource="http://purl.org/ica/ric#RiC-E4-Agent"/>
        <rdfs:range rdf:resource="http://purl.org/ica/ric#RiC-E4-Agent-DelegateAgent"/>
        <rdfs:comment xml:lang="en">Relations RiC-R276</rdfs:comment>
        <rdfs:label xml:lang="en">used</rdfs:label>
        <rdfs:seeAlso rdf:resource="http://purl.org/ica/ric#RiC-R-uses"/>
    </owl:ObjectProperty>
    


    <!-- http://purl.org/ica/ric#RiC-R-uses -->

    <owl:ObjectProperty rdf:about="http://purl.org/ica/ric#RiC-R-uses">
        <rdfs:domain rdf:resource="http://purl.org/ica/ric#RiC-E4-Agent"/>
        <rdfs:range rdf:resource="http://purl.org/ica/ric#RiC-E4-Agent-DelegateAgent"/>
        <rdfs:comment xml:lang="en">Relations RiC-R277</rdfs:comment>
        <rdfs:label xml:lang="en">uses</rdfs:label>
        <rdfs:seeAlso rdf:resource="http://purl.org/ica/ric#RiC-R-used"/>
    </owl:ObjectProperty>
    


    <!-- http://purl.org/ica/ric#RiC-R-wasAccumulatedBy -->

    <owl:ObjectProperty rdf:about="http://purl.org/ica/ric#RiC-R-wasAccumulatedBy">
        <rdfs:domain rdf:resource="http://purl.org/ica/ric#RiC-E3-RecordSet"/>
        <rdfs:range rdf:resource="http://purl.org/ica/ric#RiC-E4-Agent"/>
        <rdfs:comment xml:lang="en">Relations RiC-R155</rdfs:comment>
        <rdfs:label xml:lang="en">was accumulated by</rdfs:label>
    </owl:ObjectProperty>
    


    <!-- http://purl.org/ica/ric#RiC-R-wasActiveDateOf -->

    <owl:ObjectProperty rdf:about="http://purl.org/ica/ric#RiC-R-wasActiveDateOf">
        <rdfs:domain rdf:resource="http://purl.org/ica/ric#RiC-E12-Date"/>
        <rdfs:range>
            <owl:Class>
                <owl:unionOf rdf:parseType="Collection">
                    <rdf:Description rdf:about="http://purl.org/ica/ric#RiC-E10-Mandate"/>
                    <rdf:Description rdf:about="http://purl.org/ica/ric#RiC-E13-Place"/>
                    <rdf:Description rdf:about="http://purl.org/ica/ric#RiC-E4-Agent"/>
                    <rdf:Description rdf:about="http://purl.org/ica/ric#RiC-E7-Function"/>
                    <rdf:Description rdf:about="http://purl.org/ica/ric#RiC-E9-Activity"/>
                </owl:unionOf>
            </owl:Class>
        </rdfs:range>
        <rdfs:comment xml:lang="en">Relations RiC-R657, RiC-R673, RiC-R682, RiC-R689, RiC-R701</rdfs:comment>
        <rdfs:label xml:lang="en">was active date of</rdfs:label>
        <rdfs:seeAlso rdf:resource="http://purl.org/ica/ric#RiC-R-isActiveDateOf"/>
    </owl:ObjectProperty>
    


    <!-- http://purl.org/ica/ric#RiC-R-wasAddressedTo -->

    <owl:ObjectProperty rdf:about="http://purl.org/ica/ric#RiC-R-wasAddressedTo">
        <owl:inverseOf rdf:resource="http://purl.org/ica/ric#RiC-R-wasAddresseeOf"/>
        <rdfs:domain>
            <owl:Class>
                <owl:unionOf rdf:parseType="Collection">
                    <rdf:Description rdf:about="http://purl.org/ica/ric#RiC-E1-Record"/>
                    <rdf:Description rdf:about="http://purl.org/ica/ric#RiC-E3-RecordSet"/>
                </owl:unionOf>
            </owl:Class>
        </rdfs:domain>
        <rdfs:range rdf:resource="http://purl.org/ica/ric#RiC-E4-Agent"/>
        <rdfs:comment xml:lang="en">Relations RiC-R27, RiC-R156</rdfs:comment>
        <rdfs:label xml:lang="en">was addressed to</rdfs:label>
    </owl:ObjectProperty>
    


    <!-- http://purl.org/ica/ric#RiC-R-wasAddresseeOf -->

    <owl:ObjectProperty rdf:about="http://purl.org/ica/ric#RiC-R-wasAddresseeOf">
        <rdfs:domain rdf:resource="http://purl.org/ica/ric#RiC-E4-Agent"/>
        <rdfs:range>
            <owl:Class>
                <owl:unionOf rdf:parseType="Collection">
                    <rdf:Description rdf:about="http://purl.org/ica/ric#RiC-E1-Record"/>
                    <rdf:Description rdf:about="http://purl.org/ica/ric#RiC-E3-RecordSet"/>
                </owl:unionOf>
            </owl:Class>
        </rdfs:range>
        <rdfs:comment xml:lang="en">Relations RiC-R214, RiC-R246</rdfs:comment>
        <rdfs:label xml:lang="en">was addressee of</rdfs:label>
    </owl:ObjectProperty>
    


    <!-- http://purl.org/ica/ric#RiC-R-wasArrangedBy -->

    <owl:ObjectProperty rdf:about="http://purl.org/ica/ric#RiC-R-wasArrangedBy">
        <rdfs:domain rdf:resource="http://purl.org/ica/ric#RiC-E3-RecordSet"/>
        <rdfs:range rdf:resource="http://purl.org/ica/ric#RiC-E4-Agent"/>
        <rdfs:comment xml:lang="en">Relations RiC-R157</rdfs:comment>
        <rdfs:label xml:lang="en">was arranged by</rdfs:label>
    </owl:ObjectProperty>
    


    <!-- http://purl.org/ica/ric#RiC-R-wasAssembledBy -->

    <owl:ObjectProperty rdf:about="http://purl.org/ica/ric#RiC-R-wasAssembledBy">
        <rdfs:domain rdf:resource="http://purl.org/ica/ric#RiC-E3-RecordSet"/>
        <rdfs:range rdf:resource="http://purl.org/ica/ric#RiC-E4-Agent"/>
        <rdfs:comment xml:lang="en">Relations RiC-R158</rdfs:comment>
        <rdfs:label xml:lang="en">was assembled by</rdfs:label>
    </owl:ObjectProperty>
    


    <!-- http://purl.org/ica/ric#RiC-R-wasAssociatedWith -->

    <owl:ObjectProperty rdf:about="http://purl.org/ica/ric#RiC-R-wasAssociatedWith">
        <rdf:type rdf:resource="http://www.w3.org/2002/07/owl#SymmetricProperty"/>
        <rdfs:domain>
            <owl:Class>
                <owl:unionOf rdf:parseType="Collection">
                    <rdf:Description rdf:about="http://purl.org/ica/ric#RiC-E1-Record"/>
                    <rdf:Description rdf:about="http://purl.org/ica/ric#RiC-E10-Mandate"/>
                    <rdf:Description rdf:about="http://purl.org/ica/ric#RiC-E11-DocumentaryForm"/>
                    <rdf:Description rdf:about="http://purl.org/ica/ric#RiC-E12-Date"/>
                    <rdf:Description rdf:about="http://purl.org/ica/ric#RiC-E13-Place"/>
                    <rdf:Description rdf:about="http://purl.org/ica/ric#RiC-E14-ConceptThing"/>
                    <rdf:Description rdf:about="http://purl.org/ica/ric#RiC-E2-RecordComponent"/>
                    <rdf:Description rdf:about="http://purl.org/ica/ric#RiC-E3-RecordSet"/>
                    <rdf:Description rdf:about="http://purl.org/ica/ric#RiC-E4-Agent"/>
                    <rdf:Description rdf:about="http://purl.org/ica/ric#RiC-E5-Occupation"/>
                    <rdf:Description rdf:about="http://purl.org/ica/ric#RiC-E6-Position"/>
                    <rdf:Description rdf:about="http://purl.org/ica/ric#RiC-E7-Function"/>
                    <rdf:Description rdf:about="http://purl.org/ica/ric#RiC-E8-FunctionAbstract"/>
                    <rdf:Description rdf:about="http://purl.org/ica/ric#RiC-E9-Activity"/>
                </owl:unionOf>
            </owl:Class>
        </rdfs:domain>
        <rdfs:range>
            <owl:Class>
                <owl:unionOf rdf:parseType="Collection">
                    <rdf:Description rdf:about="http://purl.org/ica/ric#RiC-E1-Record"/>
                    <rdf:Description rdf:about="http://purl.org/ica/ric#RiC-E10-Mandate"/>
                    <rdf:Description rdf:about="http://purl.org/ica/ric#RiC-E11-DocumentaryForm"/>
                    <rdf:Description rdf:about="http://purl.org/ica/ric#RiC-E12-Date"/>
                    <rdf:Description rdf:about="http://purl.org/ica/ric#RiC-E13-Place"/>
                    <rdf:Description rdf:about="http://purl.org/ica/ric#RiC-E14-ConceptThing"/>
                    <rdf:Description rdf:about="http://purl.org/ica/ric#RiC-E2-RecordComponent"/>
                    <rdf:Description rdf:about="http://purl.org/ica/ric#RiC-E3-RecordSet"/>
                    <rdf:Description rdf:about="http://purl.org/ica/ric#RiC-E4-Agent"/>
                    <rdf:Description rdf:about="http://purl.org/ica/ric#RiC-E5-Occupation"/>
                    <rdf:Description rdf:about="http://purl.org/ica/ric#RiC-E6-Position"/>
                    <rdf:Description rdf:about="http://purl.org/ica/ric#RiC-E7-Function"/>
                    <rdf:Description rdf:about="http://purl.org/ica/ric#RiC-E8-FunctionAbstract"/>
                    <rdf:Description rdf:about="http://purl.org/ica/ric#RiC-E9-Activity"/>
                </owl:unionOf>
            </owl:Class>
        </rdfs:range>
        <rdfs:comment xml:lang="en">Relations RiC-R12, RiC-R16, RiC-R19, RiC-R28, RiC-R39, RiC-R43, RiC-R47, RiC-R50, RiC-R54, RiC-R58, RiC-R61, RiC-R64, RiC-R69, RiC-R73, RiC-R76, RiC-R81, RiC-R83, RiC-R90, RiC-R100, RiC-R104, RiC-R108, RiC-R111, RiC-R115, RiC-R118, RiC-R121, RiC-R124, RiC-R129, RiC-R133, RiC-R137, RiC-R139, RiC-R146, RiC-R159, RiC-R169, RiC-R173, RiC-R177, RiC-R180, RiC-R184, RiC-R188, RiC-R190, RiC-R194, RiC-R199, RiC-R203, RiC-R215, RiC-R228, RiC-R247, RiC-R278, RiC-R295, RiC-R300, RiC-R304, RiC-R306, RiC-R310, RiC-R312, RiC-R315, RiC-R324, RiC-R330, RiC-R334, RiC-R338, RiC-R342, RiC-R346, RiC-R349, RiC-R354, RiC-R357, RiC-R360, RiC-R362, RiC-R364, RiC-R366, RiC-R368, RiC-R370, RiC-R372, RiC-R374, RiC-R378, RiC-R382, RiC-R386, RiC-R389, RiC-R395, RiC-R399, RiC-R401, RiC-R403, RiC-R405, RiC-R408, RiC-R412, RiC-R417, RiC-R420, RiC-R423, RiC-R427, RiC-R431, RiC-R435, RiC-R438, RiC-R441, RiC-R443, RiC-R450, RiC-R454, RiC-R457, RiC-R461, RiC-R465, RiC-R472, RiC-R474, RiC-R476, RiC-R479, RiC-R482, RiC-R485, RiC-R487, RiC-R489, RiC-R491, RiC-R494, RiC-R496, RiC-R498, RiC-R500, RiC-R502, RiC-R504, RiC-R506, RiC-R508, RiC-R512, RiC-R516, RiC-R520, RiC-R523, RiC-R526, RiC-R528, RiC-R531, RiC-R534, RiC-R541, RiC-R545, RiC-R549, RiC-R556, RiC-R558, RiC-R560, RiC-R564, RiC-R567, RiC-R571, RiC-R574, RiC-R576, RiC-R581, RiC-R586, RiC-R588, RiC-R593, RiC-R597, RiC-R599, RiC-R607, RiC-R611, RiC-R613, RiC-R616, RiC-R619, RiC-R621, RiC-R623, RiC-R625, RiC-R627, RiC-R629, RiC-R631, RiC-R633, RiC-R635, RiC-R637, RiC-R639, RiC-R641, RiC-R643, RiC-R645, RiC-R648, RiC-R652, RiC-R658, RiC-R664, RiC-R667, RiC-R674, RiC-R678, RiC-R683, RiC-R690, RiC-R695, RiC-R697, RiC-R702, RiC-R706, RiC-R710, RiC-R716, RiC-R722, RiC-R729, RiC-R734, RiC-R737, RiC-R740, RiC-R742, RiC-R744, RiC-R747, RiC-R750, RiC-R757, RiC-R759, RiC-R761, RiC-R764, RiC-R767, RiC-R770, RiC-R772, RiC-R774, RiC-R776, RiC-R778, RiC-R780, RiC-R782, RiC-R784, RiC-R786, RiC-R788, RiC-R790, RiC-R792</rdfs:comment>
        <rdfs:label xml:lang="en">was associated with</rdfs:label>
        <rdfs:seeAlso rdf:resource="http://purl.org/ica/ric#RiC-R-isAssociatedWith"/>
    </owl:ObjectProperty>
    


    <!-- http://purl.org/ica/ric#RiC-R-wasAuthoredBy -->

    <owl:ObjectProperty rdf:about="http://purl.org/ica/ric#RiC-R-wasAuthoredBy">
        <rdfs:domain>
            <owl:Class>
                <owl:unionOf rdf:parseType="Collection">
                    <rdf:Description rdf:about="http://purl.org/ica/ric#RiC-E1-Record"/>
                    <rdf:Description rdf:about="http://purl.org/ica/ric#RiC-E2-RecordComponent"/>
                </owl:unionOf>
            </owl:Class>
        </rdfs:domain>
        <rdfs:range rdf:resource="http://purl.org/ica/ric#RiC-E4-Agent"/>
        <rdfs:comment xml:lang="en">Relations RiC-R29, RiC-R91</rdfs:comment>
        <rdfs:label xml:lang="en">was authored by</rdfs:label>
    </owl:ObjectProperty>
    


    <!-- http://purl.org/ica/ric#RiC-R-wasAuthorizedBy -->

    <owl:ObjectProperty rdf:about="http://purl.org/ica/ric#RiC-R-wasAuthorizedBy">
        <rdfs:domain rdf:resource="http://purl.org/ica/ric#RiC-E4-Agent"/>
        <rdfs:range rdf:resource="http://purl.org/ica/ric#RiC-E10-Mandate"/>
        <rdfs:comment xml:lang="en">Relations RiC-R313</rdfs:comment>
        <rdfs:label xml:lang="en">was authorized by</rdfs:label>
    </owl:ObjectProperty>
    


    <!-- http://purl.org/ica/ric#RiC-R-wasBirthDateOf -->

    <owl:ObjectProperty rdf:about="http://purl.org/ica/ric#RiC-R-wasBirthDateOf">
        <rdfs:domain rdf:resource="http://purl.org/ica/ric#RiC-E12-Date"/>
        <rdfs:range rdf:resource="http://purl.org/ica/ric#RiC-E4-Agent-Person"/>
        <rdfs:comment xml:lang="en">Relations RiC-R659</rdfs:comment>
        <rdfs:label xml:lang="en">was birth date of</rdfs:label>
    </owl:ObjectProperty>
    


    <!-- http://purl.org/ica/ric#RiC-R-wasBirthPlaceOf -->

    <owl:ObjectProperty rdf:about="http://purl.org/ica/ric#RiC-R-wasBirthPlaceOf">
        <rdfs:domain rdf:resource="http://purl.org/ica/ric#RiC-E13-Place"/>
        <rdfs:range rdf:resource="http://purl.org/ica/ric#RiC-E4-Agent-Person"/>
        <rdfs:comment xml:lang="en">Relations RiC-R730</rdfs:comment>
        <rdfs:label xml:lang="en">was birth place of</rdfs:label>
    </owl:ObjectProperty>
    


    <!-- http://purl.org/ica/ric#RiC-R-wasChildOf -->

    <owl:ObjectProperty rdf:about="http://purl.org/ica/ric#RiC-R-wasChildOf">
        <owl:inverseOf rdf:resource="http://purl.org/ica/ric#RiC-R-wasParentOf"/>
        <rdfs:domain rdf:resource="http://purl.org/ica/ric#RiC-E4-Agent-Person"/>
        <rdfs:range rdf:resource="http://purl.org/ica/ric#RiC-E4-Agent-Person"/>
        <rdfs:comment xml:lang="en">Relations RiC-R279</rdfs:comment>
        <rdfs:label xml:lang="en">was child of</rdfs:label>
        <rdfs:seeAlso rdf:resource="http://purl.org/ica/ric#RiC-R-isChildOf"/>
    </owl:ObjectProperty>
    


    <!-- http://purl.org/ica/ric#RiC-R-wasCitizenOf -->

    <owl:ObjectProperty rdf:about="http://purl.org/ica/ric#RiC-R-wasCitizenOf">
        <rdfs:domain rdf:resource="http://purl.org/ica/ric#RiC-E4-Agent-Person"/>
        <rdfs:range rdf:resource="http://purl.org/ica/ric#RiC-E13-Place"/>
        <rdfs:comment xml:lang="en">Relations RiC-R331</rdfs:comment>
        <rdfs:label xml:lang="en">was citizen of</rdfs:label>
        <rdfs:seeAlso rdf:resource="http://purl.org/ica/ric#RiC-R-isCitizenOf"/>
    </owl:ObjectProperty>
    


    <!-- http://purl.org/ica/ric#RiC-R-wasCollectedBy -->

    <owl:ObjectProperty rdf:about="http://purl.org/ica/ric#RiC-R-wasCollectedBy">
        <rdfs:domain>
            <owl:Class>
                <owl:unionOf rdf:parseType="Collection">
                    <rdf:Description rdf:about="http://purl.org/ica/ric#RiC-E1-Record"/>
                    <rdf:Description rdf:about="http://purl.org/ica/ric#RiC-E2-RecordComponent"/>
                    <rdf:Description rdf:about="http://purl.org/ica/ric#RiC-E3-RecordSet"/>
                </owl:unionOf>
            </owl:Class>
        </rdfs:domain>
        <rdfs:range rdf:resource="http://purl.org/ica/ric#RiC-E4-Agent"/>
        <rdfs:comment xml:lang="en">Relations RiC-R30, RiC-R92, RiC-R160</rdfs:comment>
        <rdfs:label xml:lang="en">was collected by</rdfs:label>
    </owl:ObjectProperty>
    


    <!-- http://purl.org/ica/ric#RiC-R-wasControlledBy -->

    <owl:ObjectProperty rdf:about="http://purl.org/ica/ric#RiC-R-wasControlledBy">
        <rdfs:domain rdf:resource="http://purl.org/ica/ric#RiC-E4-Agent"/>
        <rdfs:range rdf:resource="http://purl.org/ica/ric#RiC-E4-Agent"/>
        <rdfs:comment xml:lang="en">Relations RiC-R280</rdfs:comment>
        <rdfs:label xml:lang="en">was controlled by</rdfs:label>
        <rdfs:seeAlso rdf:resource="http://purl.org/ica/ric#RiC-R-isControlledBy"/>
    </owl:ObjectProperty>
    


    <!-- http://purl.org/ica/ric#RiC-R-wasCreatedAt -->

    <owl:ObjectProperty rdf:about="http://purl.org/ica/ric#RiC-R-wasCreatedAt">
        <owl:inverseOf rdf:resource="http://purl.org/ica/ric#RiC-R-wasCreationLocationOfPlaceOf"/>
        <rdfs:domain>
            <owl:Class>
                <owl:unionOf rdf:parseType="Collection">
                    <rdf:Description rdf:about="http://purl.org/ica/ric#RiC-E1-Record"/>
                    <rdf:Description rdf:about="http://purl.org/ica/ric#RiC-E2-RecordComponent"/>
                    <rdf:Description rdf:about="http://purl.org/ica/ric#RiC-E3-RecordSet"/>
                </owl:unionOf>
            </owl:Class>
        </rdfs:domain>
        <rdfs:range rdf:resource="http://purl.org/ica/ric#RiC-E13-Place"/>
        <rdfs:comment xml:lang="en">Relations RiC-R70, RiC-R130, RiC-R200</rdfs:comment>
        <rdfs:label xml:lang="en">was created at</rdfs:label>
    </owl:ObjectProperty>
    


    <!-- http://purl.org/ica/ric#RiC-R-wasCreatedBy -->

    <owl:ObjectProperty rdf:about="http://purl.org/ica/ric#RiC-R-wasCreatedBy">
        <rdfs:domain>
            <owl:Class>
                <owl:unionOf rdf:parseType="Collection">
                    <rdf:Description rdf:about="http://purl.org/ica/ric#RiC-E1-Record"/>
                    <rdf:Description rdf:about="http://purl.org/ica/ric#RiC-E2-RecordComponent"/>
                    <rdf:Description rdf:about="http://purl.org/ica/ric#RiC-E3-RecordSet"/>
                    <rdf:Description rdf:about="http://purl.org/ica/ric#RiC-E4-Agent-DelegateAgent"/>
                </owl:unionOf>
            </owl:Class>
        </rdfs:domain>
        <rdfs:range rdf:resource="http://purl.org/ica/ric#RiC-E4-Agent"/>
        <rdfs:comment xml:lang="en">Relations RiC-R31, RiC-R93, RiC-R161, RiC-R281</rdfs:comment>
        <rdfs:label xml:lang="en">was created by</rdfs:label>
    </owl:ObjectProperty>
    


    <!-- http://purl.org/ica/ric#RiC-R-wasCreationDateOf -->

    <owl:ObjectProperty rdf:about="http://purl.org/ica/ric#RiC-R-wasCreationDateOf">
        <rdfs:domain rdf:resource="http://purl.org/ica/ric#RiC-E12-Date"/>
        <rdfs:range>
            <owl:Class>
                <owl:unionOf rdf:parseType="Collection">
                    <rdf:Description rdf:about="http://purl.org/ica/ric#RiC-E1-Record"/>
                    <rdf:Description rdf:about="http://purl.org/ica/ric#RiC-E2-RecordComponent"/>
                    <rdf:Description rdf:about="http://purl.org/ica/ric#RiC-E3-RecordSet"/>
                </owl:unionOf>
            </owl:Class>
        </rdfs:range>
        <rdfs:comment xml:lang="en">Relations RiC-R646, RiC-R649, RiC-R653</rdfs:comment>
        <rdfs:label xml:lang="en">was creation date of</rdfs:label>
    </owl:ObjectProperty>
    


    <!-- http://purl.org/ica/ric#RiC-R-wasCreationLocationOfPlaceOf -->

    <owl:ObjectProperty rdf:about="http://purl.org/ica/ric#RiC-R-wasCreationLocationOfPlaceOf">
        <rdfs:domain rdf:resource="http://purl.org/ica/ric#RiC-E13-Place"/>
        <rdfs:range>
            <owl:Class>
                <owl:unionOf rdf:parseType="Collection">
                    <rdf:Description rdf:about="http://purl.org/ica/ric#RiC-E1-Record"/>
                    <rdf:Description rdf:about="http://purl.org/ica/ric#RiC-E2-RecordComponent"/>
                    <rdf:Description rdf:about="http://purl.org/ica/ric#RiC-E3-RecordSet"/>
                </owl:unionOf>
            </owl:Class>
        </rdfs:range>
        <rdfs:comment xml:lang="en">Relations RiC-R711, RiC-R717</rdfs:comment>
        <rdfs:label xml:lang="en">was creation location of / was creation place of</rdfs:label>
    </owl:ObjectProperty>
    


    <!-- http://purl.org/ica/ric#RiC-R-wasDeathDateOf -->

    <owl:ObjectProperty rdf:about="http://purl.org/ica/ric#RiC-R-wasDeathDateOf">
        <rdfs:domain rdf:resource="http://purl.org/ica/ric#RiC-E12-Date"/>
        <rdfs:range rdf:resource="http://purl.org/ica/ric#RiC-E4-Agent-Person"/>
        <rdfs:comment xml:lang="en">Relations RiC-R660</rdfs:comment>
        <rdfs:label xml:lang="en">was death date of</rdfs:label>
    </owl:ObjectProperty>
    


    <!-- http://purl.org/ica/ric#RiC-R-wasDeathPlaceOf -->

    <owl:ObjectProperty rdf:about="http://purl.org/ica/ric#RiC-R-wasDeathPlaceOf">
        <rdfs:domain rdf:resource="http://purl.org/ica/ric#RiC-E13-Place"/>
        <rdfs:range rdf:resource="http://purl.org/ica/ric#RiC-E4-Agent-Person"/>
        <rdfs:comment xml:lang="en">Relations RiC-R731</rdfs:comment>
        <rdfs:label xml:lang="en">was death place of</rdfs:label>
    </owl:ObjectProperty>
    


    <!-- http://purl.org/ica/ric#RiC-R-wasDefinedBy -->

    <owl:ObjectProperty rdf:about="http://purl.org/ica/ric#RiC-R-wasDefinedBy">
        <rdfs:domain>
            <owl:Class>
                <owl:unionOf rdf:parseType="Collection">
                    <rdf:Description rdf:about="http://purl.org/ica/ric#RiC-E6-Position"/>
                    <rdf:Description rdf:about="http://purl.org/ica/ric#RiC-E7-Function"/>
                    <rdf:Description rdf:about="http://purl.org/ica/ric#RiC-E9-Activity"/>
                </owl:unionOf>
            </owl:Class>
        </rdfs:domain>
        <rdfs:range rdf:resource="http://purl.org/ica/ric#RiC-E10-Mandate"/>
        <rdfs:comment xml:lang="en">Relations RiC-R409, RiC-R462, RiC-R546</rdfs:comment>
        <rdfs:label xml:lang="en">was defined by</rdfs:label>
        <rdfs:seeAlso rdf:resource="http://purl.org/ica/ric#RiC-R-isDefinedBy"/>
    </owl:ObjectProperty>
    


    <!-- http://purl.org/ica/ric#RiC-R-wasDirectedBy -->

    <owl:ObjectProperty rdf:about="http://purl.org/ica/ric#RiC-R-wasDirectedBy">
        <owl:inverseOf rdf:resource="http://purl.org/ica/ric#RiC-R-wasDirectorOf"/>
        <rdfs:range rdf:resource="http://purl.org/ica/ric#RiC-E4-Agent-Person"/>
        <rdfs:comment xml:lang="en">Relations RiC-R282</rdfs:comment>
        <rdfs:label xml:lang="en">was directed by</rdfs:label>
        <rdfs:seeAlso rdf:resource="http://purl.org/ica/ric#RiC-R-isDirectedBy"/>
    </owl:ObjectProperty>
    


    <!-- http://purl.org/ica/ric#RiC-R-wasDirectorOf -->

    <owl:ObjectProperty rdf:about="http://purl.org/ica/ric#RiC-R-wasDirectorOf">
        <rdfs:domain rdf:resource="http://purl.org/ica/ric#RiC-E4-Agent-Person"/>
        <rdfs:comment xml:lang="en">Relations RiC-R283</rdfs:comment>
        <rdfs:label xml:lang="en">was director of</rdfs:label>
        <rdfs:seeAlso rdf:resource="http://purl.org/ica/ric#RiC-R-isDirectorOf"/>
    </owl:ObjectProperty>
    


    <!-- http://purl.org/ica/ric#RiC-R-wasEndDateOf -->

    <owl:ObjectProperty rdf:about="http://purl.org/ica/ric#RiC-R-wasEndDateOf">
        <rdfs:domain rdf:resource="http://purl.org/ica/ric#RiC-E12-Date"/>
        <rdfs:range>
            <owl:Class>
                <owl:unionOf rdf:parseType="Collection">
                    <rdf:Description rdf:about="http://purl.org/ica/ric#RiC-E10-Mandate"/>
                    <rdf:Description rdf:about="http://purl.org/ica/ric#RiC-E13-Place"/>
                    <rdf:Description rdf:about="http://purl.org/ica/ric#RiC-E4-Agent-Group"/>
                    <rdf:Description rdf:about="http://purl.org/ica/ric#RiC-E6-Position"/>
                    <rdf:Description rdf:about="http://purl.org/ica/ric#RiC-E7-Function"/>
                    <rdf:Description rdf:about="http://purl.org/ica/ric#RiC-E9-Activity"/>
                </owl:unionOf>
            </owl:Class>
        </rdfs:range>
        <rdfs:comment xml:lang="en">Relations RiC-R661, RiC-R668, RiC-R675, RiC-R684, RiC-R691, RiC-R703</rdfs:comment>
        <rdfs:label xml:lang="en">was end date of</rdfs:label>
        <rdfs:seeAlso rdf:resource="http://purl.org/ica/ric#RiC-R-isEndDateOf"/>
    </owl:ObjectProperty>
    


    <!-- http://purl.org/ica/ric#RiC-R-wasEstablishedBy -->

    <owl:ObjectProperty rdf:about="http://purl.org/ica/ric#RiC-R-wasEstablishedBy">
        <rdfs:domain rdf:resource="http://purl.org/ica/ric#RiC-E6-Position"/>
        <rdfs:range rdf:resource="http://purl.org/ica/ric#RiC-E4-Agent-Group"/>
        <rdfs:comment xml:lang="en">Relations RiC-R390</rdfs:comment>
        <rdfs:label xml:lang="en">was established by</rdfs:label>
    </owl:ObjectProperty>
    


    <!-- http://purl.org/ica/ric#RiC-R-wasFulfilledBy -->

    <owl:ObjectProperty rdf:about="http://purl.org/ica/ric#RiC-R-wasFulfilledBy">
        <rdfs:domain rdf:resource="http://purl.org/ica/ric#RiC-E7-Function"/>
        <rdfs:range rdf:resource="http://purl.org/ica/ric#RiC-E4-Agent"/>
        <rdfs:comment xml:lang="en">Relations RiC-R439</rdfs:comment>
        <rdfs:label xml:lang="en">was fulfilled by</rdfs:label>
        <rdfs:seeAlso rdf:resource="http://purl.org/ica/ric#RiC-R-isFulfilledBy"/>
    </owl:ObjectProperty>
    


    <!-- http://purl.org/ica/ric#RiC-R-wasFulfilledByPerformanceOf -->

    <owl:ObjectProperty rdf:about="http://purl.org/ica/ric#RiC-R-wasFulfilledByPerformanceOf">
        <owl:inverseOf rdf:resource="http://purl.org/ica/ric#RiC-R-wasPerformedToFulfill"/>
        <rdfs:domain rdf:resource="http://purl.org/ica/ric#RiC-E7-Function"/>
        <rdfs:range rdf:resource="http://purl.org/ica/ric#RiC-E9-Activity"/>
        <rdfs:comment xml:lang="en">Relations RiC-R458</rdfs:comment>
        <rdfs:label xml:lang="en">was fulfilled by performance of</rdfs:label>
        <rdfs:seeAlso rdf:resource="http://purl.org/ica/ric#RiC-R-isFulfilledByPerformanceOf"/>
    </owl:ObjectProperty>
    


    <!-- http://purl.org/ica/ric#RiC-R-wasHeldBy -->

    <owl:ObjectProperty rdf:about="http://purl.org/ica/ric#RiC-R-wasHeldBy">
        <owl:inverseOf rdf:resource="http://purl.org/ica/ric#RiC-R-wasHolderOf"/>
        <rdfs:domain>
            <owl:Class>
                <owl:unionOf rdf:parseType="Collection">
                    <rdf:Description rdf:about="http://purl.org/ica/ric#RiC-E1-Record"/>
                    <rdf:Description rdf:about="http://purl.org/ica/ric#RiC-E2-RecordComponent"/>
                    <rdf:Description rdf:about="http://purl.org/ica/ric#RiC-E3-RecordSet"/>
                </owl:unionOf>
            </owl:Class>
        </rdfs:domain>
        <rdfs:range rdf:resource="http://purl.org/ica/ric#RiC-E4-Agent"/>
        <rdfs:comment xml:lang="en">Relations RiC-R32, RiC-R94, RiC-R162</rdfs:comment>
        <rdfs:label xml:lang="en">was held by</rdfs:label>
        <rdfs:seeAlso rdf:resource="http://purl.org/ica/ric#RiC-R-isHeldBy"/>
    </owl:ObjectProperty>
    


    <!-- http://purl.org/ica/ric#RiC-R-wasHolderOf -->

    <owl:ObjectProperty rdf:about="http://purl.org/ica/ric#RiC-R-wasHolderOf">
        <rdfs:domain rdf:resource="http://purl.org/ica/ric#RiC-E4-Agent"/>
        <rdfs:range>
            <owl:Class>
                <owl:unionOf rdf:parseType="Collection">
                    <rdf:Description rdf:about="http://purl.org/ica/ric#RiC-E1-Record"/>
                    <rdf:Description rdf:about="http://purl.org/ica/ric#RiC-E2-RecordComponent"/>
                    <rdf:Description rdf:about="http://purl.org/ica/ric#RiC-E3-RecordSet"/>
                </owl:unionOf>
            </owl:Class>
        </rdfs:range>
        <rdfs:comment xml:lang="en">Relations RiC-R216, RiC-R229, RiC-R248</rdfs:comment>
        <rdfs:label xml:lang="en">was holder of</rdfs:label>
        <rdfs:seeAlso rdf:resource="http://purl.org/ica/ric#RiC-R-isHolderOf"/>
    </owl:ObjectProperty>
    


    <!-- http://purl.org/ica/ric#RiC-R-wasHoldingLocationPlaceOf -->

    <owl:ObjectProperty rdf:about="http://purl.org/ica/ric#RiC-R-wasHoldingLocationPlaceOf">
        <rdfs:domain rdf:resource="http://purl.org/ica/ric#RiC-E13-Place"/>
        <rdfs:range>
            <owl:Class>
                <owl:unionOf rdf:parseType="Collection">
                    <rdf:Description rdf:about="http://purl.org/ica/ric#RiC-E1-Record"/>
                    <rdf:Description rdf:about="http://purl.org/ica/ric#RiC-E2-RecordComponent"/>
                    <rdf:Description rdf:about="http://purl.org/ica/ric#RiC-E3-RecordSet"/>
                </owl:unionOf>
            </owl:Class>
        </rdfs:range>
        <rdfs:comment xml:lang="en">Relations RiC-R712, RiC-R718, RiC-724</rdfs:comment>
        <rdfs:label xml:lang="en">was holding location of / was holding place of</rdfs:label>
        <rdfs:seeAlso rdf:resource="http://purl.org/ica/ric#RiC-R-isHoldingLocationOf"/>
    </owl:ObjectProperty>
    


    <!-- http://purl.org/ica/ric#RiC-R-wasJurisdictionOf -->

    <owl:ObjectProperty rdf:about="http://purl.org/ica/ric#RiC-R-wasJurisdictionOf">
        <rdfs:domain rdf:resource="http://purl.org/ica/ric#RiC-E13-Place"/>
        <rdfs:range rdf:resource="http://purl.org/ica/ric#RiC-E10-Mandate"/>
        <rdfs:comment xml:lang="en">Relations RiC-R748</rdfs:comment>
        <rdfs:label xml:lang="en">was jurisdiction of</rdfs:label>
        <rdfs:seeAlso rdf:resource="http://purl.org/ica/ric#RiC-R-isJurisdictionOf"/>
    </owl:ObjectProperty>
    


    <!-- http://purl.org/ica/ric#RiC-R-wasLocatedAtIn -->

    <owl:ObjectProperty rdf:about="http://purl.org/ica/ric#RiC-R-wasLocatedAtIn">
        <owl:inverseOf rdf:resource="http://purl.org/ica/ric#RiC-R-wasLocationOf"/>
        <rdfs:domain>
            <owl:Class>
                <owl:unionOf rdf:parseType="Collection">
                    <rdf:Description rdf:about="http://purl.org/ica/ric#RiC-E4-Agent"/>
                    <rdf:Description rdf:about="http://purl.org/ica/ric#RiC-E6-Position"/>
                </owl:unionOf>
            </owl:Class>
        </rdfs:domain>
        <rdfs:range rdf:resource="http://purl.org/ica/ric#RiC-E13-Place"/>
        <rdfs:comment xml:lang="en">Relations RiC-R332, RiC-R421</rdfs:comment>
        <rdfs:label xml:lang="en">was located at / was located in</rdfs:label>
        <rdfs:seeAlso rdf:resource="http://purl.org/ica/ric#RiC-R-isLocatedAt"/>
    </owl:ObjectProperty>
    


    <!-- http://purl.org/ica/ric#RiC-R-wasLocationOf -->

    <owl:ObjectProperty rdf:about="http://purl.org/ica/ric#RiC-R-wasLocationOf">
        <rdfs:domain rdf:resource="http://purl.org/ica/ric#RiC-E13-Place"/>
        <rdfs:range>
            <owl:Class>
                <owl:unionOf rdf:parseType="Collection">
                    <rdf:Description rdf:about="http://purl.org/ica/ric#RiC-E4-Agent"/>
                    <rdf:Description rdf:about="http://purl.org/ica/ric#RiC-E6-Position"/>
                </owl:unionOf>
            </owl:Class>
        </rdfs:range>
        <rdfs:comment xml:lang="en">Relations RiC-R732, RiC-R738</rdfs:comment>
        <rdfs:label xml:lang="en">was location of</rdfs:label>
        <rdfs:seeAlso rdf:resource="http://purl.org/ica/ric#RiC-R-isLocationOf"/>
    </owl:ObjectProperty>
    


    <!-- http://purl.org/ica/ric#RiC-R-wasManagedBy -->

    <owl:ObjectProperty rdf:about="http://purl.org/ica/ric#RiC-R-wasManagedBy">
        <rdfs:domain rdf:resource="http://purl.org/ica/ric#RiC-E3-RecordSet"/>
        <rdfs:range rdf:resource="http://purl.org/ica/ric#RiC-E4-Agent"/>
        <rdfs:comment xml:lang="en">Relations RiC-R163</rdfs:comment>
        <rdfs:label xml:lang="en">was managed by</rdfs:label>
        <rdfs:seeAlso rdf:resource="http://purl.org/ica/ric#RiC-R-isManagedBy"/>
    </owl:ObjectProperty>
    


    <!-- http://purl.org/ica/ric#RiC-R-wasMemberOf -->

    <owl:ObjectProperty rdf:about="http://purl.org/ica/ric#RiC-R-wasMemberOf">
        <rdfs:domain>
            <owl:Class>
                <owl:unionOf rdf:parseType="Collection">
                    <rdf:Description rdf:about="http://purl.org/ica/ric#RiC-E1-Record"/>
                    <rdf:Description rdf:about="http://purl.org/ica/ric#RiC-E3-RecordSet"/>
                    <rdf:Description rdf:about="http://purl.org/ica/ric#RiC-E4-Agent"/>
                </owl:unionOf>
            </owl:Class>
        </rdfs:domain>
        <rdfs:range>
            <owl:Class>
                <owl:unionOf rdf:parseType="Collection">
                    <rdf:Description rdf:about="http://purl.org/ica/ric#RiC-E3-RecordSet"/>
                    <rdf:Description rdf:about="http://purl.org/ica/ric#RiC-E4-Agent-Group"/>
                </owl:unionOf>
            </owl:Class>
        </rdfs:range>
        <rdfs:comment xml:lang="en">Relations RiC-R20, RiC-R147, RiC-R284</rdfs:comment>
        <rdfs:label xml:lang="en">was member of</rdfs:label>
        <rdfs:seeAlso rdf:resource="http://purl.org/ica/ric#RiC-R-isMemberOf"/>
    </owl:ObjectProperty>
    


    <!-- http://purl.org/ica/ric#RiC-R-wasOccupiedBy -->

    <owl:ObjectProperty rdf:about="http://purl.org/ica/ric#RiC-R-wasOccupiedBy">
        <rdfs:domain rdf:resource="http://purl.org/ica/ric#RiC-E6-Position"/>
        <rdfs:range rdf:resource="http://purl.org/ica/ric#RiC-E4-Agent-Person"/>
        <rdfs:comment xml:lang="en">Relations RiC-R391</rdfs:comment>
        <rdfs:label xml:lang="en">was occupied by</rdfs:label>
        <rdfs:seeAlso rdf:resource="http://purl.org/ica/ric#RiC-R-isOccupiedBy"/>
    </owl:ObjectProperty>
    


    <!-- http://purl.org/ica/ric#RiC-R-wasOwnedByOwnerOf -->

    <owl:ObjectProperty rdf:about="http://purl.org/ica/ric#RiC-R-wasOwnedByOwnerOf">
        <rdfs:domain>
            <owl:Class>
                <owl:unionOf rdf:parseType="Collection">
                    <rdf:Description rdf:about="http://purl.org/ica/ric#RiC-E1-Record"/>
                    <rdf:Description rdf:about="http://purl.org/ica/ric#RiC-E2-RecordComponent"/>
                    <rdf:Description rdf:about="http://purl.org/ica/ric#RiC-E3-RecordSet"/>
                </owl:unionOf>
            </owl:Class>
        </rdfs:domain>
        <rdfs:range rdf:resource="http://purl.org/ica/ric#RiC-E4-Agent"/>
        <rdfs:comment xml:lang="en">Relations RiC-R33, RiC-R164, RiC-R95</rdfs:comment>
        <rdfs:label xml:lang="en">was owned by / was owner of</rdfs:label>
        <rdfs:seeAlso rdf:resource="http://purl.org/ica/ric#RiC-R-isOwnedBy"/>
    </owl:ObjectProperty>
    


    <!-- http://purl.org/ica/ric#RiC-R-wasParentOf -->

    <owl:ObjectProperty rdf:about="http://purl.org/ica/ric#RiC-R-wasParentOf">
        <rdfs:domain rdf:resource="http://purl.org/ica/ric#RiC-E4-Agent-Person"/>
        <rdfs:range rdf:resource="http://purl.org/ica/ric#RiC-E4-Agent-Person"/>
        <rdfs:comment xml:lang="en">Relations RiC-R285</rdfs:comment>
        <rdfs:label xml:lang="en">was parent of</rdfs:label>
        <rdfs:seeAlso rdf:resource="http://purl.org/ica/ric#RiC-R-isParentOf"/>
    </owl:ObjectProperty>
    


    <!-- http://purl.org/ica/ric#RiC-R-wasPartOf -->

    <owl:ObjectProperty rdf:about="http://purl.org/ica/ric#RiC-R-wasPartOf">
        <rdfs:domain>
            <owl:Class>
                <owl:unionOf rdf:parseType="Collection">
                    <rdf:Description rdf:about="http://purl.org/ica/ric#RiC-E2-RecordComponent"/>
                    <rdf:Description rdf:about="http://purl.org/ica/ric#RiC-E4-Agent-Group"/>
                    <rdf:Description rdf:about="http://purl.org/ica/ric#RiC-E7-Function"/>
                    <rdf:Description rdf:about="http://purl.org/ica/ric#RiC-E9-Activity"/>
                </owl:unionOf>
            </owl:Class>
        </rdfs:domain>
        <rdfs:range>
            <owl:Class>
                <owl:unionOf rdf:parseType="Collection">
                    <rdf:Description rdf:about="http://purl.org/ica/ric#RiC-E1-Record"/>
                    <rdf:Description rdf:about="http://purl.org/ica/ric#RiC-E4-Agent-Group"/>
                    <rdf:Description rdf:about="http://purl.org/ica/ric#RiC-E7-Function"/>
                    <rdf:Description rdf:about="http://purl.org/ica/ric#RiC-E9-Activity"/>
                </owl:unionOf>
            </owl:Class>
        </rdfs:range>
        <rdfs:comment xml:lang="en">Relations RiC-R77, RiC-R286, RiC-R451, RiC-R542</rdfs:comment>
        <rdfs:label xml:lang="en">was part of</rdfs:label>
        <rdfs:seeAlso rdf:resource="http://purl.org/ica/ric#RiC-R-isPartOf"/>
    </owl:ObjectProperty>
    


    <!-- http://purl.org/ica/ric#RiC-R-wasPerformedBy -->

    <owl:ObjectProperty rdf:about="http://purl.org/ica/ric#RiC-R-wasPerformedBy">
        <rdfs:domain rdf:resource="http://purl.org/ica/ric#RiC-E9-Activity"/>
        <rdfs:range rdf:resource="http://purl.org/ica/ric#RiC-E4-Agent"/>
        <rdfs:comment xml:lang="en">Relations RiC-R524</rdfs:comment>
        <rdfs:label xml:lang="en">was performed by</rdfs:label>
        <rdfs:seeAlso rdf:resource="http://purl.org/ica/ric#RiC-R-isPerformedBy"/>
    </owl:ObjectProperty>
    


    <!-- http://purl.org/ica/ric#RiC-R-wasPerformedToFulfill -->

    <owl:ObjectProperty rdf:about="http://purl.org/ica/ric#RiC-R-wasPerformedToFulfill">
        <rdfs:domain rdf:resource="http://purl.org/ica/ric#RiC-E9-Activity"/>
        <rdfs:range rdf:resource="http://purl.org/ica/ric#RiC-E7-Function"/>
        <rdfs:comment xml:lang="en">Relations RiC-R532</rdfs:comment>
        <rdfs:label xml:lang="en">was performed to fulfill</rdfs:label>
        <rdfs:seeAlso rdf:resource="http://purl.org/ica/ric#RiC-R-isPerformedToFulfil"/>
    </owl:ObjectProperty>
    


    <!-- http://purl.org/ica/ric#RiC-R-wasPursuedBy -->

    <owl:ObjectProperty rdf:about="http://purl.org/ica/ric#RiC-R-wasPursuedBy">
        <rdfs:domain rdf:resource="http://purl.org/ica/ric#RiC-E5-Occupation"/>
        <rdfs:range rdf:resource="http://purl.org/ica/ric#RiC-E4-Agent"/>
        <rdfs:comment xml:lang="en">Relations RiC-R350</rdfs:comment>
        <rdfs:label xml:lang="en">was pursued by</rdfs:label>
        <rdfs:seeAlso rdf:resource="http://purl.org/ica/ric#RiC-R-isPursuedBy"/>
    </owl:ObjectProperty>
    


    <!-- http://purl.org/ica/ric#RiC-R-wasRequiredCompetencyOf -->

    <owl:ObjectProperty rdf:about="http://purl.org/ica/ric#RiC-R-wasRequiredCompetencyOf">
        <rdfs:domain rdf:resource="http://purl.org/ica/ric#RiC-E5-Occupation"/>
        <rdfs:range rdf:resource="http://purl.org/ica/ric#RiC-E6-Position"/>
        <rdfs:comment xml:lang="en">Relations RiC-R358</rdfs:comment>
        <rdfs:label xml:lang="en">was required competency of</rdfs:label>
        <rdfs:seeAlso rdf:resource="http://purl.org/ica/ric#RiC-R-isRequiredCompetencyOf"/>
    </owl:ObjectProperty>
    


    <!-- http://purl.org/ica/ric#RiC-R-wasRevisedBy -->

    <owl:ObjectProperty rdf:about="http://purl.org/ica/ric#RiC-R-wasRevisedBy">
        <rdfs:domain>
            <owl:Class>
                <owl:unionOf rdf:parseType="Collection">
                    <rdf:Description rdf:about="http://purl.org/ica/ric#RiC-E6-Position"/>
                    <rdf:Description rdf:about="http://purl.org/ica/ric#RiC-E7-Function"/>
                    <rdf:Description rdf:about="http://purl.org/ica/ric#RiC-E9-Activity"/>
                </owl:unionOf>
            </owl:Class>
        </rdfs:domain>
        <rdfs:range rdf:resource="http://purl.org/ica/ric#RiC-E10-Mandate"/>
        <rdfs:comment xml:lang="en">Relations RiC-R410, RiC-R463, RiC-R547</rdfs:comment>
        <rdfs:label xml:lang="en">was revised by</rdfs:label>
    </owl:ObjectProperty>
    


    <!-- http://purl.org/ica/ric#RiC-R-wasRevisionDateOf -->

    <owl:ObjectProperty rdf:about="http://purl.org/ica/ric#RiC-R-wasRevisionDateOf">
        <rdfs:domain rdf:resource="http://purl.org/ica/ric#RiC-E12-Date"/>
        <rdfs:range rdf:resource="http://purl.org/ica/ric#RiC-E10-Mandate"/>
        <rdfs:comment xml:lang="en">Relations RiC-R692</rdfs:comment>
        <rdfs:label xml:lang="en">was revision date of</rdfs:label>
    </owl:ObjectProperty>
    


    <!-- http://purl.org/ica/ric#RiC-R-wasRightsHolderOf -->

    <owl:ObjectProperty rdf:about="http://purl.org/ica/ric#RiC-R-wasRightsHolderOf">
        <rdfs:domain rdf:resource="http://purl.org/ica/ric#RiC-E4-Agent"/>
        <rdfs:range>
            <owl:Class>
                <owl:unionOf rdf:parseType="Collection">
                    <rdf:Description rdf:about="http://purl.org/ica/ric#RiC-E1-Record"/>
                    <rdf:Description rdf:about="http://purl.org/ica/ric#RiC-E2-RecordComponent"/>
                    <rdf:Description rdf:about="http://purl.org/ica/ric#RiC-E3-RecordSet"/>
                </owl:unionOf>
            </owl:Class>
        </rdfs:range>
        <rdfs:comment xml:lang="en">Relations RiC-R217, RiC-R230, RiC-R249</rdfs:comment>
        <rdfs:label xml:lang="en">was rights holder of</rdfs:label>
        <rdfs:seeAlso rdf:resource="http://purl.org/ica/ric#RiC-R-isRightsHolderOf"/>
    </owl:ObjectProperty>
    


    <!-- http://purl.org/ica/ric#RiC-R-wasSentBy -->

    <owl:ObjectProperty rdf:about="http://purl.org/ica/ric#RiC-R-wasSentBy">
        <rdfs:domain>
            <owl:Class>
                <owl:unionOf rdf:parseType="Collection">
                    <rdf:Description rdf:about="http://purl.org/ica/ric#RiC-E1-Record"/>
                    <rdf:Description rdf:about="http://purl.org/ica/ric#RiC-E3-RecordSet"/>
                </owl:unionOf>
            </owl:Class>
        </rdfs:domain>
        <rdfs:range rdf:resource="http://purl.org/ica/ric#RiC-E4-Agent"/>
        <rdfs:comment xml:lang="en">Relations RiC-R34, RiC-R165</rdfs:comment>
        <rdfs:label xml:lang="en">was sent by</rdfs:label>
    </owl:ObjectProperty>
    


    <!-- http://purl.org/ica/ric#RiC-R-wasSiblingOf -->

    <owl:ObjectProperty rdf:about="http://purl.org/ica/ric#RiC-R-wasSiblingOf">
        <rdf:type rdf:resource="http://www.w3.org/2002/07/owl#SymmetricProperty"/>
        <rdfs:domain rdf:resource="http://purl.org/ica/ric#RiC-E4-Agent-Person"/>
        <rdfs:range rdf:resource="http://purl.org/ica/ric#RiC-E4-Agent-Person"/>
        <rdfs:comment xml:lang="en">Relations RiC-R287</rdfs:comment>
        <rdfs:label xml:lang="en">was sibling of</rdfs:label>
        <rdfs:seeAlso rdf:resource="http://purl.org/ica/ric#RiC-R-isSiblingOf"/>
    </owl:ObjectProperty>
    


    <!-- http://purl.org/ica/ric#RiC-R-wasSpouseOf -->

    <owl:ObjectProperty rdf:about="http://purl.org/ica/ric#RiC-R-wasSpouseOf">
        <rdf:type rdf:resource="http://www.w3.org/2002/07/owl#SymmetricProperty"/>
        <rdfs:domain rdf:resource="http://purl.org/ica/ric#RiC-E4-Agent-Person"/>
        <rdfs:range rdf:resource="http://purl.org/ica/ric#RiC-E4-Agent-Person"/>
        <rdfs:comment xml:lang="en">Relations RiC-R288</rdfs:comment>
        <rdfs:label xml:lang="en">was spouse of</rdfs:label>
        <rdfs:seeAlso rdf:resource="http://purl.org/ica/ric#RiC-R-isSpouseOf"/>
    </owl:ObjectProperty>
    


    <!-- http://purl.org/ica/ric#RiC-R-wasStartDateOf -->

    <owl:ObjectProperty rdf:about="http://purl.org/ica/ric#RiC-R-wasStartDateOf">
        <rdfs:domain rdf:resource="http://purl.org/ica/ric#RiC-E12-Date"/>
        <rdfs:range>
            <owl:Class>
                <owl:unionOf rdf:parseType="Collection">
                    <rdf:Description rdf:about="http://purl.org/ica/ric#RiC-E10-Mandate"/>
                    <rdf:Description rdf:about="http://purl.org/ica/ric#RiC-E13-Place"/>
                    <rdf:Description rdf:about="http://purl.org/ica/ric#RiC-E4-Agent-Group"/>
                    <rdf:Description rdf:about="http://purl.org/ica/ric#RiC-E6-Position"/>
                    <rdf:Description rdf:about="http://purl.org/ica/ric#RiC-E7-Function"/>
                    <rdf:Description rdf:about="http://purl.org/ica/ric#RiC-E9-Activity"/>
                </owl:unionOf>
            </owl:Class>
        </rdfs:range>
        <rdfs:comment xml:lang="en">Relations RiC-R662, RiC-R669, RiC-R676, RiC-R685, RiC-R693, RiC-R704</rdfs:comment>
        <rdfs:label xml:lang="en">was start date of</rdfs:label>
    </owl:ObjectProperty>
    


    <!-- http://purl.org/ica/ric#RiC-R-wasSubordinateOf -->

    <owl:ObjectProperty rdf:about="http://purl.org/ica/ric#RiC-R-wasSubordinateOf">
        <owl:inverseOf rdf:resource="http://purl.org/ica/ric#RiC-R-wasSuperiorOf"/>
        <rdfs:domain rdf:resource="http://purl.org/ica/ric#RiC-E4-Agent"/>
        <rdfs:range rdf:resource="http://purl.org/ica/ric#RiC-E4-Agent"/>
        <rdfs:comment xml:lang="en">Relations RiC-R289</rdfs:comment>
        <rdfs:label xml:lang="en">was subordinate of</rdfs:label>
        <rdfs:seeAlso rdf:resource="http://purl.org/ica/ric#RiC-R-isSubordinateOf"/>
    </owl:ObjectProperty>
    


    <!-- http://purl.org/ica/ric#RiC-R-wasSuperiorOf -->

    <owl:ObjectProperty rdf:about="http://purl.org/ica/ric#RiC-R-wasSuperiorOf">
        <rdfs:domain rdf:resource="http://purl.org/ica/ric#RiC-E4-Agent"/>
        <rdfs:range rdf:resource="http://purl.org/ica/ric#RiC-E4-Agent"/>
        <rdfs:comment xml:lang="en">Relations RiC-R290</rdfs:comment>
        <rdfs:label xml:lang="en">was superior of</rdfs:label>
        <rdfs:seeAlso rdf:resource="http://purl.org/ica/ric#RiC-R-isSuperiorOf"/>
    </owl:ObjectProperty>
    


    <!-- http://purl.org/ica/ric#RiC-R-wasUsedBy -->

    <owl:ObjectProperty rdf:about="http://purl.org/ica/ric#RiC-R-wasUsedBy">
        <rdfs:domain rdf:resource="http://purl.org/ica/ric#RiC-E4-Agent-DelegateAgent"/>
        <rdfs:range rdf:resource="http://purl.org/ica/ric#RiC-E4-Agent"/>
        <rdfs:comment xml:lang="en">Relations RiC-R291</rdfs:comment>
        <rdfs:label xml:lang="en">was used by</rdfs:label>
        <rdfs:seeAlso rdf:resource="http://purl.org/ica/ric#RiC-R-isUsedBy"/>
    </owl:ObjectProperty>
    


    <!-- http://purl.org/ica/ric#RiC-R-wasWrittenBy -->

    <owl:ObjectProperty rdf:about="http://purl.org/ica/ric#RiC-R-wasWrittenBy">
        <owl:inverseOf rdf:resource="http://purl.org/ica/ric#RiC-R-wrote"/>
        <rdfs:domain>
            <owl:Class>
                <owl:unionOf rdf:parseType="Collection">
                    <rdf:Description rdf:about="http://purl.org/ica/ric#RiC-E1-Record"/>
                    <rdf:Description rdf:about="http://purl.org/ica/ric#RiC-E2-RecordComponent"/>
                </owl:unionOf>
            </owl:Class>
        </rdfs:domain>
        <rdfs:range rdf:resource="http://purl.org/ica/ric#RiC-E4-Agent"/>
        <rdfs:comment xml:lang="en">Relations RiC-R35, RiC-R96</rdfs:comment>
        <rdfs:label xml:lang="en">was written by</rdfs:label>
    </owl:ObjectProperty>
    


    <!-- http://purl.org/ica/ric#RiC-R-wrote -->

    <owl:ObjectProperty rdf:about="http://purl.org/ica/ric#RiC-R-wrote">
        <rdfs:domain rdf:resource="http://purl.org/ica/ric#RiC-E4-Agent"/>
        <rdfs:range>
            <owl:Class>
                <owl:unionOf rdf:parseType="Collection">
                    <rdf:Description rdf:about="http://purl.org/ica/ric#RiC-E1-Record"/>
                    <rdf:Description rdf:about="http://purl.org/ica/ric#RiC-E2-RecordComponent"/>
                </owl:unionOf>
            </owl:Class>
        </rdfs:range>
        <rdfs:comment xml:lang="en">Relations RiC-R218, RiC-R231</rdfs:comment>
        <rdfs:label xml:lang="en">wrote</rdfs:label>
    </owl:ObjectProperty>
    


    <!-- 
    ///////////////////////////////////////////////////////////////////////////////////////
    //
    // Data properties
    //
    ///////////////////////////////////////////////////////////////////////////////////////
     -->

    


    <!-- http://purl.org/ica/ric#RiC-P-OperatingHours -->

    <owl:DatatypeProperty rdf:about="http://purl.org/ica/ric#RiC-P-OperatingHours">
        <rdfs:range rdf:resource="http://www.w3.org/2000/01/rdf-schema#Literal"/>
        <rdfs:comment xml:lang="en">Data Type: Text</rdfs:comment>
        <rdfs:comment xml:lang="en">Property for RiC-P40</rdfs:comment>
        <rdfs:label xml:lang="en">operating hours</rdfs:label>
        <skos:definition xml:lang="en">Days and hours of day during which public services of an Agent are available.</skos:definition>
        <skos:example xml:lang="es">Apertura al público: Lunes a Viernes de 8.00 am - 15.00 pm 
Horas de Apertura Semanales: 35 
Cerrado al público: Sábados y Domingos. Festivos: 1 y 6 de enero, 28 de febrero, Jueves y Viernes Santo, 1 mayo, 30 de mayo, Corpus Christi, 15 de agosto, 1 de noviembre, 6, 8, 24, 25 y 31 de diciembre. 
Spain. Subdirección General de los Archivos Estatales 
Note: For the institution Archivo General de Indias</skos:example>
        <skos:example xml:lang="en">Open: Mon-Fri 9.15-4.45; Sat 9.15-12.30, 1.30-4.30. Late opening Thurs to 7.30 pm 
Closed : One week early December 
United Kingdom, The National Archives 
Note: For the institution West Sussex Record Office</skos:example>
    </owl:DatatypeProperty>
    


    <!-- http://purl.org/ica/ric#RiC-P-accrualNote -->

    <owl:DatatypeProperty rdf:about="http://purl.org/ica/ric#RiC-P-accrualNote">
        <rdfs:domain rdf:resource="http://purl.org/ica/ric#RiC-E3-RecordSet"/>
        <rdfs:range rdf:resource="http://www.w3.org/2000/01/rdf-schema#Literal"/>
        <rdfs:comment xml:lang="en">Data Type: Text</rdfs:comment>
        <rdfs:comment xml:lang="en">Property for RiC-P24</rdfs:comment>
        <rdfs:label xml:lang="en">accrual note</rdfs:label>
        <skos:definition xml:lang="en">Information on anticipated accessions to the Record Set.</skos:definition>
        <skos:example xml:lang="en">There is an agreement with the creator that additional snapshots of their e-mail directory will be accessioned at yearly intervals.</skos:example>
        <skos:scopeNote xml:lang="en">Such accessions may be single Records or Record Sets.</skos:scopeNote>
    </owl:DatatypeProperty>
    


    <!-- http://purl.org/ica/ric#RiC-P-accrualStatus -->

    <owl:DatatypeProperty rdf:about="http://purl.org/ica/ric#RiC-P-accrualStatus"/>
    


    <!-- http://purl.org/ica/ric#RiC-P-address -->

    <owl:DatatypeProperty rdf:about="http://purl.org/ica/ric#RiC-P-address">
        <rdfs:domain rdf:resource="http://purl.org/ica/ric#RiC-E13-Place"/>
        <rdfs:range rdf:resource="http://www.w3.org/2000/01/rdf-schema#Literal"/>
        <rdfs:comment xml:lang="en">Data Type: Text</rdfs:comment>
        <rdfs:comment xml:lang="en">Property for RiC-P65.</rdfs:comment>
        <rdfs:label xml:lang="en">address</rdfs:label>
        <skos:definition xml:lang="en">Physical location of the Place.</skos:definition>
        <skos:example xml:lang="fr">59 rue Guynemer, F-93383 Pierrefitte-sur-Seine Cedex</skos:example>
    </owl:DatatypeProperty>
    


    <!-- http://purl.org/ica/ric#RiC-P-arrangement -->

    <owl:DatatypeProperty rdf:about="http://purl.org/ica/ric#RiC-P-arrangement">
        <rdfs:domain rdf:resource="http://purl.org/ica/ric#RiC-E3-RecordSet"/>
        <rdfs:range rdf:resource="http://www.w3.org/2000/01/rdf-schema#Literal"/>
        <rdfs:comment xml:lang="en">Data Type: Text</rdfs:comment>
        <rdfs:comment xml:lang="en">Property for RiC-P26</rdfs:comment>
        <rdfs:label xml:lang="en">arrangement</rdfs:label>
        <skos:definition xml:lang="en">Criteria and principles used to order the Records or Records Sets within the Record Set.</skos:definition>
        <skos:example xml:lang="en">arranged according to the alphabetical order of the places concerned; arranged chronologically</skos:example>
        <skos:scopeNote xml:lang="en">Encompasses only intellectual arrangement information. Physical arrangement information is out of scope.</skos:scopeNote>
    </owl:DatatypeProperty>
    


    <!-- http://purl.org/ica/ric#RiC-P-authenticityAndIntegrityNote -->

    <owl:DatatypeProperty rdf:about="http://purl.org/ica/ric#RiC-P-authenticityAndIntegrityNote">
        <rdfs:domain>
            <owl:Class>
                <owl:unionOf rdf:parseType="Collection">
                    <rdf:Description rdf:about="http://purl.org/ica/ric#RiC-E1-Record"/>
                    <rdf:Description rdf:about="http://purl.org/ica/ric#RiC-E3-RecordSet"/>
                </owl:unionOf>
            </owl:Class>
        </rdfs:domain>
        <rdfs:range rdf:resource="http://www.w3.org/2000/01/rdf-schema#Literal"/>
        <rdfs:comment xml:lang="en">Data Type: Text</rdfs:comment>
        <rdfs:comment xml:lang="en">Property for RiC-P5, RiC-P22</rdfs:comment>
        <rdfs:label xml:lang="en">authenticity and integrity note</rdfs:label>
        <skos:definition xml:lang="en">Description of features of the Record attesting to how it is genuine, reliable, trustworthy, whole and complete.</skos:definition>
        <skos:example xml:lang="en">the record missing its lower left corner of text and bears the seal of the King the record is electronically signed and the signature is valid at the moment of description; the database (.dbf) file has the checksum SHA-1: bb165836546e13c8d80e97aa44e8f4369608e9f8</skos:example>
    </owl:DatatypeProperty>
    


    <!-- http://purl.org/ica/ric#RiC-P-calendar -->

    <owl:DatatypeProperty rdf:about="http://purl.org/ica/ric#RiC-P-calendar">
        <rdfs:domain rdf:resource="http://purl.org/ica/ric#RiC-E12-Date"/>
        <rdfs:range rdf:resource="http://www.w3.org/2000/01/rdf-schema#Literal"/>
        <rdfs:comment xml:lang="en">Data Type: Text</rdfs:comment>
        <rdfs:comment xml:lang="en">Property for RiC-P62</rdfs:comment>
        <rdfs:label xml:lang="en">calendar</rdfs:label>
        <skos:definition xml:lang="en">Calendar with which the literal expression of the Date (Date as expressed and understood by human Agents) is expressed.</skos:definition>
        <skos:example xml:lang="en">Gregorian; French Revolution calendar</skos:example>
    </owl:DatatypeProperty>
    


    <!-- http://purl.org/ica/ric#RiC-P-classification -->

    <owl:DatatypeProperty rdf:about="http://purl.org/ica/ric#RiC-P-classification"/>
    


    <!-- http://purl.org/ica/ric#RiC-P-conditionsOfAccess -->

    <owl:DatatypeProperty rdf:about="http://purl.org/ica/ric#RiC-P-conditionsOfAccess">
        <rdfs:domain>
            <owl:Class>
                <owl:unionOf rdf:parseType="Collection">
                    <rdf:Description rdf:about="http://purl.org/ica/ric#RiC-E1-Record"/>
                    <rdf:Description rdf:about="http://purl.org/ica/ric#RiC-E3-RecordSet"/>
                </owl:unionOf>
            </owl:Class>
        </rdfs:domain>
        <rdfs:range rdf:resource="http://www.w3.org/2000/01/rdf-schema#Literal"/>
        <rdfs:comment xml:lang="en">Data Type: Text</rdfs:comment>
        <rdfs:comment xml:lang="en">Property for RiC-P18</rdfs:comment>
        <rdfs:label xml:lang="en">conditions of access</rdfs:label>
        <skos:definition xml:lang="en">Conditions affecting the availability of a Record for consultation.</skos:definition>
        <skos:example xml:lang="en">Open; Closed under data protection legislation; Closed as awaiting conservation treatment</skos:example>
        <skos:scopeNote xml:lang="en">Such conditions may be laws, regulations and policies, including policies and  requirements pertaining to privacy, security concerns or restrictions; or they  may pertain to the physical state of the Record, for example, conditions that  require preservation treatment; or they may specify any software/hardware  necessary to access the Record.</skos:scopeNote>
    </owl:DatatypeProperty>
    


    <!-- http://purl.org/ica/ric#RiC-P-conditionsOfUse -->

    <owl:DatatypeProperty rdf:about="http://purl.org/ica/ric#RiC-P-conditionsOfUse">
        <rdfs:domain>
            <owl:Class>
                <owl:unionOf rdf:parseType="Collection">
                    <rdf:Description rdf:about="http://purl.org/ica/ric#RiC-E1-Record"/>
                    <rdf:Description rdf:about="http://purl.org/ica/ric#RiC-E3-RecordSet"/>
                </owl:unionOf>
            </owl:Class>
        </rdfs:domain>
        <rdfs:range rdf:resource="http://www.w3.org/2000/01/rdf-schema#Literal"/>
        <rdfs:comment xml:lang="en">Data Type: Text</rdfs:comment>
        <rdfs:comment xml:lang="en">Property for RiC-P19</rdfs:comment>
        <rdfs:label xml:lang="en">conditions of use</rdfs:label>
        <skos:definition xml:lang="en">Conditions affecting the availability of the Record for use after access has been provided.</skos:definition>
        <skos:example xml:lang="en">freely usable without restrictions; the permision of the owner of the Record must be obtained before use</skos:example>
        <skos:scopeNote xml:lang="en">Includes conditions governing reproduction of the Record under applicable  copyright (intellectual property) or property legislation.</skos:scopeNote>
    </owl:DatatypeProperty>
    


    <!-- http://purl.org/ica/ric#RiC-P-contactInformation -->

    <owl:DatatypeProperty rdf:about="http://purl.org/ica/ric#RiC-P-contactInformation">
        <rdfs:range rdf:resource="http://www.w3.org/2000/01/rdf-schema#Literal"/>
        <rdfs:comment xml:lang="en">Data Type: Text</rdfs:comment>
        <rdfs:comment xml:lang="en">Property for RiC-P39</rdfs:comment>
        <rdfs:label xml:lang="en">contact information</rdfs:label>
        <skos:definition xml:lang="en">Contact information to request information about available public services, service policies, and so on.</skos:definition>
        <skos:example xml:lang="fr">29 chemin du Moulin Detesta
13090 Aix-en-Provence (France)
Site web : 
http://www.archivesnationales.culture.gouv.fr/caom/fr/index.html 
France. Direction des Archives de France 
Note: For the institution Archives nationales d’outre-mer
Téléphone : +33 (0)4 42 93 38 50 
Télécopie : +33 (0)4 42 93 38 99 
Adresse électronique : caom.aix</skos:example>
        <skos:example xml:lang="pt">Coordenação Regional no Distrito Federal, em Brasília (COREG): 
SIG – Q6 Lote 800 – Anexo ao prédio da Imprensa Nacional 
70610-460 – Brasília – DF 
Brasil 
www.arquivonacional.gov.br 
Brazil. Arquivo Nacional 
Note: For the institution Arquivo Nacional</skos:example>
    </owl:DatatypeProperty>
    


    <!-- http://purl.org/ica/ric#RiC-P-contentExtent -->

    <owl:DatatypeProperty rdf:about="http://purl.org/ica/ric#RiC-P-contentExtent">
        <rdfs:domain>
            <owl:Class>
                <owl:unionOf rdf:parseType="Collection">
                    <rdf:Description rdf:about="http://purl.org/ica/ric#RiC-E1-Record"/>
                    <rdf:Description rdf:about="http://purl.org/ica/ric#RiC-E3-RecordSet"/>
                </owl:unionOf>
            </owl:Class>
        </rdfs:domain>
        <rdfs:range rdf:resource="http://www.w3.org/2000/01/rdf-schema#Literal"/>
        <rdfs:comment xml:lang="en">Data Type: Text</rdfs:comment>
        <rdfs:comment xml:lang="en">Property for RiC-P7, RiC-P29</rdfs:comment>
        <rdfs:label xml:lang="en">content extent</rdfs:label>
        <skos:definition xml:lang="en">Countable characteristics of the content of the Record, expressed as a 
quantity.</skos:definition>
        <skos:example xml:lang="en">duration: 3 minutes and 24 seconds; 6 maps; 34 poems.</skos:example>
        <skos:scopeNote xml:lang="en">Content extent information is independent of carrier extent information; the number, size or duration of the content unit(s) would remain the same even if the number or size of the carriers it was contained on differed.</skos:scopeNote>
    </owl:DatatypeProperty>
    


    <!-- http://purl.org/ica/ric#RiC-P-contentType -->

    <owl:DatatypeProperty rdf:about="http://purl.org/ica/ric#RiC-P-contentType"/>
    


    <!-- http://purl.org/ica/ric#RiC-P-date -->

    <owl:DatatypeProperty rdf:about="http://purl.org/ica/ric#RiC-P-date">
        <rdfs:range rdf:resource="http://www.w3.org/2001/XMLSchema#dateTime"/>
        <rdfs:comment xml:lang="en">Data Type: ISO 8601 Time and Date Format.</rdfs:comment>
        <rdfs:comment xml:lang="en">Property for RiC-P68.</rdfs:comment>
        <rdfs:label xml:lang="en">date</rdfs:label>
        <skos:definition xml:lang="en">Chronological information associated with the relation that contributes to its identification and contextualization.</skos:definition>
        <skos:example xml:lang="en">1792-08-10; 1798-10-30; 1720/1780</skos:example>
        <skos:scopeNote xml:lang="en">If applicable, includes the Date (range or time) when there is a relation between two entities. Will not apply to all relations. For example, will not apply to relations to Date. Additional exceptions will be noted in future RiC releases.</skos:scopeNote>
    </owl:DatatypeProperty>
    


    <!-- http://purl.org/ica/ric#RiC-P-description -->

    <owl:DatatypeProperty rdf:about="http://purl.org/ica/ric#RiC-P-description">
        <rdfs:domain>
            <owl:Class>
                <owl:unionOf rdf:parseType="Collection">
                    <rdf:Description rdf:about="http://purl.org/ica/ric#RiC-E10-Mandate"/>
                    <rdf:Description rdf:about="http://purl.org/ica/ric#RiC-E11-DocumentaryForm"/>
                    <rdf:Description rdf:about="http://purl.org/ica/ric#RiC-E14-ConceptThing"/>
                    <rdf:Description rdf:about="http://purl.org/ica/ric#RiC-E5-Occupation"/>
                    <rdf:Description rdf:about="http://purl.org/ica/ric#RiC-E6-Position"/>
                    <rdf:Description rdf:about="http://purl.org/ica/ric#RiC-E7-Function"/>
                    <rdf:Description rdf:about="http://purl.org/ica/ric#RiC-E8-FunctionAbstract"/>
                    <rdf:Description rdf:about="http://purl.org/ica/ric#RiC-E9-Activity"/>
                </owl:unionOf>
            </owl:Class>
        </rdfs:domain>
        <rdfs:range rdf:resource="http://www.w3.org/2000/01/rdf-schema#Literal"/>
        <rdfs:comment xml:lang="en">Data Type: Text</rdfs:comment>
        <rdfs:comment xml:lang="en">Property for RiC-P43, RiC-P46, RiC-P49, RiC-P51, RiC-P53, RiC-P56, RiC-P59, RiC-P67.</rdfs:comment>
        <rdfs:label xml:lang="en">description</rdfs:label>
        <skos:definition xml:lang="en">For RiC-P43: Description of the Occupation including the Functions fulfilled and the Activities involved.</skos:definition>
        <skos:definition xml:lang="en">For RiC-P46: Description of the Position as defined by and within the controlling corporate body.</skos:definition>
        <skos:definition xml:lang="en">For RiC-P49: Description of the nature, scope and meaning of the Function.</skos:definition>
        <skos:definition xml:lang="en">For RiC-P51: Definition of the Function (Abstract).</skos:definition>
        <skos:definition xml:lang="en">For RiC-P53: Description of coordinated actions or transactions performed in fulfillment of a Function, or pursuit of an Occupation.</skos:definition>
        <skos:definition xml:lang="en">For RiC-P56: Information describing the authority, Functions, Activities, policies, or procedures that comprise the Mandate; the jurisdictional limits and the temporal period within which the Mandate is effective or valid; and the Agent or Agents that are governed by the Mandate.</skos:definition>
        <skos:definition xml:lang="en">For RiC-P59: Description of the Documentary Form including its main extrinsic and intrinsic characteristics.</skos:definition>
        <skos:definition xml:lang="en">For RiC-P67: Description of the Concept/Thing.</skos:definition>
        <skos:example xml:lang="en">For RiC-P49: The function of undertaking academic research covers the conduct of all academic research, whether it is funded by the university itself, by external organizations, or by both. It also covers research undertaken in collaboration with other institutions [example for research, University of Strathclyde].</skos:example>
        <skos:example xml:lang="en">For RiC-P51: The systematic investigation into and study of materials and sources in order to establish facts and research new conclusions [example for ‘research’].</skos:example>
        <skos:example xml:lang="en">For RiC-P53: Tasks involved in developing and establishing the university’s research strategy include: identifying requirements for a new or revised strategy; undertaking research; developing strategy proposals; consulting on strategy proposals; reviewing and revising strategy proposals in light of comments received; drafting strategy documents; consulting on strategy documents; reviewing draft strategy documents in light of comments received; producing final strategy documents; submitting final strategy documents for formal endorsement; formally endorsing strategy documents; disseminating strategy documents; reviewing strategies [example for research strategy development, University of Strathclyde].</skos:example>
        <skos:scopeNote xml:lang="en">For RiC-P46: The remit of the Position.</skos:scopeNote>
        <skos:scopeNote xml:lang="en">For RiC-P53: Includes description of constituent Activities.</skos:scopeNote>
    </owl:DatatypeProperty>
    


    <!-- http://purl.org/ica/ric#RiC-P-encodingFormat -->

    <owl:DatatypeProperty rdf:about="http://purl.org/ica/ric#RiC-P-encodingFormat"/>
    


    <!-- http://purl.org/ica/ric#RiC-P-facilities -->

    <owl:DatatypeProperty rdf:about="http://purl.org/ica/ric#RiC-P-facilities">
        <rdfs:range rdf:resource="http://www.w3.org/2000/01/rdf-schema#Literal"/>
        <rdfs:comment xml:lang="en">Data Type: Text</rdfs:comment>
        <rdfs:comment xml:lang="en">Property for RiC-P41</rdfs:comment>
        <rdfs:label xml:lang="en">facilities</rdfs:label>
        <skos:definition xml:lang="en">Description of physical facilities where an Agent provides public services.</skos:definition>
        <skos:scopeNote xml:lang="en">Includes issues of physical accessibility, such as wheelchair access, and other provisions for users with physical disabilities.</skos:scopeNote>
    </owl:DatatypeProperty>
    


    <!-- http://purl.org/ica/ric#RiC-P-gender -->

    <owl:DatatypeProperty rdf:about="http://purl.org/ica/ric#RiC-P-gender"/>
    


    <!-- http://purl.org/ica/ric#RiC-P-generalNote -->

    <owl:DatatypeProperty rdf:about="http://purl.org/ica/ric#RiC-P-generalNote">
        <rdfs:domain>
            <owl:Class>
                <owl:unionOf rdf:parseType="Collection">
                    <rdf:Description rdf:about="http://purl.org/ica/ric#RiC-E1-Record"/>
                    <rdf:Description rdf:about="http://purl.org/ica/ric#RiC-E10-Mandate"/>
                    <rdf:Description rdf:about="http://purl.org/ica/ric#RiC-E11-DocumentaryForm"/>
                    <rdf:Description rdf:about="http://purl.org/ica/ric#RiC-E12-Date"/>
                    <rdf:Description rdf:about="http://purl.org/ica/ric#RiC-E13-Place"/>
                    <rdf:Description rdf:about="http://purl.org/ica/ric#RiC-E14-ConceptThing"/>
                    <rdf:Description rdf:about="http://purl.org/ica/ric#RiC-E2-RecordComponent"/>
                    <rdf:Description rdf:about="http://purl.org/ica/ric#RiC-E3-RecordSet"/>
                    <rdf:Description rdf:about="http://purl.org/ica/ric#RiC-E4-Agent"/>
                    <rdf:Description rdf:about="http://purl.org/ica/ric#RiC-E5-Occupation"/>
                    <rdf:Description rdf:about="http://purl.org/ica/ric#RiC-E6-Position"/>
                    <rdf:Description rdf:about="http://purl.org/ica/ric#RiC-E7-Function"/>
                    <rdf:Description rdf:about="http://purl.org/ica/ric#RiC-E8-FunctionAbstract"/>
                    <rdf:Description rdf:about="http://purl.org/ica/ric#RiC-E9-Activity"/>
                </owl:unionOf>
            </owl:Class>
        </rdfs:domain>
        <rdfs:range rdf:resource="http://www.w3.org/2000/01/rdf-schema#Literal"/>
        <rdfs:comment xml:lang="en">Data Type: Text</rdfs:comment>
        <rdfs:comment xml:lang="en">Property RiC-P4</rdfs:comment>
        <rdfs:label xml:lang="en">general note</rdfs:label>
        <skos:definition xml:lang="en">Description of the entity that is not otherwise addressed.</skos:definition>
        <skos:scopeNote xml:lang="en">Includes information on the relation of the entity to any other RiC entity that is not otherwise provided.</skos:scopeNote>
    </owl:DatatypeProperty>
    


    <!-- http://purl.org/ica/ric#RiC-P-geographicCoordinates -->

    <owl:DatatypeProperty rdf:about="http://purl.org/ica/ric#RiC-P-geographicCoordinates"/>
    


    <!-- http://purl.org/ica/ric#RiC-P-globalPersistentIdentifier -->

    <owl:DatatypeProperty rdf:about="http://purl.org/ica/ric#RiC-P-globalPersistentIdentifier">
        <rdfs:domain>
            <owl:Class>
                <owl:unionOf rdf:parseType="Collection">
                    <rdf:Description rdf:about="http://purl.org/ica/ric#RiC-E1-Record"/>
                    <rdf:Description rdf:about="http://purl.org/ica/ric#RiC-E10-Mandate"/>
                    <rdf:Description rdf:about="http://purl.org/ica/ric#RiC-E11-DocumentaryForm"/>
                    <rdf:Description rdf:about="http://purl.org/ica/ric#RiC-E12-Date"/>
                    <rdf:Description rdf:about="http://purl.org/ica/ric#RiC-E13-Place"/>
                    <rdf:Description rdf:about="http://purl.org/ica/ric#RiC-E14-ConceptThing"/>
                    <rdf:Description rdf:about="http://purl.org/ica/ric#RiC-E2-RecordComponent"/>
                    <rdf:Description rdf:about="http://purl.org/ica/ric#RiC-E3-RecordSet"/>
                    <rdf:Description rdf:about="http://purl.org/ica/ric#RiC-E4-Agent"/>
                    <rdf:Description rdf:about="http://purl.org/ica/ric#RiC-E5-Occupation"/>
                    <rdf:Description rdf:about="http://purl.org/ica/ric#RiC-E6-Position"/>
                    <rdf:Description rdf:about="http://purl.org/ica/ric#RiC-E7-Function"/>
                    <rdf:Description rdf:about="http://purl.org/ica/ric#RiC-E8-FunctionAbstract"/>
                    <rdf:Description rdf:about="http://purl.org/ica/ric#RiC-E9-Activity"/>
                </owl:unionOf>
            </owl:Class>
        </rdfs:domain>
        <rdfs:range rdf:resource="http://www.w3.org/2001/XMLSchema#anyURI"/>
        <rdfs:comment xml:lang="en">Data Type: URI</rdfs:comment>
        <rdfs:comment xml:lang="en">Property RiC-P1</rdfs:comment>
        <rdfs:label xml:lang="en">global persistent Identifier</rdfs:label>
        <skos:definition xml:lang="en">Globally unique and persistently resolvable identifier for the entity.</skos:definition>
        <skos:example xml:lang="en">http://n2t.net/ark:/99166/w6v1266v [example of an Archival Resource Key 
persistent identifier for a Record]; http://isni.org/0000000073572182 
[example of a persistent International Standard Name Identifier for a person]</skos:example>
    </owl:DatatypeProperty>
    


    <!-- http://purl.org/ica/ric#RiC-P-history -->

    <owl:DatatypeProperty rdf:about="http://purl.org/ica/ric#RiC-P-history">
        <rdfs:domain>
            <owl:Class>
                <owl:unionOf rdf:parseType="Collection">
                    <rdf:Description rdf:about="http://purl.org/ica/ric#RiC-E1-Record"/>
                    <rdf:Description rdf:about="http://purl.org/ica/ric#RiC-E10-Mandate"/>
                    <rdf:Description rdf:about="http://purl.org/ica/ric#RiC-E11-DocumentaryForm"/>
                    <rdf:Description rdf:about="http://purl.org/ica/ric#RiC-E3-RecordSet"/>
                    <rdf:Description rdf:about="http://purl.org/ica/ric#RiC-E4-Agent"/>
                    <rdf:Description rdf:about="http://purl.org/ica/ric#RiC-E5-Occupation"/>
                    <rdf:Description rdf:about="http://purl.org/ica/ric#RiC-E6-Position"/>
                    <rdf:Description rdf:about="http://purl.org/ica/ric#RiC-E7-Function"/>
                    <rdf:Description rdf:about="http://purl.org/ica/ric#RiC-E9-Activity"/>
                </owl:unionOf>
            </owl:Class>
        </rdfs:domain>
        <rdfs:range rdf:resource="http://www.w3.org/2000/01/rdf-schema#Literal"/>
        <rdfs:comment xml:lang="en">Data Type: Text</rdfs:comment>
        <rdfs:comment xml:lang="en">Property for RiC-P20, RiC-P28, RiC-P35, RiC-P44, RiC-P47, RiC-P50, RiC-P54, RiC-P57, RiC-P60.</rdfs:comment>
        <rdfs:label xml:lang="en">history</rdfs:label>
        <skos:definition xml:lang="en">For RiC-P20: An account of the history of the Record. To the extent known, this may cover the entire history of the Record from its inception to the date of the description.</skos:definition>
        <skos:definition xml:lang="en">For RiC-P28: An account of the history of the Record Set. To the extent known, this may  cover the entire history of the Record Set from its inception to the date of  the description.</skos:definition>
        <skos:definition xml:lang="en">For RiC-P35: Concise history of the Agent.</skos:definition>
        <skos:definition xml:lang="en">For RiC-P44: Concise history of the Occupation and its changes over time, including  changes concerning the rules governing it and the persons who pursued it.</skos:definition>
        <skos:definition xml:lang="en">For RiC-P47: History of the Position, of its creation and definition, and of its changes over  time, including changes concerning the competencies required, the authority  and Functions assigned, and the persons holding the Position.</skos:definition>
        <skos:definition xml:lang="en">For RiC-P50: History of origin and development of the goals, purposes, or objectives  defined in a Function.</skos:definition>
        <skos:definition xml:lang="en">For RiC-P57: Information describing the origin and development of the Mandate.</skos:definition>
        <skos:definition xml:lang="en">For RiC-P60: History of the Documentary Form including the context in which it first appeared or its usage developed, in which it was used, its changes over time, and the Agents who used it.</skos:definition>
        <skos:definition xml:lang="en">RiC-P54: History of origin and development of the Activity.</skos:definition>
        <skos:example xml:lang="en">For RiC-P28: The manuscripts are part of the collections of Robert Harley (d 1724) and Edward Harley (d 1741), 1st and 2nd Earls of Oxford, that were brought by Parliament and transferred to the British Museum in 1753. Those materials were then separated into this collection and those for Harley Charters and Harley Rolls and became part of the collections of the British Library in 1972.</skos:example>
        <skos:scopeNote xml:lang="en">For RiC-P20: The history may include events associated with custody, actions taken on the Record as part of its management (appraisal, description, classification and reclassification, data storage migration, encoding type conversions, and so on) that have contributed to its state at the time of description.  When known, provide Dates of and Agents associated with the events.</skos:scopeNote>
        <skos:scopeNote xml:lang="en">For RiC-P28: To the extent known, the history may cover the entire history of the Record Set from its inception to the date of the description. Significant Events include but are not limited to creation or formation of the Record Set, transfers of custody or ownership, changes in custodial responsibility, changes in the arrangement, additions (accruals) or removing or separation of member Records or Record Sets, and uses of the Record Set. Description of the events should include Agent(s), the Date(s) of the event(s), and the Place(s) where the event(s) occurred. Record Sets are not static, the membership is dynamic, that is member Records may come and go. Significant changes in classification would constitute the formulation of new Record Sets.</skos:scopeNote>
        <skos:scopeNote xml:lang="en">For RiC-P35: History may incorporate the general social, cultural, or economic context in  which the Agent lived or existed when such context aids in understanding the  Agent&apos;s Functions, Occupations, Positions or Activities.</skos:scopeNote>
        <skos:scopeNote xml:lang="en">For RiC-P50: Information may include description of the role or roles played by Agents in  authorizing or fulfilling the Function and how they changed over time, and  the Activities performed in fulfillment of the Function.</skos:scopeNote>
        <skos:scopeNote xml:lang="en">For RiC-P54: Information may include description of the Positions held by Agents in authorizing or performing the Activity and how they changed over time changes in how the Activity was performed and changes in Activities’ constituent Activities.</skos:scopeNote>
        <skos:scopeNote xml:lang="en">For RiC-P57: Such information includes description of the Agent or Agents that participated in the creation or development of the rules that comprise the Mandate revision of the jurisdictional limits or temporal period within which the Mandate is effective or valid, and changes in the Agent or Agents that are controlled or guided by the Mandate.</skos:scopeNote>
    </owl:DatatypeProperty>
    


    <!-- http://purl.org/ica/ric#RiC-P-identityType -->

    <owl:DatatypeProperty rdf:about="http://purl.org/ica/ric#RiC-P-identityType"/>
    


    <!-- http://purl.org/ica/ric#RiC-P-languageInformation -->

    <owl:DatatypeProperty rdf:about="http://purl.org/ica/ric#RiC-P-languageInformation"/>
    


    <!-- http://purl.org/ica/ric#RiC-P-localIdentifier -->

    <owl:DatatypeProperty rdf:about="http://purl.org/ica/ric#RiC-P-localIdentifier">
        <rdfs:domain>
            <owl:Class>
                <owl:unionOf rdf:parseType="Collection">
                    <rdf:Description rdf:about="http://purl.org/ica/ric#RiC-E1-Record"/>
                    <rdf:Description rdf:about="http://purl.org/ica/ric#RiC-E10-Mandate"/>
                    <rdf:Description rdf:about="http://purl.org/ica/ric#RiC-E11-DocumentaryForm"/>
                    <rdf:Description rdf:about="http://purl.org/ica/ric#RiC-E12-Date"/>
                    <rdf:Description rdf:about="http://purl.org/ica/ric#RiC-E13-Place"/>
                    <rdf:Description rdf:about="http://purl.org/ica/ric#RiC-E14-ConceptThing"/>
                    <rdf:Description rdf:about="http://purl.org/ica/ric#RiC-E2-RecordComponent"/>
                    <rdf:Description rdf:about="http://purl.org/ica/ric#RiC-E3-RecordSet"/>
                    <rdf:Description rdf:about="http://purl.org/ica/ric#RiC-E4-Agent"/>
                    <rdf:Description rdf:about="http://purl.org/ica/ric#RiC-E5-Occupation"/>
                    <rdf:Description rdf:about="http://purl.org/ica/ric#RiC-E6-Position"/>
                    <rdf:Description rdf:about="http://purl.org/ica/ric#RiC-E7-Function"/>
                    <rdf:Description rdf:about="http://purl.org/ica/ric#RiC-E8-FunctionAbstract"/>
                    <rdf:Description rdf:about="http://purl.org/ica/ric#RiC-E9-Activity"/>
                </owl:unionOf>
            </owl:Class>
        </rdfs:domain>
        <rdfs:range rdf:resource="http://www.w3.org/2000/01/rdf-schema#Literal"/>
        <rdfs:comment xml:lang="en">Data Type: Text</rdfs:comment>
        <rdfs:comment xml:lang="en">Property RiC-P2</rdfs:comment>
        <rdfs:label xml:lang="en">local Identifier</rdfs:label>
        <skos:definition xml:lang="en">Local identifier(s) assigned to the entity.</skos:definition>
        <skos:example xml:lang="en">BUD-01-F002 [example of a classification number from a corporate file plan]; NAS1/A/1.1 [example of local identifier for a Record]; F 1204 [example of a local identifier for a Record Set assigned by a repository]</skos:example>
        <skos:scopeNote xml:lang="en">This covers all identifiers other than Global Persistent Identifiers.</skos:scopeNote>
    </owl:DatatypeProperty>
    


    <!-- http://purl.org/ica/ric#RiC-P-mediaType -->

    <owl:DatatypeProperty rdf:about="http://purl.org/ica/ric#RiC-P-mediaType"/>
    


    <!-- http://purl.org/ica/ric#RiC-P-medium -->

    <owl:DatatypeProperty rdf:about="http://purl.org/ica/ric#RiC-P-medium"/>
    


    <!-- http://purl.org/ica/ric#RiC-P-name -->

    <owl:DatatypeProperty rdf:about="http://purl.org/ica/ric#RiC-P-name"/>
    


    <!-- http://purl.org/ica/ric#RiC-P-physicalCharacteristicsNote -->

    <owl:DatatypeProperty rdf:about="http://purl.org/ica/ric#RiC-P-physicalCharacteristicsNote">
        <rdfs:domain rdf:resource="http://purl.org/ica/ric#RiC-E1-Record"/>
        <rdfs:range rdf:resource="http://www.w3.org/2000/01/rdf-schema#Literal"/>
        <rdfs:comment xml:lang="en">Data Type: Text</rdfs:comment>
        <rdfs:comment xml:lang="en">Property for RiC-P16</rdfs:comment>
        <rdfs:label xml:lang="en">physical characteristics note</rdfs:label>
        <skos:definition xml:lang="en">Information about the physical characteristics of the Record.</skos:definition>
        <skos:example xml:lang="en">Record heavily foxed; emulsion flaking; watermarked; British Library binding</skos:example>
        <skos:scopeNote xml:lang="en">Includes information about the physical nature and condition such as  conservation status.</skos:scopeNote>
    </owl:DatatypeProperty>
    


    <!-- http://purl.org/ica/ric#RiC-P-physicalOrLogicalExtent -->

    <owl:DatatypeProperty rdf:about="http://purl.org/ica/ric#RiC-P-physicalOrLogicalExtent">
        <rdfs:domain>
            <owl:Class>
                <owl:unionOf rdf:parseType="Collection">
                    <rdf:Description rdf:about="http://purl.org/ica/ric#RiC-E1-Record"/>
                    <rdf:Description rdf:about="http://purl.org/ica/ric#RiC-E3-RecordSet"/>
                </owl:unionOf>
            </owl:Class>
        </rdfs:domain>
        <rdfs:range rdf:resource="http://www.w3.org/2000/01/rdf-schema#Literal"/>
        <rdfs:comment xml:lang="en">Data Type: Text</rdfs:comment>
        <rdfs:comment xml:lang="en">Property for RiC-P15, RiC-P30</rdfs:comment>
        <rdfs:label xml:lang="en">physical or logical extent</rdfs:label>
        <skos:definition xml:lang="en">For RiC-P15: Number of physical units and/or physical dimensions of Record carriers or, in the case of digital media carriers, the size of storage space occupied.</skos:definition>
        <skos:definition xml:lang="en">For RiC-P30: 40 pages; 5 folios; 25 m2; 1 USB stick; 3GB</skos:definition>
        <skos:definition xml:lang="en">For RiC-P30: Number of physical units and/or physical dimensions of Record Set carriers or, in the case of digital media carriers, the size of storage space occupied.</skos:definition>
        <skos:example xml:lang="en">For RiC-P15: 1 page; 5 folios; 17 x 34.5 cm; 1 USB stick; 3GB</skos:example>
    </owl:DatatypeProperty>
    


    <!-- http://purl.org/ica/ric#RiC-P-place -->

    <owl:DatatypeProperty rdf:about="http://purl.org/ica/ric#RiC-P-place"/>
    


    <!-- http://purl.org/ica/ric#RiC-P-productionTechnique -->

    <owl:DatatypeProperty rdf:about="http://purl.org/ica/ric#RiC-P-productionTechnique"/>
    


    <!-- http://purl.org/ica/ric#RiC-P-qualityOfInformation -->

    <owl:DatatypeProperty rdf:about="http://purl.org/ica/ric#RiC-P-qualityOfInformation">
        <rdfs:domain rdf:resource="http://purl.org/ica/ric#RiC-E1-Record"/>
        <rdfs:range rdf:resource="http://www.w3.org/2000/01/rdf-schema#Literal"/>
        <rdfs:comment xml:lang="en">Data Type: Text</rdfs:comment>
        <rdfs:comment xml:lang="en">Property for RiC-P8</rdfs:comment>
        <rdfs:label xml:lang="en">quality of Information</rdfs:label>
        <skos:definition xml:lang="en">Conditions of a Record that impact the legibility or completeness of its information, and thus the viability of its use.</skos:definition>
        <skos:example xml:lang="en">some loss of information due to poor quality image capture; some loss of text due to rodent damage</skos:example>
        <skos:scopeNote xml:lang="en">Such conditions may be associated with deficiencies in the processes of  Record creation or capture, or the deterioration of the Record (e.g. its carrier) causing loss of information over time.</skos:scopeNote>
    </owl:DatatypeProperty>
    


    <!-- http://purl.org/ica/ric#RiC-P-recordState -->

    <owl:DatatypeProperty rdf:about="http://purl.org/ica/ric#RiC-P-recordState"/>
    


    <!-- http://purl.org/ica/ric#RiC-P-scopeAndContent -->

    <owl:DatatypeProperty rdf:about="http://purl.org/ica/ric#RiC-P-scopeAndContent">
        <rdfs:domain>
            <owl:Class>
                <owl:unionOf rdf:parseType="Collection">
                    <rdf:Description rdf:about="http://purl.org/ica/ric#RiC-E1-Record"/>
                    <rdf:Description rdf:about="http://purl.org/ica/ric#RiC-E3-RecordSet"/>
                </owl:unionOf>
            </owl:Class>
        </rdfs:domain>
        <rdfs:range rdf:resource="http://www.w3.org/2000/01/rdf-schema#Literal"/>
        <rdfs:comment xml:lang="en">Data Type: Text</rdfs:comment>
        <rdfs:comment xml:lang="en">Property for RiC-P9, RiC-P31</rdfs:comment>
        <rdfs:label xml:lang="en">scope and content</rdfs:label>
        <skos:definition xml:lang="en">For RiC-P31: Summary of the scope (such as, time periods, geography) and content (such as content type, documentary forms, subject matter, administrative processes) of the member Records or Record Sets.</skos:definition>
        <skos:definition xml:lang="en">For RiC-P9: Summary of the scope (such as, time periods, geography) and content (such as subject matter, administrative processes) of the Record.</skos:definition>
        <skos:example xml:lang="en">For RiC-P9: Includes a detailed list of the lands and villages given by the King to the Abbey; among the witnesses, the duke of Normandy; the author explains why he does not agree with the decision made and adds that it cannot be applied</skos:example>
        <skos:scopeNote xml:lang="en">For RiC-P9: May include description of relations with Agents, other Records, Functions, Activities, Dates and Places. May also include description of components of the Record when considered significant and not considered separately.</skos:scopeNote>
    </owl:DatatypeProperty>
    


    <!-- http://purl.org/ica/ric#RiC-P-servicestothePublic -->

    <owl:DatatypeProperty rdf:about="http://purl.org/ica/ric#RiC-P-servicestothePublic">
        <rdfs:range rdf:resource="http://www.w3.org/2000/01/rdf-schema#Literal"/>
        <rdfs:comment xml:lang="en">Data Type: Text</rdfs:comment>
        <rdfs:comment xml:lang="en">Property for RiC-P38</rdfs:comment>
        <rdfs:label xml:lang="en">services to the public</rdfs:label>
        <skos:definition xml:lang="en">Description of public services policies, in particular with respect to  qualifications to use the services, and rights, privileges, and responsibilities of users of the services.</skos:definition>
    </owl:DatatypeProperty>
    


    <!-- http://purl.org/ica/ric#RiC-P-technicalCharacteristics -->

    <owl:DatatypeProperty rdf:about="http://purl.org/ica/ric#RiC-P-technicalCharacteristics">
        <rdfs:domain rdf:resource="http://purl.org/ica/ric#RiC-E4-Agent-DelegateAgent"/>
        <rdfs:range rdf:resource="http://www.w3.org/2000/01/rdf-schema#Literal"/>
        <rdfs:comment xml:lang="en">Data Type: Text</rdfs:comment>
        <rdfs:comment xml:lang="en">Property for RiC-P37</rdfs:comment>
        <rdfs:label xml:lang="en">technical characteristics</rdfs:label>
        <skos:definition xml:lang="en">Description of the technical characteristics of the delegate-Agent.</skos:definition>
    </owl:DatatypeProperty>
    


    <!-- http://purl.org/ica/ric#RiC-P-type -->

    <owl:DatatypeProperty rdf:about="http://purl.org/ica/ric#RiC-P-type"/>
    


    <!-- 
    ///////////////////////////////////////////////////////////////////////////////////////
    //
    // Classes
    //
    ///////////////////////////////////////////////////////////////////////////////////////
     -->

    


    <!-- http://purl.org/ica/ric#RiC-E1-Record -->

    <owl:Class rdf:about="http://purl.org/ica/ric#RiC-E1-Record">
        <rdfs:subClassOf>
            <owl:Restriction>
                <owl:onProperty rdf:resource="http://purl.org/ica/ric#RiC-R-hadPart"/>
                <owl:allValuesFrom rdf:resource="http://purl.org/ica/ric#RiC-E2-RecordComponent"/>
            </owl:Restriction>
        </rdfs:subClassOf>
        <rdfs:subClassOf>
            <owl:Restriction>
                <owl:onProperty rdf:resource="http://purl.org/ica/ric#RiC-R-hasPart"/>
                <owl:allValuesFrom rdf:resource="http://purl.org/ica/ric#RiC-E2-RecordComponent"/>
            </owl:Restriction>
        </rdfs:subClassOf>
        <rdfs:subClassOf>
            <owl:Restriction>
                <owl:onProperty rdf:resource="http://purl.org/ica/ric#RiC-R-hasSubject"/>
                <owl:allValuesFrom>
                    <owl:Class>
                        <owl:unionOf rdf:parseType="Collection">
                            <rdf:Description rdf:about="http://purl.org/ica/ric#RiC-E1-Record"/>
                            <rdf:Description rdf:about="http://purl.org/ica/ric#RiC-E10-Mandate"/>
                            <rdf:Description rdf:about="http://purl.org/ica/ric#RiC-E13-Place"/>
                            <rdf:Description rdf:about="http://purl.org/ica/ric#RiC-E14-ConceptThing"/>
                            <rdf:Description rdf:about="http://purl.org/ica/ric#RiC-E4-Agent"/>
                            <rdf:Description rdf:about="http://purl.org/ica/ric#RiC-E5-Occupation"/>
                            <rdf:Description rdf:about="http://purl.org/ica/ric#RiC-E6-Position"/>
                            <rdf:Description rdf:about="http://purl.org/ica/ric#RiC-E7-Function"/>
                            <rdf:Description rdf:about="http://purl.org/ica/ric#RiC-E8-FunctionAbstract"/>
                            <rdf:Description rdf:about="http://purl.org/ica/ric#RiC-E9-Activity"/>
                        </owl:unionOf>
                    </owl:Class>
                </owl:allValuesFrom>
            </owl:Restriction>
        </rdfs:subClassOf>
        <rdfs:subClassOf>
            <owl:Restriction>
                <owl:onProperty rdf:resource="http://purl.org/ica/ric#RiC-R-isEvidenceOf"/>
                <owl:allValuesFrom>
                    <owl:Class>
                        <owl:unionOf rdf:parseType="Collection">
                            <rdf:Description rdf:about="http://purl.org/ica/ric#RiC-E10-Mandate"/>
                            <rdf:Description rdf:about="http://purl.org/ica/ric#RiC-E7-Function"/>
                        </owl:unionOf>
                    </owl:Class>
                </owl:allValuesFrom>
            </owl:Restriction>
        </rdfs:subClassOf>
        <rdfs:subClassOf>
            <owl:Restriction>
                <owl:onProperty rdf:resource="http://purl.org/ica/ric#RiC-R-isMemberOf"/>
                <owl:allValuesFrom rdf:resource="http://purl.org/ica/ric#RiC-E3-RecordSet"/>
            </owl:Restriction>
        </rdfs:subClassOf>
        <rdfs:subClassOf>
            <owl:Restriction>
                <owl:onProperty rdf:resource="http://purl.org/ica/ric#RiC-R-isSubjectOf"/>
                <owl:allValuesFrom rdf:resource="http://purl.org/ica/ric#RiC-E1-Record"/>
            </owl:Restriction>
        </rdfs:subClassOf>
        <rdfs:subClassOf>
            <owl:Restriction>
                <owl:onProperty rdf:resource="http://purl.org/ica/ric#RiC-R-wasMemberOf"/>
                <owl:allValuesFrom rdf:resource="http://purl.org/ica/ric#RiC-E3-RecordSet"/>
            </owl:Restriction>
        </rdfs:subClassOf>
        <rdfs:comment xml:lang="en">Class for entity RiC-E1.</rdfs:comment>
        <rdfs:label xml:lang="en">Record</rdfs:label>
        <skos:definition xml:lang="en">Linguistic, symbolic, or graphic information represented in any persistent form, on any durable carrier, by any method, by an Agent in the course of life or work events and Activities.</skos:definition>
        <skos:example xml:lang="en">deed appointing John Bambridge, Sheriff of Leicestershire, with 3  Great Seal of Charles I appended; sketch Map of the Qatar Peninsula; email message concerning an agreement to participate in the ICA Seoul Congress containing two attachments and digitally signed</skos:example>
        <skos:scopeNote xml:lang="en">One or more Records in one context may be subsumed or incorporated into a Record in another context to form a new Record. This ‘compound Record’ should not be confused with a Record Set, as it is evidence of a single transaction by an Agent rather than a grouping of distinct Records as part of their management and use.</skos:scopeNote>
        <skos:scopeNote xml:lang="en">Such information may serve a variety of purposes, including documenting the events and Activities. Because of its relation to the events and Activities, it serves as evidence for them no matter its quality for use in a particular context.</skos:scopeNote>
    </owl:Class>
    


    <!-- http://purl.org/ica/ric#RiC-E10-Mandate -->

    <owl:Class rdf:about="http://purl.org/ica/ric#RiC-E10-Mandate">
        <rdfs:subClassOf>
            <owl:Restriction>
                <owl:onProperty rdf:resource="http://purl.org/ica/ric#RiC-R-isEvidencedBy"/>
                <owl:allValuesFrom>
                    <owl:Class>
                        <owl:unionOf rdf:parseType="Collection">
                            <rdf:Description rdf:about="http://purl.org/ica/ric#RiC-E1-Record"/>
                            <rdf:Description rdf:about="http://purl.org/ica/ric#RiC-E3-RecordSet"/>
                        </owl:unionOf>
                    </owl:Class>
                </owl:allValuesFrom>
            </owl:Restriction>
        </rdfs:subClassOf>
        <rdfs:subClassOf>
            <owl:Restriction>
                <owl:onProperty rdf:resource="http://purl.org/ica/ric#RiC-R-isSubjectOf"/>
                <owl:allValuesFrom>
                    <owl:Class>
                        <owl:unionOf rdf:parseType="Collection">
                            <rdf:Description rdf:about="http://purl.org/ica/ric#RiC-E1-Record"/>
                            <rdf:Description rdf:about="http://purl.org/ica/ric#RiC-E2-RecordComponent"/>
                            <rdf:Description rdf:about="http://purl.org/ica/ric#RiC-E3-RecordSet"/>
                        </owl:unionOf>
                    </owl:Class>
                </owl:allValuesFrom>
            </owl:Restriction>
        </rdfs:subClassOf>
        <rdfs:comment xml:lang="en">Class for entity RiC-E10.</rdfs:comment>
        <rdfs:label xml:lang="en">Mandate</rdfs:label>
        <skos:definition xml:lang="en">Authority or rules that govern the actions of an Agent within a specific social and cultural context.</skos:definition>
        <skos:example xml:lang="en">authority granted by electors to a person to represent them in  Parliament; authority of a Mayor to grant building authorisations; rules set out in Records in Context: A Conceptual Model for Archival Description, a document published by the International Council on Archives (ICA) which defines how an archivist describes archival material; the mandate of the Australian Hearing Services, as set out by the Australian Hearing Services Act 1991 (s 7), is to provide hearing services, carry out research and development in relation to hearing services and acoustic development, and conduct education about hearing services, in addition to any other functions conferred on the Authority (s 8). The power to perform these functions is exercised by the Authority (s 9) a body corporate governed by a Board of Directors (ss 7, 13, 14, 15 and 16), which is subject to the direction of the Minister for Human Services (s 12). The Managing Director manages the Authority, under the Board (s 42). (Adapted from source: https://www.humanservices.gov.au/corporate/about-us/legislation)</skos:example>
        <skos:scopeNote xml:lang="en">A Mandate establishes the rules that govern the actions and confer the authority or competencies of Agents to fulfill designated Functions or perform designated Activities.</skos:scopeNote>
        <skos:scopeNote xml:lang="en">A Mandate should not be confused with the one or more documentary sources that serve as evidence of its identity.</skos:scopeNote>
        <skos:scopeNote xml:lang="en">A Mandate specifies or authorizes the Functions (goals) of an Agent (who); or the Activities to be performed by an Agent in fulfillment of the Function (means); or the policies or procedures that govern the performance of the Activity (how); and the Place (jurisdiction) and Date (time period) within which an Agent may perform the Activities (where and when).</skos:scopeNote>
        <skos:scopeNote xml:lang="en">Mandates exist in a specific social and cultural context, and within that context are subject to change over time.</skos:scopeNote>
        <skos:scopeNote xml:lang="en">The evidence for identifying a Mandate may be found in its entirety in one documentary source (for example, a law or regulation), or may be found in two or more sources.</skos:scopeNote>
        <skos:scopeNote xml:lang="en">The source or sources of some Mandates are external to the Agent (for example, expressed in elections, social mores, customs, community expectations, laws, regulations, standards and best practice codes), while others are expressed within the Agent’s immediate context (for example, policies, or written or verbal instructions).</skos:scopeNote>
        <skos:scopeNote xml:lang="en">While a Mandate may be tacit, in whole or part, it may be explicitly expressed in a variety of documentary sources (for example, constitutions, legislation, (legal) acts, statutes, legal codes, ordinances, charges, charters, mission statements, regulations, policies, procedures, or standards).</skos:scopeNote>
    </owl:Class>
    


    <!-- http://purl.org/ica/ric#RiC-E11-DocumentaryForm -->

    <owl:Class rdf:about="http://purl.org/ica/ric#RiC-E11-DocumentaryForm">
        <rdfs:comment xml:lang="en">Class for entity RiC-E11.</rdfs:comment>
        <rdfs:label xml:lang="en">Documentary Form</rdfs:label>
        <skos:definition xml:lang="en">The rules used in the creation of a Record that prescribes the particular physical or intellectual elements that must be present.</skos:definition>
        <skos:example xml:lang="en">deed of gift; email; letter; papal bull; charter; letters patent; birth certificate; will</skos:example>
        <skos:scopeNote xml:lang="en">Documentary forms exist in a specific social and cultural context, and within that context are subject to change over time.</skos:scopeNote>
        <skos:scopeNote xml:lang="en">The Documentary Form plays an important role in determining the type of information a Record may comprise, its status of perfection, and its authenticity and reliability.</skos:scopeNote>
    </owl:Class>
    


    <!-- http://purl.org/ica/ric#RiC-E12-Date -->

    <owl:Class rdf:about="http://purl.org/ica/ric#RiC-E12-Date">
        <rdfs:comment xml:lang="en">Class for entity RiC-E12.</rdfs:comment>
        <rdfs:label xml:lang="en">Date</rdfs:label>
        <skos:definition xml:lang="en">Chronological information associated with an entity that contributes to its identification and contextualization.</skos:definition>
        <skos:example xml:lang="en">1925-1957; 20th Century; 3 Henry VIII; 4 March 1842; 9 Thermidor An II; c. 1860s</skos:example>
    </owl:Class>
    


    <!-- http://purl.org/ica/ric#RiC-E13-Place -->

    <owl:Class rdf:about="http://purl.org/ica/ric#RiC-E13-Place">
        <rdfs:subClassOf>
            <owl:Restriction>
                <owl:onProperty rdf:resource="http://purl.org/ica/ric#RiC-R-isSubjectOf"/>
                <owl:allValuesFrom>
                    <owl:Class>
                        <owl:unionOf rdf:parseType="Collection">
                            <rdf:Description rdf:about="http://purl.org/ica/ric#RiC-E1-Record"/>
                            <rdf:Description rdf:about="http://purl.org/ica/ric#RiC-E2-RecordComponent"/>
                            <rdf:Description rdf:about="http://purl.org/ica/ric#RiC-E3-RecordSet"/>
                        </owl:unionOf>
                    </owl:Class>
                </owl:allValuesFrom>
            </owl:Restriction>
        </rdfs:subClassOf>
        <rdfs:comment xml:lang="en">Class for entity RiC-E13.</rdfs:comment>
        <rdfs:label xml:lang="en">Place</rdfs:label>
        <skos:definition xml:lang="en">Jurisdictions and any geographic or administrative point or area.</skos:definition>
        <skos:example xml:lang="en">Amazon River; Nova Scotia; Paris; North Lanarkshire District; Manchester Diocese; Rugby Urban Sanitary District</skos:example>
        <skos:scopeNote xml:lang="en">Includes settlements of any kind (towns, villages, etc.), historical regions, and political and administrative districts.</skos:scopeNote>
    </owl:Class>
    


    <!-- http://purl.org/ica/ric#RiC-E14-ConceptThing -->

    <owl:Class rdf:about="http://purl.org/ica/ric#RiC-E14-ConceptThing">
        <rdfs:subClassOf>
            <owl:Restriction>
                <owl:onProperty rdf:resource="http://purl.org/ica/ric#RiC-R-isSubjectOf"/>
                <owl:allValuesFrom>
                    <owl:Class>
                        <owl:unionOf rdf:parseType="Collection">
                            <rdf:Description rdf:about="http://purl.org/ica/ric#RiC-E1-Record"/>
                            <rdf:Description rdf:about="http://purl.org/ica/ric#RiC-E2-RecordComponent"/>
                            <rdf:Description rdf:about="http://purl.org/ica/ric#RiC-E3-RecordSet"/>
                        </owl:unionOf>
                    </owl:Class>
                </owl:allValuesFrom>
            </owl:Restriction>
        </rdfs:subClassOf>
        <rdfs:comment xml:lang="en">Class for entity RiC-E14.</rdfs:comment>
        <rdfs:label xml:lang="en">Concept/Thing</rdfs:label>
        <skos:definition xml:lang="en">Any idea or notion, material thing, or event or occurrence that can be associated with, or in some cases be the subject of, other entities.</skos:definition>
        <skos:example xml:lang="en">airplanes; Battle of the Somme; impressionism; Puck; renaissance; slavery; Before Christian Era (BCE); French Revolution</skos:example>
        <skos:scopeNote xml:lang="en">Includes all RiC entities as well as the following:  abstract concepts; cultural movements, named periods and events; named things, objects and works; legendary, mythical or fictitious figures, characters or beings.</skos:scopeNote>
    </owl:Class>
    


    <!-- http://purl.org/ica/ric#RiC-E2-RecordComponent -->

    <owl:Class rdf:about="http://purl.org/ica/ric#RiC-E2-RecordComponent">
        <rdfs:subClassOf>
            <owl:Restriction>
                <owl:onProperty rdf:resource="http://purl.org/ica/ric#RiC-R-hasSubject"/>
                <owl:allValuesFrom>
                    <owl:Class>
                        <owl:unionOf rdf:parseType="Collection">
                            <rdf:Description rdf:about="http://purl.org/ica/ric#RiC-E10-Mandate"/>
                            <rdf:Description rdf:about="http://purl.org/ica/ric#RiC-E13-Place"/>
                            <rdf:Description rdf:about="http://purl.org/ica/ric#RiC-E14-ConceptThing"/>
                            <rdf:Description rdf:about="http://purl.org/ica/ric#RiC-E4-Agent"/>
                            <rdf:Description rdf:about="http://purl.org/ica/ric#RiC-E5-Occupation"/>
                            <rdf:Description rdf:about="http://purl.org/ica/ric#RiC-E6-Position"/>
                            <rdf:Description rdf:about="http://purl.org/ica/ric#RiC-E7-Function"/>
                            <rdf:Description rdf:about="http://purl.org/ica/ric#RiC-E8-FunctionAbstract"/>
                            <rdf:Description rdf:about="http://purl.org/ica/ric#RiC-E9-Activity"/>
                        </owl:unionOf>
                    </owl:Class>
                </owl:allValuesFrom>
            </owl:Restriction>
        </rdfs:subClassOf>
        <rdfs:subClassOf>
            <owl:Restriction>
                <owl:onProperty rdf:resource="http://purl.org/ica/ric#RiC-R-isEvidenceOf"/>
                <owl:allValuesFrom rdf:resource="http://purl.org/ica/ric#RiC-E7-Function"/>
            </owl:Restriction>
        </rdfs:subClassOf>
        <rdfs:subClassOf>
            <owl:Restriction>
                <owl:onProperty rdf:resource="http://purl.org/ica/ric#RiC-R-isPartOf"/>
                <owl:allValuesFrom rdf:resource="http://purl.org/ica/ric#RiC-E1-Record"/>
            </owl:Restriction>
        </rdfs:subClassOf>
        <rdfs:subClassOf>
            <owl:Restriction>
                <owl:onProperty rdf:resource="http://purl.org/ica/ric#RiC-R-wasPartOf"/>
                <owl:allValuesFrom rdf:resource="http://purl.org/ica/ric#RiC-E1-Record"/>
            </owl:Restriction>
        </rdfs:subClassOf>
        <rdfs:comment xml:lang="en">Class for entity RiC-E2.</rdfs:comment>
        <rdfs:label xml:lang="en">Record Component</rdfs:label>
        <skos:definition xml:lang="en">Part of a Record with discrete information content that contributes to the Record&apos;s physical or intellectual completeness.</skos:definition>
        <skos:example xml:lang="en">3rd Great Seal of Charles I; two digital photographs attached to an email message.</skos:example>
        <skos:scopeNote xml:lang="en">If removed the completeness of the record is compromised.</skos:scopeNote>
    </owl:Class>
    


    <!-- http://purl.org/ica/ric#RiC-E3-RecordSet -->

    <owl:Class rdf:about="http://purl.org/ica/ric#RiC-E3-RecordSet">
        <rdfs:subClassOf>
            <owl:Restriction>
                <owl:onProperty rdf:resource="http://purl.org/ica/ric#RiC-R-hadMember"/>
                <owl:allValuesFrom>
                    <owl:Class>
                        <owl:unionOf rdf:parseType="Collection">
                            <rdf:Description rdf:about="http://purl.org/ica/ric#RiC-E1-Record"/>
                            <rdf:Description rdf:about="http://purl.org/ica/ric#RiC-E3-RecordSet"/>
                        </owl:unionOf>
                    </owl:Class>
                </owl:allValuesFrom>
            </owl:Restriction>
        </rdfs:subClassOf>
        <rdfs:subClassOf>
            <owl:Restriction>
                <owl:onProperty rdf:resource="http://purl.org/ica/ric#RiC-R-hasMember"/>
                <owl:allValuesFrom>
                    <owl:Class>
                        <owl:unionOf rdf:parseType="Collection">
                            <rdf:Description rdf:about="http://purl.org/ica/ric#RiC-E1-Record"/>
                            <rdf:Description rdf:about="http://purl.org/ica/ric#RiC-E3-RecordSet"/>
                        </owl:unionOf>
                    </owl:Class>
                </owl:allValuesFrom>
            </owl:Restriction>
        </rdfs:subClassOf>
        <rdfs:subClassOf>
            <owl:Restriction>
                <owl:onProperty rdf:resource="http://purl.org/ica/ric#RiC-R-hasSubject"/>
                <owl:allValuesFrom>
                    <owl:Class>
                        <owl:unionOf rdf:parseType="Collection">
                            <rdf:Description rdf:about="http://purl.org/ica/ric#RiC-E10-Mandate"/>
                            <rdf:Description rdf:about="http://purl.org/ica/ric#RiC-E13-Place"/>
                            <rdf:Description rdf:about="http://purl.org/ica/ric#RiC-E14-ConceptThing"/>
                            <rdf:Description rdf:about="http://purl.org/ica/ric#RiC-E4-Agent"/>
                            <rdf:Description rdf:about="http://purl.org/ica/ric#RiC-E5-Occupation"/>
                            <rdf:Description rdf:about="http://purl.org/ica/ric#RiC-E6-Position"/>
                            <rdf:Description rdf:about="http://purl.org/ica/ric#RiC-E7-Function"/>
                            <rdf:Description rdf:about="http://purl.org/ica/ric#RiC-E8-FunctionAbstract"/>
                            <rdf:Description rdf:about="http://purl.org/ica/ric#RiC-E9-Activity"/>
                        </owl:unionOf>
                    </owl:Class>
                </owl:allValuesFrom>
            </owl:Restriction>
        </rdfs:subClassOf>
        <rdfs:subClassOf>
            <owl:Restriction>
                <owl:onProperty rdf:resource="http://purl.org/ica/ric#RiC-R-isEvidenceOf"/>
                <owl:allValuesFrom>
                    <owl:Class>
                        <owl:unionOf rdf:parseType="Collection">
                            <rdf:Description rdf:about="http://purl.org/ica/ric#RiC-E10-Mandate"/>
                            <rdf:Description rdf:about="http://purl.org/ica/ric#RiC-E7-Function"/>
                        </owl:unionOf>
                    </owl:Class>
                </owl:allValuesFrom>
            </owl:Restriction>
        </rdfs:subClassOf>
        <rdfs:subClassOf>
            <owl:Restriction>
                <owl:onProperty rdf:resource="http://purl.org/ica/ric#RiC-R-isMemberOf"/>
                <owl:allValuesFrom rdf:resource="http://purl.org/ica/ric#RiC-E3-RecordSet"/>
            </owl:Restriction>
        </rdfs:subClassOf>
        <rdfs:subClassOf>
            <owl:Restriction>
                <owl:onProperty rdf:resource="http://purl.org/ica/ric#RiC-R-wasMemberOf"/>
                <owl:allValuesFrom rdf:resource="http://purl.org/ica/ric#RiC-E3-RecordSet"/>
            </owl:Restriction>
        </rdfs:subClassOf>
        <rdfs:comment xml:lang="en">Class for entity RiC-E3.</rdfs:comment>
        <rdfs:label xml:lang="en">Record Set</rdfs:label>
        <skos:definition xml:lang="en">One or more Records that are intellectually brought together at some Date, by an Agent, wherever the Records may reside and whatever the shared properties or relations among them may be.</skos:definition>
        <skos:example xml:lang="en">Cotton Manuscripts Collection; miscellaneous papers and fragments; papers 1st of the Earls of Liverpool;  official correspondence of the 1  Earl of Liverpool.</skos:example>
        <skos:scopeNote xml:lang="en">By exception, some Records are brought together based on their not belonging in the context of selection to other designated groups: a ‘Miscellaneous’ series for example.</skos:scopeNote>
        <skos:scopeNote xml:lang="en">In a particular context, an Agent (e.g. administrator, records manager, archivist, end-user, etc.) selects the member Records of a Record Set based on a shared property or properties, or a shared Relation or Relations. The grouping of the Records serves a purpose or purposes specific to the context of the Agent.</skos:scopeNote>
        <skos:scopeNote xml:lang="en">One or more Records in one context may be subsumed or incorporated into a Record in another context to form a new Record. Such a ‘compound Record’ should not be confused with a Record Set.</skos:scopeNote>
        <skos:scopeNote xml:lang="en">Record Sets and Records contained within a Record Set may be ordered into a sequence based on a common property or relation, or common properties or relations (e.g. alphabetical by Agent or related Place name); chronological order by an allocated Date; or some other criterion (e.g. an imposed order by relevance).</skos:scopeNote>
        <skos:scopeNote xml:lang="en">Records Sets may also contain other Records Sets. Both a Record Set and a Record may simultaneously be a member of more than one Record Set, and over the course of its existence, a Record Set or Record may be a member of an indeterminate number of Record Sets in an indeterminate number of contexts.</skos:scopeNote>
        <skos:scopeNote xml:lang="en">The selection and grouping, for example, may represent the act of classifying the Records in accordance with a formal classification scheme that may be based on function, subject, organizational structure, or other criteria; an act of archival arrangement (e.g. based on common provenance); or some other selection and grouping that fulfils a particular purpose or purposes (e.g. a classification that reflects or supports the purposes of a researcher). The Record Set created by an Agent in the course of life or work events and Activities should be kept in a manner that preserves context and evidential value.</skos:scopeNote>
    </owl:Class>
    


    <!-- http://purl.org/ica/ric#RiC-E4-Agent -->

    <owl:Class rdf:about="http://purl.org/ica/ric#RiC-E4-Agent">
        <rdfs:subClassOf>
            <owl:Restriction>
                <owl:onProperty rdf:resource="http://purl.org/ica/ric#RiC-R-isMemberOf"/>
                <owl:allValuesFrom rdf:resource="http://purl.org/ica/ric#RiC-E4-Agent-Group"/>
            </owl:Restriction>
        </rdfs:subClassOf>
        <rdfs:subClassOf>
            <owl:Restriction>
                <owl:onProperty rdf:resource="http://purl.org/ica/ric#RiC-R-isSubjectOf"/>
                <owl:allValuesFrom>
                    <owl:Class>
                        <owl:unionOf rdf:parseType="Collection">
                            <rdf:Description rdf:about="http://purl.org/ica/ric#RiC-E1-Record"/>
                            <rdf:Description rdf:about="http://purl.org/ica/ric#RiC-E2-RecordComponent"/>
                            <rdf:Description rdf:about="http://purl.org/ica/ric#RiC-E3-RecordSet"/>
                        </owl:unionOf>
                    </owl:Class>
                </owl:allValuesFrom>
            </owl:Restriction>
        </rdfs:subClassOf>
        <rdfs:subClassOf>
            <owl:Restriction>
                <owl:onProperty rdf:resource="http://purl.org/ica/ric#RiC-R-wasMemberOf"/>
                <owl:allValuesFrom rdf:resource="http://purl.org/ica/ric#RiC-E4-Agent-Group"/>
            </owl:Restriction>
        </rdfs:subClassOf>
        <rdfs:comment xml:lang="en">Class for entity RiC-E4.</rdfs:comment>
        <rdfs:label xml:lang="en">Agent</rdfs:label>
        <skos:definition xml:lang="es">A person or group, or an entity created by a person or group, that is responsible for actions taken and their effects.</skos:definition>
        <skos:scopeNote xml:lang="es">Agent also includes entities created by a person or group that act on behalf of the creating Agent in an autonomous or semi-autonomous manner. Examples of such Delegate-Agents are software agents, robots, and space and underwater probes that generate data (records) in fulfilment of the function assigned to and the instructions given to them by the creating person or group.</skos:scopeNote>
        <skos:scopeNote xml:lang="es">An Agent is known by one or more identities; an identity is a constellation of properties or relations that together “identify” the Agent. Persons or groups commonly have one identity, though they also may have one or more assumed or fictitious identities. Such assumed identities may be shared by more than one person or group. Assumed identities include but are not limited to pseudonyms, heteronyms, DBA (Doing Business As), and trade identities.</skos:scopeNote>
        <skos:scopeNote xml:lang="es">An assumed identity should not be confused with Positions in corporate bodies, for example, presidents, prime ministers, governors, popes, royalty, or bishops.  Nor should an assumed identity be confused with a variant of the same identity.</skos:scopeNote>
        <skos:scopeNote xml:lang="es">Australian Hearing Services; Gilbert and George; Library and Archives Canada; Nelson Mandela; Noel family, Viscounts Campden; The Who; Faculty of Science, University of Strathclyde; France, Ministère de la Culture et de la Communication, direction générale des patrimoines</skos:scopeNote>
        <skos:scopeNote xml:lang="es">Typically archivists will want to attribute responsibility for acting to the person or persons, or group or groups ‘behind’ the assumed identity, but documentation of assumed identities and relating them to the persons or groups whom they represent is important for several reasons: an assumed identity may be the only one known by a user, and thus documentation of an assumed identity and relating it to the person or group identity represented by it facilitates access; an assumed identity may be a significant component of the history of the person or group it represents; an assumed identity may be the subject of records; and, an assumed identity may elide the given identity of the person or group it represents, thus effectively eclipsing or replacing the given identity.</skos:scopeNote>
    </owl:Class>
    


    <!-- http://purl.org/ica/ric#RiC-E4-Agent-DelegateAgent -->

    <owl:Class rdf:about="http://purl.org/ica/ric#RiC-E4-Agent-DelegateAgent">
        <rdfs:subClassOf rdf:resource="http://purl.org/ica/ric#RiC-E4-Agent"/>
        <rdfs:comment xml:lang="en">Defined as a subclass of Agent</rdfs:comment>
        <rdfs:label xml:lang="en">Delegate-agent</rdfs:label>
    </owl:Class>
    


    <!-- http://purl.org/ica/ric#RiC-E4-Agent-Group -->

    <owl:Class rdf:about="http://purl.org/ica/ric#RiC-E4-Agent-Group">
        <rdfs:subClassOf rdf:resource="http://purl.org/ica/ric#RiC-E4-Agent"/>
        <rdfs:subClassOf>
            <owl:Restriction>
                <owl:onProperty rdf:resource="http://purl.org/ica/ric#RiC-R-hadMember"/>
                <owl:allValuesFrom rdf:resource="http://purl.org/ica/ric#RiC-E4-Agent"/>
            </owl:Restriction>
        </rdfs:subClassOf>
        <rdfs:subClassOf>
            <owl:Restriction>
                <owl:onProperty rdf:resource="http://purl.org/ica/ric#RiC-R-hadPart"/>
                <owl:allValuesFrom rdf:resource="http://purl.org/ica/ric#RiC-E4-Agent-Group"/>
            </owl:Restriction>
        </rdfs:subClassOf>
        <rdfs:subClassOf>
            <owl:Restriction>
                <owl:onProperty rdf:resource="http://purl.org/ica/ric#RiC-R-hasMember"/>
                <owl:allValuesFrom rdf:resource="http://purl.org/ica/ric#RiC-E4-Agent"/>
            </owl:Restriction>
        </rdfs:subClassOf>
        <rdfs:subClassOf>
            <owl:Restriction>
                <owl:onProperty rdf:resource="http://purl.org/ica/ric#RiC-R-hasPart"/>
                <owl:allValuesFrom rdf:resource="http://purl.org/ica/ric#RiC-E4-Agent-Group"/>
            </owl:Restriction>
        </rdfs:subClassOf>
        <rdfs:subClassOf>
            <owl:Restriction>
                <owl:onProperty rdf:resource="http://purl.org/ica/ric#RiC-R-isPartOf"/>
                <owl:allValuesFrom rdf:resource="http://purl.org/ica/ric#RiC-E4-Agent-Group"/>
            </owl:Restriction>
        </rdfs:subClassOf>
        <rdfs:subClassOf>
            <owl:Restriction>
                <owl:onProperty rdf:resource="http://purl.org/ica/ric#RiC-R-wasPartOf"/>
                <owl:allValuesFrom rdf:resource="http://purl.org/ica/ric#RiC-E4-Agent-Group"/>
            </owl:Restriction>
        </rdfs:subClassOf>
        <rdfs:comment xml:lang="en">Defined as subclass of Agent</rdfs:comment>
        <rdfs:label xml:lang="en">Group</rdfs:label>
    </owl:Class>
    


    <!-- http://purl.org/ica/ric#RiC-E4-Agent-Person -->

    <owl:Class rdf:about="http://purl.org/ica/ric#RiC-E4-Agent-Person">
        <rdfs:subClassOf rdf:resource="http://purl.org/ica/ric#RiC-E4-Agent"/>
        <rdfs:comment xml:lang="en">Defined as subclass of Agent</rdfs:comment>
        <rdfs:label xml:lang="en">Person</rdfs:label>
    </owl:Class>
    


    <!-- http://purl.org/ica/ric#RiC-E5-Occupation -->

    <owl:Class rdf:about="http://purl.org/ica/ric#RiC-E5-Occupation">
        <rdfs:subClassOf>
            <owl:Restriction>
                <owl:onProperty rdf:resource="http://purl.org/ica/ric#RiC-R-isSubjectOf"/>
                <owl:allValuesFrom>
                    <owl:Class>
                        <owl:unionOf rdf:parseType="Collection">
                            <rdf:Description rdf:about="http://purl.org/ica/ric#RiC-E1-Record"/>
                            <rdf:Description rdf:about="http://purl.org/ica/ric#RiC-E2-RecordComponent"/>
                            <rdf:Description rdf:about="http://purl.org/ica/ric#RiC-E3-RecordSet"/>
                        </owl:unionOf>
                    </owl:Class>
                </owl:allValuesFrom>
            </owl:Restriction>
        </rdfs:subClassOf>
        <rdfs:comment xml:lang="en">Class for entity RiC-E5.</rdfs:comment>
        <rdfs:label xml:lang="en">Occupation</rdfs:label>
        <skos:definition xml:lang="es">A profession, trade, or craft pursued by a person in fulfilment of a Function.</skos:definition>
        <skos:example xml:lang="es">archivist; doctor; lawyer; records manager; teacher</skos:example>
        <skos:scopeNote xml:lang="es">An Occupation may be pursued independently by a person, or pursued within a group, contributing to the fulfillment of the Function of the group.</skos:scopeNote>
        <skos:scopeNote xml:lang="es">Occupation should not be confused with Position, for example, a lawyer that holds the Position of legal counsel in an agency.</skos:scopeNote>
        <skos:scopeNote xml:lang="es">The pursuit of an Occupation involves the performance of an Activity in fulfilment of a Function. Successful performance of the Activity is based on the ability to perform successfully (a competency). This competency may be acquired through education or experience, or a combination of both. The authority of the person to pursue the Occupation may be derived tacitly or explicitly from an external Agent, based on a demonstrated mastery of the competency.</skos:scopeNote>
        <skos:scopeNote xml:lang="es">Though Occupation is related to a domain or field of Activity, it should not be confused with this domain, for example, an archivist works in the domain of archival science.</skos:scopeNote>
    </owl:Class>
    


    <!-- http://purl.org/ica/ric#RiC-E6-Position -->

    <owl:Class rdf:about="http://purl.org/ica/ric#RiC-E6-Position">
        <rdfs:subClassOf>
            <owl:Restriction>
                <owl:onProperty rdf:resource="http://purl.org/ica/ric#RiC-R-isSubjectOf"/>
                <owl:allValuesFrom>
                    <owl:Class>
                        <owl:unionOf rdf:parseType="Collection">
                            <rdf:Description rdf:about="http://purl.org/ica/ric#RiC-E1-Record"/>
                            <rdf:Description rdf:about="http://purl.org/ica/ric#RiC-E2-RecordComponent"/>
                            <rdf:Description rdf:about="http://purl.org/ica/ric#RiC-E3-RecordSet"/>
                        </owl:unionOf>
                    </owl:Class>
                </owl:allValuesFrom>
            </owl:Restriction>
        </rdfs:subClassOf>
        <rdfs:comment xml:lang="en">Class for entity RiC-E6.</rdfs:comment>
        <rdfs:label xml:lang="en">Position</rdfs:label>
        <skos:definition xml:lang="en">A role that may be assigned to a person (or to several persons simultaneously) within a corporate body, and that exists independently of the person(s) who may hold it.</skos:definition>
        <skos:example xml:lang="en">head, president or director of a corporate body or unit of a corporate body; executive manager; technical advisor; assistant of a director; gatekeeper; prime minister</skos:example>
        <skos:scopeNote xml:lang="en">A Position is often defined in a Mandate, which may specify the Functions and competencies necessary to fulfill it, as well as the Activities to be performed.</skos:scopeNote>
        <skos:scopeNote xml:lang="en">A Position is often given a title/name.</skos:scopeNote>
        <skos:scopeNote xml:lang="en">A Position may be tied to a project or to a set of tasks and thus have a defined duration.</skos:scopeNote>
        <skos:scopeNote xml:lang="en">A Position may change over time, as the corporate body that establishes it changes over time. Position is not to be confused with Occupation, which is a profession, trade, or craft pursued by a person in fulfilment of a Function; nor with Function, which is the Agent’s goal; nor with Activity, which is the sets of actions performed by an Agent.</skos:scopeNote>
        <skos:scopeNote xml:lang="en">Within the Records created by a corporate body, the Position entity may be used to identify the Record Sets resulting from Activities performed by persons who hold a Position over time, without necessarily identifying or describing those persons, or identifying which Records were created by each of them.</skos:scopeNote>
    </owl:Class>
    


    <!-- http://purl.org/ica/ric#RiC-E7-Function -->

    <owl:Class rdf:about="http://purl.org/ica/ric#RiC-E7-Function">
        <rdfs:subClassOf>
            <owl:Restriction>
                <owl:onProperty rdf:resource="http://purl.org/ica/ric#RiC-R-hadPart"/>
                <owl:allValuesFrom rdf:resource="http://purl.org/ica/ric#RiC-E7-Function"/>
            </owl:Restriction>
        </rdfs:subClassOf>
        <rdfs:subClassOf>
            <owl:Restriction>
                <owl:onProperty rdf:resource="http://purl.org/ica/ric#RiC-R-hasPart"/>
                <owl:allValuesFrom rdf:resource="http://purl.org/ica/ric#RiC-E7-Function"/>
            </owl:Restriction>
        </rdfs:subClassOf>
        <rdfs:subClassOf>
            <owl:Restriction>
                <owl:onProperty rdf:resource="http://purl.org/ica/ric#RiC-R-isEvidencedBy"/>
                <owl:allValuesFrom>
                    <owl:Class>
                        <owl:unionOf rdf:parseType="Collection">
                            <rdf:Description rdf:about="http://purl.org/ica/ric#RiC-E1-Record"/>
                            <rdf:Description rdf:about="http://purl.org/ica/ric#RiC-E2-RecordComponent"/>
                            <rdf:Description rdf:about="http://purl.org/ica/ric#RiC-E3-RecordSet"/>
                        </owl:unionOf>
                    </owl:Class>
                </owl:allValuesFrom>
            </owl:Restriction>
        </rdfs:subClassOf>
        <rdfs:subClassOf>
            <owl:Restriction>
                <owl:onProperty rdf:resource="http://purl.org/ica/ric#RiC-R-isPartOf"/>
                <owl:allValuesFrom rdf:resource="http://purl.org/ica/ric#RiC-E7-Function"/>
            </owl:Restriction>
        </rdfs:subClassOf>
        <rdfs:subClassOf>
            <owl:Restriction>
                <owl:onProperty rdf:resource="http://purl.org/ica/ric#RiC-R-isSubjectOf"/>
                <owl:allValuesFrom>
                    <owl:Class>
                        <owl:unionOf rdf:parseType="Collection">
                            <rdf:Description rdf:about="http://purl.org/ica/ric#RiC-E1-Record"/>
                            <rdf:Description rdf:about="http://purl.org/ica/ric#RiC-E2-RecordComponent"/>
                            <rdf:Description rdf:about="http://purl.org/ica/ric#RiC-E3-RecordSet"/>
                        </owl:unionOf>
                    </owl:Class>
                </owl:allValuesFrom>
            </owl:Restriction>
        </rdfs:subClassOf>
        <rdfs:subClassOf>
            <owl:Restriction>
                <owl:onProperty rdf:resource="http://purl.org/ica/ric#RiC-R-wasPartOf"/>
                <owl:allValuesFrom rdf:resource="http://purl.org/ica/ric#RiC-E7-Function"/>
            </owl:Restriction>
        </rdfs:subClassOf>
        <rdfs:comment xml:lang="en">Class for entity RiC-E7.</rdfs:comment>
        <rdfs:label xml:lang="en">Function</rdfs:label>
        <skos:definition xml:lang="en">An enduring goal, purpose, or objective of an Agent.</skos:definition>
        <skos:example xml:lang="en">teaching, University of Glasgow; marketing, Army &amp; Navy Stores Ltd.; providing hearing services, research and development, and conducting education about hearing services, Australian Hearing Services</skos:example>
        <skos:scopeNote xml:lang="en">A Function exists in a specific social and cultural context, and within that context is subject to change over time.  It should not be confused with Function (Abstract) which defines a Function independent of a particular context.</skos:scopeNote>
        <skos:scopeNote xml:lang="en">A Function may be composed of other Functions.</skos:scopeNote>
        <skos:scopeNote xml:lang="en">A Function may be related to more than one Agent simultaneously or over time.</skos:scopeNote>
        <skos:scopeNote xml:lang="en">The fulfilment of a Function requires the performance of one or more Activities. Both the Function and performance of the Activities are governed by one or more explicit or implicit Mandates.</skos:scopeNote>
    </owl:Class>
    


    <!-- http://purl.org/ica/ric#RiC-E8-FunctionAbstract -->

    <owl:Class rdf:about="http://purl.org/ica/ric#RiC-E8-FunctionAbstract">
        <rdfs:subClassOf>
            <owl:Restriction>
                <owl:onProperty rdf:resource="http://purl.org/ica/ric#RiC-R-isSubjectOf"/>
                <owl:allValuesFrom>
                    <owl:Class>
                        <owl:unionOf rdf:parseType="Collection">
                            <rdf:Description rdf:about="http://purl.org/ica/ric#RiC-E1-Record"/>
                            <rdf:Description rdf:about="http://purl.org/ica/ric#RiC-E2-RecordComponent"/>
                            <rdf:Description rdf:about="http://purl.org/ica/ric#RiC-E3-RecordSet"/>
                        </owl:unionOf>
                    </owl:Class>
                </owl:allValuesFrom>
            </owl:Restriction>
        </rdfs:subClassOf>
        <rdfs:comment xml:lang="en">Class for entity RiC-E8.</rdfs:comment>
        <rdfs:label xml:lang="en">Function (Abstract)</rdfs:label>
        <skos:definition xml:lang="en">Designation and definition of a Function independent of the instances of the Function that is specific to a particular social and cultural context.</skos:definition>
        <skos:example xml:lang="en">financial budgeting; fundraising; hearing services; research; teaching; marketing; sales; human resources</skos:example>
        <skos:scopeNote xml:lang="en">Function (Abstract) should not be confused with Function, which defines the goals, purposes or objectives of an Agent within its specific context.</skos:scopeNote>
        <skos:scopeNote xml:lang="en">Function (Abstract) will be defined in both global and domain-specific vocabularies.</skos:scopeNote>
    </owl:Class>
    


    <!-- http://purl.org/ica/ric#RiC-E9-Activity -->

    <owl:Class rdf:about="http://purl.org/ica/ric#RiC-E9-Activity">
        <rdfs:subClassOf>
            <owl:Restriction>
                <owl:onProperty rdf:resource="http://purl.org/ica/ric#RiC-R-hadPart"/>
                <owl:allValuesFrom rdf:resource="http://purl.org/ica/ric#RiC-E9-Activity"/>
            </owl:Restriction>
        </rdfs:subClassOf>
        <rdfs:subClassOf>
            <owl:Restriction>
                <owl:onProperty rdf:resource="http://purl.org/ica/ric#RiC-R-hasPart"/>
                <owl:allValuesFrom rdf:resource="http://purl.org/ica/ric#RiC-E9-Activity"/>
            </owl:Restriction>
        </rdfs:subClassOf>
        <rdfs:subClassOf>
            <owl:Restriction>
                <owl:onProperty rdf:resource="http://purl.org/ica/ric#RiC-R-isPartOf"/>
                <owl:allValuesFrom rdf:resource="http://purl.org/ica/ric#RiC-E9-Activity"/>
            </owl:Restriction>
        </rdfs:subClassOf>
        <rdfs:subClassOf>
            <owl:Restriction>
                <owl:onProperty rdf:resource="http://purl.org/ica/ric#RiC-R-isSubjectOf"/>
                <owl:allValuesFrom>
                    <owl:Class>
                        <owl:unionOf rdf:parseType="Collection">
                            <rdf:Description rdf:about="http://purl.org/ica/ric#RiC-E1-Record"/>
                            <rdf:Description rdf:about="http://purl.org/ica/ric#RiC-E2-RecordComponent"/>
                            <rdf:Description rdf:about="http://purl.org/ica/ric#RiC-E3-RecordSet"/>
                        </owl:unionOf>
                    </owl:Class>
                </owl:allValuesFrom>
            </owl:Restriction>
        </rdfs:subClassOf>
        <rdfs:subClassOf>
            <owl:Restriction>
                <owl:onProperty rdf:resource="http://purl.org/ica/ric#RiC-R-wasPartOf"/>
                <owl:allValuesFrom rdf:resource="http://purl.org/ica/ric#RiC-E9-Activity"/>
            </owl:Restriction>
        </rdfs:subClassOf>
        <rdfs:comment xml:lang="en">Class for entity RiC-E9.</rdfs:comment>
        <rdfs:label xml:lang="en">Activity</rdfs:label>
        <skos:definition xml:lang="en">A set of coordinated actions or transactions performed by an Agent in fulfilment of a Function, or in the pursuit of an Occupation.</skos:definition>
        <skos:example xml:lang="en">financial accounting, University of Glasgow; fundraising campaign management, University of Glasgow</skos:example>
        <skos:scopeNote xml:lang="en">Activities exist in a specific social and cultural context, and within that context are subject to change over time.</skos:scopeNote>
        <skos:scopeNote xml:lang="en">Activities may be composed of other Activities.</skos:scopeNote>
        <skos:scopeNote xml:lang="en">An Activity may be performed in fulfilment of one or more Functions or in the pursuit of one or more Occupations, by more than one Agent at the same time or over time.</skos:scopeNote>
        <skos:scopeNote xml:lang="en">The performance of the Activities is governed by one or more explicit or implicit Mandates.</skos:scopeNote>
    </owl:Class>
    


    <!-- 
    ///////////////////////////////////////////////////////////////////////////////////////
    //
    // Annotations
    //
    ///////////////////////////////////////////////////////////////////////////////////////
     -->

    <rdf:Description rdf:about="http://purl.org/ica/ric#RiC-P-accrualStatus">
        <skos:example xml:lang="en">closed; open; unknown</skos:example>
        <rdfs:comment xml:lang="en">Data Type: Controlled Term</rdfs:comment>
        <skos:definition xml:lang="en">Whether or not the Record Set is open for additional accessions of Records or Record Sets.</skos:definition>
        <skos:scopeNote xml:lang="en">Closed indicates that no additional Records or Record Sets will (or are anticipated to) be added to the Record Set. Open indicates that additional Records or Record Sets will (or are expected to) be added to the Record Set.</skos:scopeNote>
        <rdfs:comment xml:lang="en">Property for RiC-P25</rdfs:comment>
        <rdfs:label xml:lang="en">accrual status</rdfs:label>
    </rdf:Description>
    <rdf:Description rdf:about="http://purl.org/ica/ric#RiC-P-classification">
        <skos:scopeNote xml:lang="en">For RiC-P27: This information may be in the form of text, or a term or code maintained in a classification scheme. The criterion or criteria may be represented in a RiC property or relation that is shared by the members in the Record Set. This shared property or relation may belong to both the Record and Record Set, and may also be inherited by descendant members of a Record Set. It depends on how it is represented in the description: if it is a description of the criteria used in forming or assembling the Record Set, then it is a property of the Record Set descendant Records, then it is among the properties that are shared by the descendant Records.</skos:scopeNote>
        <rdfs:label xml:lang="en">classification</rdfs:label>
        <skos:definition xml:lang="en">For RiC-P17: Information on the criterion or criteria that may be used to identify a Record as a member of a Record Set</skos:definition>
        <rdfs:comment xml:lang="en">Property for RiC-P17, RiC-P27</rdfs:comment>
        <skos:example xml:lang="en">BUD-01-F002 [example of a classification number from a corporate file plan]; human resource management; student registration; finnancial affairs; digitization</skos:example>
        <skos:scopeNote xml:lang="en">For RiC-P17: This information may be in the form of text, or a term or code maintained in  a classification scheme. The criterion or criteria may be represented in a RiC property or through a  relation, for example, to a Documentary Form or a Function (Abstract). The Records sharing this property or relation in common identify them as  members of a particular Record Set.</skos:scopeNote>
        <skos:definition>For RiC-P27: Information on the criterion or criteria used in selecting the members of the Record Set.</skos:definition>
        <rdfs:comment xml:lang="en">Data Type: Text or Controlled Code or Term</rdfs:comment>
    </rdf:Description>
    <rdf:Description rdf:about="http://purl.org/ica/ric#RiC-P-contentType">
        <rdfs:label xml:lang="en">content type</rdfs:label>
        <skos:definition xml:lang="en">The fundamental form of communication in which a Record is expressed and the human sense through which it is intended to be perceived.</skos:definition>
        <rdfs:comment xml:lang="en">Property for RiC-P6</rdfs:comment>
        <rdfs:comment xml:lang="en">Data Type: Controlled Term</rdfs:comment>
        <skos:example xml:lang="en">cartographic image; notated music; spoken word; still image; text</skos:example>
    </rdf:Description>
    <rdf:Description rdf:about="http://purl.org/ica/ric#RiC-P-encodingFormat">
        <rdfs:label xml:lang="en">encoding format</rdfs:label>
        <skos:definition xml:lang="en">Information about the logical form of digitally represented content.</skos:definition>
        <rdfs:comment xml:lang="en">Property for RiC-P10</rdfs:comment>
        <skos:example xml:lang="en">text/csv</skos:example>
        <rdfs:comment xml:lang="en">Data Type: Controlled Term (Mime types: http://www.iana.org/assignments/media-types/media-types.xhtml)</rdfs:comment>
    </rdf:Description>
    <rdf:Description rdf:about="http://purl.org/ica/ric#RiC-P-gender">
        <rdfs:comment xml:lang="en">Data Type: Controlled Term</rdfs:comment>
        <skos:example xml:lang="en">male; female; unknown</skos:example>
        <rdfs:label xml:lang="en">gender</rdfs:label>
        <rdfs:comment xml:lang="en">Property for RiC-P36</rdfs:comment>
        <skos:definition xml:lang="en">The gender with which a person (or person assumed identity) identifies.</skos:definition>
    </rdf:Description>
    <rdf:Description rdf:about="http://purl.org/ica/ric#RiC-P-geographicCoordinates">
        <skos:definition xml:lang="en">Longitudinal and latitudinal information of the Place.</skos:definition>
        <rdfs:label xml:lang="en">geographic coordinates</rdfs:label>
        <rdfs:comment xml:lang="en">Data Type: Controlled Code or Term  (ISO 6709 Standard representation of geographic point location by coordinates)</rdfs:comment>
        <rdfs:comment xml:lang="en">Property for RiC-P64.</rdfs:comment>
    </rdf:Description>
    <rdf:Description rdf:about="http://purl.org/ica/ric#RiC-P-identityType">
        <rdfs:comment xml:lang="en">Property for RiC-P33</rdfs:comment>
        <rdfs:label xml:lang="en">identity type</rdfs:label>
        <skos:definition xml:lang="en">The specific kind of identity of an Agent.</skos:definition>
        <skos:scopeNote xml:lang="en">A given identity is the identity that is commonly considered the identity of the ‘real’ Agent. An assumed identity is an identity invented by one or more ‘real’ Agents, with the ‘real’ Agent or Agents acting under the guise of the assumed identity.</skos:scopeNote>
        <rdfs:comment xml:lang="en">Data Type: Controlled Term</rdfs:comment>
        <skos:example xml:lang="en">given; individual assumed; joint assumed; unknown</skos:example>
    </rdf:Description>
    <rdf:Description rdf:about="http://purl.org/ica/ric#RiC-P-languageInformation">
        <rdfs:comment xml:lang="en">Data Type: Controlled Code or Term (ISO 639 Codes for the representation of names of languages; ISO 15924 Codes for the representation of names and scripts)</rdfs:comment>
        <skos:example xml:lang="en">Languages: Arabic (ara); Chinese (chi); English (eng); French (fre); Spanish (spa)

Scripts: Arabic (Arab); Han (Hans); Latin (Latn)

Transliteration scheme: ISO 233-2:1993 Information and documentation - Translation of Arabic characters into Latin characters - Part 2: Arabic language - Simplified transliteration; ISO 843:1997 Information and documentation -- Conversion of Greek characters into Latin characters</skos:example>
        <rdfs:label xml:lang="en">language information</rdfs:label>
        <skos:definition xml:lang="en">A spoken or written human language represented in the Records.</skos:definition>
        <skos:scopeNote xml:lang="en">Information includes the language, the script of the language, and the script transliteration scheme when appropriate. More than one language may be represented in a Record.</skos:scopeNote>
        <rdfs:comment xml:lang="en">Property for RiC-P11, RiC-P34</rdfs:comment>
    </rdf:Description>
    <rdf:Description rdf:about="http://purl.org/ica/ric#RiC-P-mediaType">
        <skos:example xml:lang="en">audio; computer; microform; unmediated; video</skos:example>
        <rdfs:comment xml:lang="en">Data Type: Controlled Term</rdfs:comment>
        <rdfs:comment xml:lang="en">Property for RiC-P12</rdfs:comment>
        <skos:definition xml:lang="en">The general type of intermediation device required to render the content of a Record.</skos:definition>
        <rdfs:label xml:lang="en">media type</rdfs:label>
    </rdf:Description>
    <rdf:Description rdf:about="http://purl.org/ica/ric#RiC-P-medium">
        <skos:definition xml:lang="en">Physical material in or on which information is represented.</skos:definition>
        <rdfs:comment xml:lang="en">Data Type: Controlled Term</rdfs:comment>
        <skos:scopeNote xml:lang="en">Includes physical carriers in or on which information is represented that do not require an intermediation device.</skos:scopeNote>
        <rdfs:comment xml:lang="en">Property for RiC-P14</rdfs:comment>
        <rdfs:label xml:lang="en">medium</rdfs:label>
        <skos:example xml:lang="en">clay tablets; papyrus; magnetic disk; optical disk; paper; parchment; film; vinyl disk; magnetic tape</skos:example>
    </rdf:Description>
    <rdf:Description rdf:about="http://purl.org/ica/ric#RiC-P-name">
        <skos:definition xml:lang="en">Text for a title or term designating the entity.</skos:definition>
        <rdfs:comment xml:lang="en">Data Type: Text, or Controlled Phrase, or Controlled Term, or Controlled Format</rdfs:comment>
        <rdfs:label xml:lang="en">name</rdfs:label>
        <skos:example xml:lang="en">4 March 1842; deed of gift; doctor; fundraising, University of Glasgow; hearing services; Nelson Mandela; Papers of the Earls of Liverpool; París; prime minister; Sketch Map of the Qatar Peninsula</skos:example>
        <rdfs:comment xml:lang="en">Property RiC-P3 (text)</rdfs:comment>
    </rdf:Description>
    <rdf:Description rdf:about="http://purl.org/ica/ric#RiC-P-place">
        <skos:scopeNote xml:lang="en">Includes settlements of any kind (towns, villages, etc.), historical regions, political and administrative districts, and geographical features. If applicable, includes the geographical or administrative point or area (e.g. district, country, state) where the relation between two entities exists.</skos:scopeNote>
        <rdfs:label xml:lang="en">place</rdfs:label>
        <skos:definition xml:lang="en">Jurisdictions and named geographical features.</skos:definition>
        <skos:example xml:lang="en">Amazon River; Nova Scotia; Paris</skos:example>
        <rdfs:comment xml:lang="en">Property for RiC-P69.</rdfs:comment>
        <rdfs:comment xml:lang="en">Data Type: Controlled Term or Phrase</rdfs:comment>
    </rdf:Description>
    <rdf:Description rdf:about="http://purl.org/ica/ric#RiC-P-productionTechnique">
        <skos:definition xml:lang="en">The method used in the representation of information on the Record carrier.</skos:definition>
        <rdfs:comment xml:lang="en">Data Type: Text or Controlled Term</rdfs:comment>
        <rdfs:comment xml:lang="en">Property for RiC-P13</rdfs:comment>
        <skos:example xml:lang="en">manuscription (handwriting); engraving; magnetic recording; optical recording</skos:example>
        <rdfs:label xml:lang="en">production technique</rdfs:label>
    </rdf:Description>
    <rdf:Description rdf:about="http://purl.org/ica/ric#RiC-P-recordState">
        <rdfs:comment xml:lang="en">Property for RiC-P21</rdfs:comment>
        <skos:definition xml:lang="en">Description of the production or reproduction status of the Record.</skos:definition>
        <rdfs:label xml:lang="en">record state</rdfs:label>
        <skos:example xml:lang="en">draft; final draft; original; simple copy; certified copy</skos:example>
        <rdfs:comment xml:lang="en">Data Type: Text or Controlled Term</rdfs:comment>
    </rdf:Description>
    <rdf:Description rdf:about="http://purl.org/ica/ric#RiC-P-type">
        <skos:definition xml:lang="en">For RiC-P52: Categorization of the Activity.</skos:definition>
        <skos:example xml:lang="en">For RiC-P32: group; corporate body; conference; family; person; delegate-agent; unknown</skos:example>
        <skos:example xml:lang="en">For RiC-P61: single; range.</skos:example>
        <skos:example xml:lang="en">For RiC-P52: activity; business process; action; task; transaction</skos:example>
        <skos:definition xml:lang="en">For RiC-P48: Categorization of the Function.</skos:definition>
        <skos:definition xml:lang="en">For RiC-P42: Categorization of the Occupation.</skos:definition>
        <skos:definition xml:lang="en">For RiC-P66: Categorization of the Concept/Thing.</skos:definition>
        <skos:example xml:lang="en">For RiC-P63: settlement; administrative division; country; mountain; river.</skos:example>
        <rdfs:comment xml:lang="en">Property for RiC-P23, RiC-P32, RiC-P42, RiC-P45, RiC-P48, RiC-P52, RiC-P55, RiC-P58, RiC-P61, RiC-P63, RiC-P66</rdfs:comment>
        <skos:definition xml:lang="en">For RiC-P32: Specific kind of Agent.</skos:definition>
        <skos:example xml:lang="en">For RiC-P45: academic; administrative and professional; operational; technical</skos:example>
        <rdfs:label xml:lang="en">type</rdfs:label>
        <skos:definition xml:lang="en">For RiC-P58: Categorization of the Documentary Form.</skos:definition>
        <skos:definition xml:lang="en">For RiC-P23: A broad categorization of the type of Record Set.</skos:definition>
        <skos:example xml:lang="en">For RiC-P58: long playing record (LP); charter; register</skos:example>
        <skos:scopeNote xml:lang="en">For RiC-P23: For legacy purposes this type is the equivalent of the Level of Description element in ISAD(G) (3.1.4) except for the value &quot;item&quot;, which equates to the Record entity in RiC. Record Set Type may be extended to reflect types of Record Sets that are not
archival.</skos:scopeNote>
        <skos:definition xml:lang="en">For RiC-P63: An indication of the category of Place, especially to distinguish natural and  human notions.</skos:definition>
        <skos:definition xml:lang="en">For RiC-P45: Categorization of the Position using either a list of types established external  to or within the institution.</skos:definition>
        <skos:example xml:lang="en">For RiC-P42: health professionals; legal professionals; service and sales workers</skos:example>
        <skos:example xml:lang="en">For RiC-P48: funcion; sub-function</skos:example>
        <skos:definition xml:lang="en">For RiC-P61: Categorization of the Date.</skos:definition>
        <skos:definition xml:lang="en">For RiC-P55: Categorization of the Mandate.</skos:definition>
        <rdfs:comment xml:lang="en">Data Type: Controlled Term (or Phrase for RiC-P63)</rdfs:comment>
        <skos:example xml:lang="en">For RiC-P55: decree; legislation; rule; standard; letter of appointment</skos:example>
        <skos:example xml:lang="en">For RiC-P23: fonds; series; file; class; piece; collection; accrual; accession; project.</skos:example>
        <skos:scopeNote xml:lang="en">For RiC-P32: The top level types define groups (including families, corporate bodies and conferences), persons and delegate-agents created by a person or group that act on behalf of the creating Agent in an autonomous or semi-autonomous manner. If the type is unknown that this should be stated. Each type may be extended to cover more specific categorization, for example, to distinguish between public and private corporate bodies, or to specify the legal status of the Agent according to some international or local scheme. Not all properties under Agent apply to all types.</skos:scopeNote>
    </rdf:Description>
</rdf:RDF>



<!-- Generated by the OWL API (version 4.2.8.20170104-2310) https://github.com/owlcs/owlapi -->

